include/s2n-bignum-c89.h
@@ -990,16 +990,16 @@ extern void edwards25519_scalarmuldouble(uint64_t res[8],uint64_t scalar[4], uin
 extern void edwards25519_scalarmuldouble_alt(uint64_t res[8],uint64_t scalar[4], uint64_t point[8],uint64_t bscalar[4]);
 
 /* Inverse number-theoretic transform from ML-KEM */
-/* Input a[256] (signed 16-bit words); output a[256] (signed 16-bit words) */
-extern void mlkem_intt(int16_t a[256]);
+/* Input a[256] (signed 16-bit words), z_01234[80] (signed 16-bit words), z_56[384] (signed 16-bit words); output a[256] (signed 16-bit words) */
+extern void mlkem_intt(int16_t a[256],int16_t z_01234[80],int16_t z_56[384]);
 
 /* Keccak-f1600 permutation for SHA3 */
 /* Input a[25]; output a[25] */
 extern void mlkem_keccak_f1600(uint64_t a[25]);
 
 /* Forward number-theoretic transform from ML-KEM */
-/* Input a[256] (signed 16-bit words); output a[256] (signed 16-bit words) */
-extern void mlkem_ntt(int16_t a[256]);
+/* Input a[256] (signed 16-bit words), z_01234[80] (signed 16-bit words), z_56[384] (signed 16-bit words); output a[256] (signed 16-bit words) */
+extern void mlkem_ntt(int16_t a[256],int16_t z_01234[80],int16_t z_56[384]);
 
 /* Point addition on NIST curve P-256 in Montgomery-Jacobian coordinates */
 /* Inputs p1[12], p2[12]; output p3[12] */
