include/s2n-bignum.h
@@ -1004,16 +1004,16 @@ extern void edwards25519_scalarmuldouble(uint64_t res[S2N_BIGNUM_STATIC 8],uint6
 extern void edwards25519_scalarmuldouble_alt(uint64_t res[S2N_BIGNUM_STATIC 8],uint64_t scalar[S2N_BIGNUM_STATIC 4], uint64_t point[S2N_BIGNUM_STATIC 8],uint64_t bscalar[S2N_BIGNUM_STATIC 4]);
 
 // Inverse number-theoretic transform from ML-KEM
-// Input a[256] (signed 16-bit words); output a[256] (signed 16-bit words)
-extern void mlkem_intt(int16_t a[S2N_BIGNUM_STATIC 256]);
+// Input a[256] (signed 16-bit words), z_01234[80] (signed 16-bit words), z_56[384] (signed 16-bit words); output a[256] (signed 16-bit words)
+extern void mlkem_intt(int16_t a[S2N_BIGNUM_STATIC 256],int16_t z_01234[S2N_BIGNUM_STATIC 80],int16_t z_56[S2N_BIGNUM_STATIC 384]);
 
 // Keccak-f1600 permutation for SHA3
 // Input a[25]; output a[25]
 extern void mlkem_keccak_f1600(uint64_t a[S2N_BIGNUM_STATIC 25]);
 
 // Forward number-theoretic transform from ML-KEM
-// Input a[256] (signed 16-bit words); output a[256] (signed 16-bit words)
-extern void mlkem_ntt(int16_t a[S2N_BIGNUM_STATIC 256]);
+// Input a[256] (signed 16-bit words), z_01234[80] (signed 16-bit words), z_56[384] (signed 16-bit words); output a[256] (signed 16-bit words)
+extern void mlkem_ntt(int16_t a[S2N_BIGNUM_STATIC 256],int16_t z_01234[S2N_BIGNUM_STATIC 80],int16_t z_56[S2N_BIGNUM_STATIC 384]);
 
 // Point addition on NIST curve P-256 in Montgomery-Jacobian coordinates
 // Inputs p1[12], p2[12]; output p3[12]
