arm/proofs/mlkem_intt.ml
@@ -10,20 +10,17 @@
 needs "arm/proofs/base.ml";;
 needs "arm/proofs/utils/mlkem.ml";;
 
-(**** print_coda_from_elf (-1) "arm/mlkem/mlkem_intt.o";;
+(**** print_literal_from_elf "arm/mlkem/mlkem_intt.o";;
  ****)
 
-let mlkem_intt_mc,mlkem_intt_data = define_coda_literal_from_elf
-  "mlkem_intt_mc" "mlkem_intt_data" "arm/mlkem/mlkem_intt.o"
+let mlkem_intt_mc = define_assert_from_elf
+ "mlkem_intt_mc" "arm/mlkem/mlkem_intt.o"
 [
   0xd10103ff;       (* arm_SUB SP SP (rvalue (word 64)) *)
-  0x6d0027e8;       (* arm_STP D8 D9 SP (Immediate_Offset (word 0)) *)
-  0x6d012fea;       (* arm_STP D10 D11 SP (Immediate_Offset (word 16)) *)
-  0x6d0237ec;       (* arm_STP D12 D13 SP (Immediate_Offset (word 32)) *)
-  0x6d033fee;       (* arm_STP D14 D15 SP (Immediate_Offset (word 48)) *)
-  0x10004641;       (* arm_ADR X1 (word 2248) *)
-  0x10002e22;       (* arm_ADR X2 (word 1476) *)
-  0x4e020fe7;       (* arm_DUP_GEN Q7 XZR 16 128 *)
+  0x6d0027e8;       (* arm_STP D8 D9 SP (Immediate_Offset (iword (&0))) *)
+  0x6d012fea;       (* arm_STP D10 D11 SP (Immediate_Offset (iword (&16))) *)
+  0x6d0237ec;       (* arm_STP D12 D13 SP (Immediate_Offset (iword (&32))) *)
+  0x6d033fee;       (* arm_STP D14 D15 SP (Immediate_Offset (iword (&48))) *)
   0x5281a025;       (* arm_MOV W5 (rvalue (word 3329)) *)
   0x4e021ca7;       (* arm_INS_GEN Q7 W5 0 16 *)
   0x5289d7e5;       (* arm_MOV W5 (rvalue (word 20159)) *)
@@ -58,399 +55,420 @@ let mlkem_intt_mc,mlkem_intt_data = define_coda_literal_from_elf
   0xb5fffd64;       (* arm_CBNZ X4 (word 2097068) *)
   0xaa0003e3;       (* arm_MOV X3 X0 *)
   0xd2800104;       (* arm_MOV X4 (rvalue (word 8)) *)
-  0x3dc0087b;       (* arm_LDR Q27 X3 (Immediate_Offset (word 32)) *)
-  0x3dc00c6d;       (* arm_LDR Q13 X3 (Immediate_Offset (word 48)) *)
-  0x3dc00062;       (* arm_LDR Q2 X3 (Immediate_Offset (word 0)) *)
-  0x3dc0047c;       (* arm_LDR Q28 X3 (Immediate_Offset (word 16)) *)
-  0x3dc00c49;       (* arm_LDR Q9 X2 (Immediate_Offset (word 48)) *)
-  0x3dc00456;       (* arm_LDR Q22 X2 (Immediate_Offset (word 16)) *)
-  0x3dc01051;       (* arm_LDR Q17 X2 (Immediate_Offset (word 64)) *)
-  0x3dc0144e;       (* arm_LDR Q14 X2 (Immediate_Offset (word 80)) *)
-  0x4e8d2b77;       (* arm_TRN1 Q23 Q27 Q13 32 128 *)
-  0x4e8d6b7b;       (* arm_TRN2 Q27 Q27 Q13 32 128 *)
-  0x4e9c284d;       (* arm_TRN1 Q13 Q2 Q28 32 128 *)
-  0x4e9c6842;       (* arm_TRN2 Q2 Q2 Q28 32 128 *)
-  0x3dc0085c;       (* arm_LDR Q28 X2 (Immediate_Offset (word 32)) *)
-  0x3cc60444;       (* arm_LDR Q4 X2 (Postimmediate_Offset (word 96)) *)
-  0x4ed769b8;       (* arm_TRN2 Q24 Q13 Q23 64 128 *)
-  0x4edb684f;       (* arm_TRN2 Q15 Q2 Q27 64 128 *)
-  0x4ed729ad;       (* arm_TRN1 Q13 Q13 Q23 64 128 *)
-  0x4edb285b;       (* arm_TRN1 Q27 Q2 Q27 64 128 *)
-  0x4e6f8702;       (* arm_ADD_VEC Q2 Q24 Q15 16 128 *)
-  0x6e6f8717;       (* arm_SUB_VEC Q23 Q24 Q15 16 128 *)
-  0x4e7b85b8;       (* arm_ADD_VEC Q24 Q13 Q27 16 128 *)
-  0x6e7b85bb;       (* arm_SUB_VEC Q27 Q13 Q27 16 128 *)
-  0x3cc1042f;       (* arm_LDR Q15 X1 (Postimmediate_Offset (word 16)) *)
-  0x4e719ef1;       (* arm_MUL_VEC Q17 Q23 Q17 16 128 *)
-  0x6e69b76d;       (* arm_SQRDMULH_VEC Q13 Q27 Q9 16 128 *)
-  0x6e6eb6ee;       (* arm_SQRDMULH_VEC Q14 Q23 Q14 16 128 *)
-  0x4e7c9f7b;       (* arm_MUL_VEC Q27 Q27 Q28 16 128 *)
-  0x6f4741bb;       (* arm_MLS_VEC Q27 Q13 (Q7 :> LANE_H 0) 16 128 *)
-  0x6e628709;       (* arm_SUB_VEC Q9 Q24 Q2 16 128 *)
-  0x6f4741d1;       (* arm_MLS_VEC Q17 Q14 (Q7 :> LANE_H 0) 16 128 *)
-  0x6e76b52d;       (* arm_SQRDMULH_VEC Q13 Q9 Q22 16 128 *)
-  0x4e628702;       (* arm_ADD_VEC Q2 Q24 Q2 16 128 *)
-  0x4e649d3c;       (* arm_MUL_VEC Q28 Q9 Q4 16 128 *)
-  0x6e718769;       (* arm_SUB_VEC Q9 Q27 Q17 16 128 *)
-  0x4e71877b;       (* arm_ADD_VEC Q27 Q27 Q17 16 128 *)
-  0x6e76b536;       (* arm_SQRDMULH_VEC Q22 Q9 Q22 16 128 *)
-  0x4e9b2851;       (* arm_TRN1 Q17 Q2 Q27 32 128 *)
-  0x4e649d29;       (* arm_MUL_VEC Q9 Q9 Q4 16 128 *)
-  0x4e9b684a;       (* arm_TRN2 Q10 Q2 Q27 32 128 *)
-  0x6f4741bc;       (* arm_MLS_VEC Q28 Q13 (Q7 :> LANE_H 0) 16 128 *)
-  0x6f4742c9;       (* arm_MLS_VEC Q9 Q22 (Q7 :> LANE_H 0) 16 128 *)
-  0x4e896b82;       (* arm_TRN2 Q2 Q28 Q9 32 128 *)
-  0x4e892b8d;       (* arm_TRN1 Q13 Q28 Q9 32 128 *)
-  0x4ecd6a36;       (* arm_TRN2 Q22 Q17 Q13 64 128 *)
-  0x4ec2695c;       (* arm_TRN2 Q28 Q10 Q2 64 128 *)
-  0x4ecd2a29;       (* arm_TRN1 Q9 Q17 Q13 64 128 *)
-  0x6e7c86db;       (* arm_SUB_VEC Q27 Q22 Q28 16 128 *)
-  0x4ec22952;       (* arm_TRN1 Q18 Q10 Q2 64 128 *)
-  0x4e7c86ce;       (* arm_ADD_VEC Q14 Q22 Q28 16 128 *)
-  0x4f5fdb74;       (* arm_SQRDMULH_VEC Q20 Q27 (Q15 :> LANE_H 5) 16 128 *)
-  0x4f4f8b75;       (* arm_MUL_VEC Q21 Q27 (Q15 :> LANE_H 4) 16 128 *)
-  0xd1000484;       (* arm_SUB X4 X4 (rvalue (word 1)) *)
-  0x4f57c1d7;       (* arm_SQDMULH_VEC Q23 Q14 (Q7 :> LANE_H 1) 16 128 *)
-  0x6e72853a;       (* arm_SUB_VEC Q26 Q9 Q18 16 128 *)
-  0x3dc01866;       (* arm_LDR Q6 X3 (Immediate_Offset (word 96)) *)
-  0x3dc01c7c;       (* arm_LDR Q28 X3 (Immediate_Offset (word 112)) *)
-  0x6f474295;       (* arm_MLS_VEC Q21 Q20 (Q7 :> LANE_H 0) 16 128 *)
-  0x3dc0106b;       (* arm_LDR Q11 X3 (Immediate_Offset (word 64)) *)
-  0x3dc01465;       (* arm_LDR Q5 X3 (Immediate_Offset (word 80)) *)
-  0x3dc00459;       (* arm_LDR Q25 X2 (Immediate_Offset (word 16)) *)
-  0x4e72852d;       (* arm_ADD_VEC Q13 Q9 Q18 16 128 *)
-  0x4f7fd34a;       (* arm_SQRDMULH_VEC Q10 Q26 (Q15 :> LANE_H 3) 16 128 *)
-  0x4e9c28dd;       (* arm_TRN1 Q29 Q6 Q28 32 128 *)
-  0x3dc00c50;       (* arm_LDR Q16 X2 (Immediate_Offset (word 48)) *)
-  0x4e9c68c1;       (* arm_TRN2 Q1 Q6 Q28 32 128 *)
-  0x4f6f8351;       (* arm_MUL_VEC Q17 Q26 (Q15 :> LANE_H 2) 16 128 *)
-  0x4e852972;       (* arm_TRN1 Q18 Q11 Q5 32 128 *)
+  0x3dc00c77;       (* arm_LDR Q23 X3 (Immediate_Offset (word 48)) *)
+  0x3dc0087c;       (* arm_LDR Q28 X3 (Immediate_Offset (word 32)) *)
+  0x3dc0046d;       (* arm_LDR Q13 X3 (Immediate_Offset (word 16)) *)
+  0x3dc00064;       (* arm_LDR Q4 X3 (Immediate_Offset (word 0)) *)
+  0x3dc00c59;       (* arm_LDR Q25 X2 (Immediate_Offset (word 48)) *)
+  0x3dc01450;       (* arm_LDR Q16 X2 (Immediate_Offset (word 80)) *)
+  0x3cc1042c;       (* arm_LDR Q12 X1 (Postimmediate_Offset (word 16)) *)
+  0x4e976b96;       (* arm_TRN2 Q22 Q28 Q23 32 128 *)
+  0x4e972b9d;       (* arm_TRN1 Q29 Q28 Q23 32 128 *)
+  0x4e8d2886;       (* arm_TRN1 Q6 Q4 Q13 32 128 *)
+  0x4e8d6892;       (* arm_TRN2 Q18 Q4 Q13 32 128 *)
+  0x4edd68de;       (* arm_TRN2 Q30 Q6 Q29 64 128 *)
+  0x4ed66a43;       (* arm_TRN2 Q3 Q18 Q22 64 128 *)
+  0x4edd28c5;       (* arm_TRN1 Q5 Q6 Q29 64 128 *)
   0x3dc01049;       (* arm_LDR Q9 X2 (Immediate_Offset (word 64)) *)
-  0x4e85697e;       (* arm_TRN2 Q30 Q11 Q5 32 128 *)
-  0x4f57c1b4;       (* arm_SQDMULH_VEC Q20 Q13 (Q7 :> LANE_H 1) 16 128 *)
-  0x4edd6a5a;       (* arm_TRN2 Q26 Q18 Q29 64 128 *)
-  0x3dc0145b;       (* arm_LDR Q27 X2 (Immediate_Offset (word 80)) *)
-  0x6f474151;       (* arm_MLS_VEC Q17 Q10 (Q7 :> LANE_H 0) 16 128 *)
-  0x4ec16bd8;       (* arm_TRN2 Q24 Q30 Q1 64 128 *)
-  0x4edd2a5f;       (* arm_TRN1 Q31 Q18 Q29 64 128 *)
-  0x3dc0084c;       (* arm_LDR Q12 X2 (Immediate_Offset (word 32)) *)
-  0x6e788753;       (* arm_SUB_VEC Q19 Q26 Q24 16 128 *)
-  0x4f57c2ab;       (* arm_SQDMULH_VEC Q11 Q21 (Q7 :> LANE_H 1) 16 128 *)
-  0x4ec12bc0;       (* arm_TRN1 Q0 Q30 Q1 64 128 *)
-  0x6e7bb666;       (* arm_SQRDMULH_VEC Q6 Q19 Q27 16 128 *)
-  0x6e6087ea;       (* arm_SUB_VEC Q10 Q31 Q0 16 128 *)
-  0x4f152682;       (* arm_SRSHR_VEC Q2 Q20 11 16 128 *)
-  0x4f57c228;       (* arm_SQDMULH_VEC Q8 Q17 (Q7 :> LANE_H 1) 16 128 *)
-  0x4e6087ff;       (* arm_ADD_VEC Q31 Q31 Q0 16 128 *)
-  0x3cc60440;       (* arm_LDR Q0 X2 (Postimmediate_Offset (word 96)) *)
-  0x6e70b55d;       (* arm_SQRDMULH_VEC Q29 Q10 Q16 16 128 *)
-  0x4e78875b;       (* arm_ADD_VEC Q27 Q26 Q24 16 128 *)
-  0x4f152563;       (* arm_SRSHR_VEC Q3 Q11 11 16 128 *)
-  0x4e6c9d56;       (* arm_MUL_VEC Q22 Q10 Q12 16 128 *)
-  0x6e7b87fc;       (* arm_SUB_VEC Q28 Q31 Q27 16 128 *)
-  0x4e7b87e4;       (* arm_ADD_VEC Q4 Q31 Q27 16 128 *)
-  0x4f152508;       (* arm_SRSHR_VEC Q8 Q8 11 16 128 *)
-  0x6e79b78a;       (* arm_SQRDMULH_VEC Q10 Q28 Q25 16 128 *)
-  0x4f1526ec;       (* arm_SRSHR_VEC Q12 Q23 11 16 128 *)
-  0x6f4743b6;       (* arm_MLS_VEC Q22 Q29 (Q7 :> LANE_H 0) 16 128 *)
-  0x6f474111;       (* arm_MLS_VEC Q17 Q8 (Q7 :> LANE_H 0) 16 128 *)
-  0x6f474075;       (* arm_MLS_VEC Q21 Q3 (Q7 :> LANE_H 0) 16 128 *)
-  0x4e699e7b;       (* arm_MUL_VEC Q27 Q19 Q9 16 128 *)
-  0x6f4740db;       (* arm_MLS_VEC Q27 Q6 (Q7 :> LANE_H 0) 16 128 *)
-  0x6f47404d;       (* arm_MLS_VEC Q13 Q2 (Q7 :> LANE_H 0) 16 128 *)
-  0x6f47418e;       (* arm_MLS_VEC Q14 Q12 (Q7 :> LANE_H 0) 16 128 *)
-  0x4e609f89;       (* arm_MUL_VEC Q9 Q28 Q0 16 128 *)
-  0x6e7b86c8;       (* arm_SUB_VEC Q8 Q22 Q27 16 128 *)
-  0x4e7b86d7;       (* arm_ADD_VEC Q23 Q22 Q27 16 128 *)
-  0x6e79b505;       (* arm_SQRDMULH_VEC Q5 Q8 Q25 16 128 *)
-  0x6e6e85a1;       (* arm_SUB_VEC Q1 Q13 Q14 16 128 *)
-  0x4e609d19;       (* arm_MUL_VEC Q25 Q8 Q0 16 128 *)
-  0x4e6e85a2;       (* arm_ADD_VEC Q2 Q13 Q14 16 128 *)
-  0x4e972880;       (* arm_TRN1 Q0 Q4 Q23 32 128 *)
-  0x6f474149;       (* arm_MLS_VEC Q9 Q10 (Q7 :> LANE_H 0) 16 128 *)
-  0x4e97688a;       (* arm_TRN2 Q10 Q4 Q23 32 128 *)
-  0x6f4740b9;       (* arm_MLS_VEC Q25 Q5 (Q7 :> LANE_H 0) 16 128 *)
-  0x4f5fd033;       (* arm_SQRDMULH_VEC Q19 Q1 (Q15 :> LANE_H 1) 16 128 *)
-  0x4f4f8030;       (* arm_MUL_VEC Q16 Q1 (Q15 :> LANE_H 0) 16 128 *)
-  0x6e758626;       (* arm_SUB_VEC Q6 Q17 Q21 16 128 *)
-  0x4e99293f;       (* arm_TRN1 Q31 Q9 Q25 32 128 *)
-  0x4e996924;       (* arm_TRN2 Q4 Q9 Q25 32 128 *)
-  0x4f5fd0cc;       (* arm_SQRDMULH_VEC Q12 Q6 (Q15 :> LANE_H 1) 16 128 *)
-  0x4edf2809;       (* arm_TRN1 Q9 Q0 Q31 64 128 *)
-  0x6f474270;       (* arm_MLS_VEC Q16 Q19 (Q7 :> LANE_H 0) 16 128 *)
-  0x4ec46957;       (* arm_TRN2 Q23 Q10 Q4 64 128 *)
-  0x4edf6808;       (* arm_TRN2 Q8 Q0 Q31 64 128 *)
-  0x4f4f80db;       (* arm_MUL_VEC Q27 Q6 (Q15 :> LANE_H 0) 16 128 *)
-  0x3cc1042f;       (* arm_LDR Q15 X1 (Postimmediate_Offset (word 16)) *)
-  0x4ec42952;       (* arm_TRN1 Q18 Q10 Q4 64 128 *)
-  0x6f47419b;       (* arm_MLS_VEC Q27 Q12 (Q7 :> LANE_H 0) 16 128 *)
-  0x6e778506;       (* arm_SUB_VEC Q6 Q8 Q23 16 128 *)
-  0x4e75862a;       (* arm_ADD_VEC Q10 Q17 Q21 16 128 *)
-  0x3d800870;       (* arm_STR Q16 X3 (Immediate_Offset (word 32)) *)
-  0x4e77850e;       (* arm_ADD_VEC Q14 Q8 Q23 16 128 *)
-  0x4f5fd8d4;       (* arm_SQRDMULH_VEC Q20 Q6 (Q15 :> LANE_H 5) 16 128 *)
-  0x3d80046a;       (* arm_STR Q10 X3 (Immediate_Offset (word 16)) *)
-  0x3c840462;       (* arm_STR Q2 X3 (Postimmediate_Offset (word 64)) *)
-  0x4f4f88d5;       (* arm_MUL_VEC Q21 Q6 (Q15 :> LANE_H 4) 16 128 *)
-  0x3c9f007b;       (* arm_STR Q27 X3 (Immediate_Offset (word 18446744073709551600)) *)
+  0x6e6387d4;       (* arm_SUB_VEC Q20 Q30 Q3 16 128 *)
+  0x4ed62a5b;       (* arm_TRN1 Q27 Q18 Q22 64 128 *)
+  0x4e6387c0;       (* arm_ADD_VEC Q0 Q30 Q3 16 128 *)
+  0x6e70b68f;       (* arm_SQRDMULH_VEC Q15 Q20 Q16 16 128 *)
+  0x4e7b84b6;       (* arm_ADD_VEC Q22 Q5 Q27 16 128 *)
+  0x6e7b84b3;       (* arm_SUB_VEC Q19 Q5 Q27 16 128 *)
+  0x4e699e9e;       (* arm_MUL_VEC Q30 Q20 Q9 16 128 *)
+  0x3dc00851;       (* arm_LDR Q17 X2 (Immediate_Offset (word 32)) *)
+  0x3cc60449;       (* arm_LDR Q9 X2 (Postimmediate_Offset (word 96)) *)
+  0x6e79b665;       (* arm_SQRDMULH_VEC Q5 Q19 Q25 16 128 *)
+  0x6e6086d2;       (* arm_SUB_VEC Q18 Q22 Q0 16 128 *)
+  0x6f4741fe;       (* arm_MLS_VEC Q30 Q15 (Q7 :> LANE_H 0) 16 128 *)
+  0x4e719e7a;       (* arm_MUL_VEC Q26 Q19 Q17 16 128 *)
+  0x6f4740ba;       (* arm_MLS_VEC Q26 Q5 (Q7 :> LANE_H 0) 16 128 *)
+  0x3cdb0045;       (* arm_LDR Q5 X2 (Immediate_Offset (word 18446744073709551536)) *)
+  0x4e699e4e;       (* arm_MUL_VEC Q14 Q18 Q9 16 128 *)
+  0x6e65b65c;       (* arm_SQRDMULH_VEC Q28 Q18 Q5 16 128 *)
+  0x6e7e8751;       (* arm_SUB_VEC Q17 Q26 Q30 16 128 *)
+  0x4e7e8755;       (* arm_ADD_VEC Q21 Q26 Q30 16 128 *)
+  0x4e6086da;       (* arm_ADD_VEC Q26 Q22 Q0 16 128 *)
+  0x6e65b625;       (* arm_SQRDMULH_VEC Q5 Q17 Q5 16 128 *)
+  0x4e956b54;       (* arm_TRN2 Q20 Q26 Q21 32 128 *)
+  0x6f47438e;       (* arm_MLS_VEC Q14 Q28 (Q7 :> LANE_H 0) 16 128 *)
+  0x4e699e31;       (* arm_MUL_VEC Q17 Q17 Q9 16 128 *)
+  0x6f4740b1;       (* arm_MLS_VEC Q17 Q5 (Q7 :> LANE_H 0) 16 128 *)
+  0x4e952b52;       (* arm_TRN1 Q18 Q26 Q21 32 128 *)
+  0x4e9169c5;       (* arm_TRN2 Q5 Q14 Q17 32 128 *)
+  0x4e9129d0;       (* arm_TRN1 Q16 Q14 Q17 32 128 *)
+  0x4ec56a9a;       (* arm_TRN2 Q26 Q20 Q5 64 128 *)
+  0x4ed06a5e;       (* arm_TRN2 Q30 Q18 Q16 64 128 *)
+  0x4ec52a9f;       (* arm_TRN1 Q31 Q20 Q5 64 128 *)
+  0x4e7a87c8;       (* arm_ADD_VEC Q8 Q30 Q26 16 128 *)
+  0x6e7a87d9;       (* arm_SUB_VEC Q25 Q30 Q26 16 128 *)
+  0x4ed02a5a;       (* arm_TRN1 Q26 Q18 Q16 64 128 *)
+  0x4f57c105;       (* arm_SQDMULH_VEC Q5 Q8 (Q7 :> LANE_H 1) 16 128 *)
+  0x6e7f875d;       (* arm_SUB_VEC Q29 Q26 Q31 16 128 *)
+  0x4e7f8756;       (* arm_ADD_VEC Q22 Q26 Q31 16 128 *)
+  0x4f7cd3b4;       (* arm_SQRDMULH_VEC Q20 Q29 (Q12 :> LANE_H 3) 16 128 *)
+  0x4f1524ad;       (* arm_SRSHR_VEC Q13 Q5 11 16 128 *)
+  0x4f57c2df;       (* arm_SQDMULH_VEC Q31 Q22 (Q7 :> LANE_H 1) 16 128 *)
+  0xd1000484;       (* arm_SUB X4 X4 (rvalue (word 1)) *)
+  0x4f5cdb3c;       (* arm_SQRDMULH_VEC Q28 Q25 (Q12 :> LANE_H 5) 16 128 *)
+  0x3dc00c58;       (* arm_LDR Q24 X2 (Immediate_Offset (word 48)) *)
+  0x3dc01863;       (* arm_LDR Q3 X3 (Immediate_Offset (word 96)) *)
+  0x3dc0144f;       (* arm_LDR Q15 X2 (Immediate_Offset (word 80)) *)
+  0x3dc01c77;       (* arm_LDR Q23 X3 (Immediate_Offset (word 112)) *)
+  0x4f4c8b2a;       (* arm_MUL_VEC Q10 Q25 (Q12 :> LANE_H 4) 16 128 *)
+  0x3dc0106e;       (* arm_LDR Q14 X3 (Immediate_Offset (word 64)) *)
+  0x3dc01464;       (* arm_LDR Q4 X3 (Immediate_Offset (word 80)) *)
+  0x6f4741a8;       (* arm_MLS_VEC Q8 Q13 (Q7 :> LANE_H 0) 16 128 *)
+  0x3dc0104d;       (* arm_LDR Q13 X2 (Immediate_Offset (word 64)) *)
+  0x3cc60445;       (* arm_LDR Q5 X2 (Postimmediate_Offset (word 96)) *)
+  0x4f1527f1;       (* arm_SRSHR_VEC Q17 Q31 11 16 128 *)
+  0x4e972860;       (* arm_TRN1 Q0 Q3 Q23 32 128 *)
+  0x4f6c83bb;       (* arm_MUL_VEC Q27 Q29 (Q12 :> LANE_H 2) 16 128 *)
+  0x4e8429de;       (* arm_TRN1 Q30 Q14 Q4 32 128 *)
+  0x4e8469da;       (* arm_TRN2 Q26 Q14 Q4 32 128 *)
+  0x6f47429b;       (* arm_MLS_VEC Q27 Q20 (Q7 :> LANE_H 0) 16 128 *)
+  0x4ec06bd5;       (* arm_TRN2 Q21 Q30 Q0 64 128 *)
+  0x4e97686b;       (* arm_TRN2 Q11 Q3 Q23 32 128 *)
+  0x6f47438a;       (* arm_MLS_VEC Q10 Q28 (Q7 :> LANE_H 0) 16 128 *)
+  0x4ec02bd7;       (* arm_TRN1 Q23 Q30 Q0 64 128 *)
+  0x3cdb0043;       (* arm_LDR Q3 X2 (Immediate_Offset (word 18446744073709551536)) *)
+  0x6f474236;       (* arm_MLS_VEC Q22 Q17 (Q7 :> LANE_H 0) 16 128 *)
+  0x4ecb2b5f;       (* arm_TRN1 Q31 Q26 Q11 64 128 *)
+  0x4ecb6b50;       (* arm_TRN2 Q16 Q26 Q11 64 128 *)
+  0x4e7f86ee;       (* arm_ADD_VEC Q14 Q23 Q31 16 128 *)
+  0x4f57c364;       (* arm_SQDMULH_VEC Q4 Q27 (Q7 :> LANE_H 1) 16 128 *)
+  0x3cdc005a;       (* arm_LDR Q26 X2 (Immediate_Offset (word 18446744073709551552)) *)
+  0x4e7086bc;       (* arm_ADD_VEC Q28 Q21 Q16 16 128 *)
+  0x6e7086b9;       (* arm_SUB_VEC Q25 Q21 Q16 16 128 *)
+  0x4f57c155;       (* arm_SQDMULH_VEC Q21 Q10 (Q7 :> LANE_H 1) 16 128 *)
+  0x6e7c85c1;       (* arm_SUB_VEC Q1 Q14 Q28 16 128 *)
+  0x4e6d9f3d;       (* arm_MUL_VEC Q29 Q25 Q13 16 128 *)
+  0x4e7c85c2;       (* arm_ADD_VEC Q2 Q14 Q28 16 128 *)
+  0x4f152489;       (* arm_SRSHR_VEC Q9 Q4 11 16 128 *)
+  0x6e7f86eb;       (* arm_SUB_VEC Q11 Q23 Q31 16 128 *)
+  0x6e63b433;       (* arm_SQRDMULH_VEC Q19 Q1 Q3 16 128 *)
+  0x4e6886df;       (* arm_ADD_VEC Q31 Q22 Q8 16 128 *)
+  0x6e78b56d;       (* arm_SQRDMULH_VEC Q13 Q11 Q24 16 128 *)
+  0x3c84047f;       (* arm_STR Q31 X3 (Postimmediate_Offset (word 64)) *)
+  0x6e6fb73e;       (* arm_SQRDMULH_VEC Q30 Q25 Q15 16 128 *)
+  0x4e7a9d60;       (* arm_MUL_VEC Q0 Q11 Q26 16 128 *)
+  0x6f4741a0;       (* arm_MLS_VEC Q0 Q13 (Q7 :> LANE_H 0) 16 128 *)
+  0x6e6886cd;       (* arm_SUB_VEC Q13 Q22 Q8 16 128 *)
+  0x4f1526b6;       (* arm_SRSHR_VEC Q22 Q21 11 16 128 *)
+  0x6f4743dd;       (* arm_MLS_VEC Q29 Q30 (Q7 :> LANE_H 0) 16 128 *)
+  0x6f47413b;       (* arm_MLS_VEC Q27 Q9 (Q7 :> LANE_H 0) 16 128 *)
+  0x6f4742ca;       (* arm_MLS_VEC Q10 Q22 (Q7 :> LANE_H 0) 16 128 *)
+  0x4e659c29;       (* arm_MUL_VEC Q9 Q1 Q5 16 128 *)
+  0x6e7d841c;       (* arm_SUB_VEC Q28 Q0 Q29 16 128 *)
+  0x6e63b788;       (* arm_SQRDMULH_VEC Q8 Q28 Q3 16 128 *)
+  0x4e6a877a;       (* arm_ADD_VEC Q26 Q27 Q10 16 128 *)
+  0x4e659f94;       (* arm_MUL_VEC Q20 Q28 Q5 16 128 *)
+  0x6e6a8771;       (* arm_SUB_VEC Q17 Q27 Q10 16 128 *)
+  0x4e7d840a;       (* arm_ADD_VEC Q10 Q0 Q29 16 128 *)
+  0x3c9d007a;       (* arm_STR Q26 X3 (Immediate_Offset (word 18446744073709551568)) *)
+  0x6f474269;       (* arm_MLS_VEC Q9 Q19 (Q7 :> LANE_H 0) 16 128 *)
+  0x6f474114;       (* arm_MLS_VEC Q20 Q8 (Q7 :> LANE_H 0) 16 128 *)
+  0x4e8a6859;       (* arm_TRN2 Q25 Q2 Q10 32 128 *)
+  0x4e8a2848;       (* arm_TRN1 Q8 Q2 Q10 32 128 *)
+  0x4f5cd1a4;       (* arm_SQRDMULH_VEC Q4 Q13 (Q12 :> LANE_H 1) 16 128 *)
+  0x4f4c81a0;       (* arm_MUL_VEC Q0 Q13 (Q12 :> LANE_H 0) 16 128 *)
+  0x4e94292a;       (* arm_TRN1 Q10 Q9 Q20 32 128 *)
+  0x4e94693a;       (* arm_TRN2 Q26 Q9 Q20 32 128 *)
+  0x4f5cd22e;       (* arm_SQRDMULH_VEC Q14 Q17 (Q12 :> LANE_H 1) 16 128 *)
+  0x4eca690b;       (* arm_TRN2 Q11 Q8 Q10 64 128 *)
+  0x4f4c8222;       (* arm_MUL_VEC Q2 Q17 (Q12 :> LANE_H 0) 16 128 *)
+  0x4eda2b3c;       (* arm_TRN1 Q28 Q25 Q26 64 128 *)
+  0x3cc1042c;       (* arm_LDR Q12 X1 (Postimmediate_Offset (word 16)) *)
+  0x4eda6b39;       (* arm_TRN2 Q25 Q25 Q26 64 128 *)
+  0x4eca290a;       (* arm_TRN1 Q10 Q8 Q10 64 128 *)
+  0x6f474080;       (* arm_MLS_VEC Q0 Q4 (Q7 :> LANE_H 0) 16 128 *)
+  0x4e798568;       (* arm_ADD_VEC Q8 Q11 Q25 16 128 *)
+  0x6f4741c2;       (* arm_MLS_VEC Q2 Q14 (Q7 :> LANE_H 0) 16 128 *)
+  0x6e798579;       (* arm_SUB_VEC Q25 Q11 Q25 16 128 *)
+  0x6e7c855d;       (* arm_SUB_VEC Q29 Q10 Q28 16 128 *)
+  0x4e7c8556;       (* arm_ADD_VEC Q22 Q10 Q28 16 128 *)
+  0x4f57c110;       (* arm_SQDMULH_VEC Q16 Q8 (Q7 :> LANE_H 1) 16 128 *)
+  0x3c9e0060;       (* arm_STR Q0 X3 (Immediate_Offset (word 18446744073709551584)) *)
+  0x4f7cd3b4;       (* arm_SQRDMULH_VEC Q20 Q29 (Q12 :> LANE_H 3) 16 128 *)
+  0x3c9f0062;       (* arm_STR Q2 X3 (Immediate_Offset (word 18446744073709551600)) *)
+  0x4f57c2df;       (* arm_SQDMULH_VEC Q31 Q22 (Q7 :> LANE_H 1) 16 128 *)
+  0x4f15260d;       (* arm_SRSHR_VEC Q13 Q16 11 16 128 *)
   0xd1000484;       (* arm_SUB X4 X4 (rvalue (word 1)) *)
   0xb5fff584;       (* arm_CBNZ X4 (word 2096816) *)
-  0x6f474295;       (* arm_MLS_VEC Q21 Q20 (Q7 :> LANE_H 0) 16 128 *)
-  0x6e72853b;       (* arm_SUB_VEC Q27 Q9 Q18 16 128 *)
-  0x4e72853e;       (* arm_ADD_VEC Q30 Q9 Q18 16 128 *)
-  0x4f7fd36a;       (* arm_SQRDMULH_VEC Q10 Q27 (Q15 :> LANE_H 3) 16 128 *)
-  0x4f6f837c;       (* arm_MUL_VEC Q28 Q27 (Q15 :> LANE_H 2) 16 128 *)
-  0x4f57c1db;       (* arm_SQDMULH_VEC Q27 Q14 (Q7 :> LANE_H 1) 16 128 *)
-  0x6f47415c;       (* arm_MLS_VEC Q28 Q10 (Q7 :> LANE_H 0) 16 128 *)
-  0x4f57c3ca;       (* arm_SQDMULH_VEC Q10 Q30 (Q7 :> LANE_H 1) 16 128 *)
-  0x4f15277b;       (* arm_SRSHR_VEC Q27 Q27 11 16 128 *)
-  0x4f57c2ad;       (* arm_SQDMULH_VEC Q13 Q21 (Q7 :> LANE_H 1) 16 128 *)
-  0x4f57c396;       (* arm_SQDMULH_VEC Q22 Q28 (Q7 :> LANE_H 1) 16 128 *)
-  0x4f152559;       (* arm_SRSHR_VEC Q25 Q10 11 16 128 *)
-  0x4f1525b8;       (* arm_SRSHR_VEC Q24 Q13 11 16 128 *)
-  0x6f47436e;       (* arm_MLS_VEC Q14 Q27 (Q7 :> LANE_H 0) 16 128 *)
-  0x6f47433e;       (* arm_MLS_VEC Q30 Q25 (Q7 :> LANE_H 0) 16 128 *)
-  0x4f1526c2;       (* arm_SRSHR_VEC Q2 Q22 11 16 128 *)
-  0x6f474315;       (* arm_MLS_VEC Q21 Q24 (Q7 :> LANE_H 0) 16 128 *)
-  0x6f47405c;       (* arm_MLS_VEC Q28 Q2 (Q7 :> LANE_H 0) 16 128 *)
-  0x6e6e87d9;       (* arm_SUB_VEC Q25 Q30 Q14 16 128 *)
-  0x4e6e87db;       (* arm_ADD_VEC Q27 Q30 Q14 16 128 *)
-  0x4f5fd323;       (* arm_SQRDMULH_VEC Q3 Q25 (Q15 :> LANE_H 1) 16 128 *)
-  0x3c84047b;       (* arm_STR Q27 X3 (Postimmediate_Offset (word 64)) *)
-  0x6e75879b;       (* arm_SUB_VEC Q27 Q28 Q21 16 128 *)
-  0x4f4f832d;       (* arm_MUL_VEC Q13 Q25 (Q15 :> LANE_H 0) 16 128 *)
-  0x4e758782;       (* arm_ADD_VEC Q2 Q28 Q21 16 128 *)
-  0x4f5fd37f;       (* arm_SQRDMULH_VEC Q31 Q27 (Q15 :> LANE_H 1) 16 128 *)
-  0x4f4f837b;       (* arm_MUL_VEC Q27 Q27 (Q15 :> LANE_H 0) 16 128 *)
-  0x6f47406d;       (* arm_MLS_VEC Q13 Q3 (Q7 :> LANE_H 0) 16 128 *)
-  0x6f4743fb;       (* arm_MLS_VEC Q27 Q31 (Q7 :> LANE_H 0) 16 128 *)
-  0x3c9d0062;       (* arm_STR Q2 X3 (Immediate_Offset (word 18446744073709551568)) *)
-  0x3c9e006d;       (* arm_STR Q13 X3 (Immediate_Offset (word 18446744073709551584)) *)
-  0x3c9f007b;       (* arm_STR Q27 X3 (Immediate_Offset (word 18446744073709551600)) *)
+  0x4f1527e6;       (* arm_SRSHR_VEC Q6 Q31 11 16 128 *)
+  0x4f5cdb2b;       (* arm_SQRDMULH_VEC Q11 Q25 (Q12 :> LANE_H 5) 16 128 *)
+  0x4f4c8b32;       (* arm_MUL_VEC Q18 Q25 (Q12 :> LANE_H 4) 16 128 *)
+  0x4f6c83a5;       (* arm_MUL_VEC Q5 Q29 (Q12 :> LANE_H 2) 16 128 *)
+  0x6f474172;       (* arm_MLS_VEC Q18 Q11 (Q7 :> LANE_H 0) 16 128 *)
+  0x6f474285;       (* arm_MLS_VEC Q5 Q20 (Q7 :> LANE_H 0) 16 128 *)
+  0x4f57c249;       (* arm_SQDMULH_VEC Q9 Q18 (Q7 :> LANE_H 1) 16 128 *)
+  0x4f57c0a0;       (* arm_SQDMULH_VEC Q0 Q5 (Q7 :> LANE_H 1) 16 128 *)
+  0x6f4740d6;       (* arm_MLS_VEC Q22 Q6 (Q7 :> LANE_H 0) 16 128 *)
+  0x4f152539;       (* arm_SRSHR_VEC Q25 Q9 11 16 128 *)
+  0x6f4741a8;       (* arm_MLS_VEC Q8 Q13 (Q7 :> LANE_H 0) 16 128 *)
+  0x4f152414;       (* arm_SRSHR_VEC Q20 Q0 11 16 128 *)
+  0x6f474332;       (* arm_MLS_VEC Q18 Q25 (Q7 :> LANE_H 0) 16 128 *)
+  0x6f474285;       (* arm_MLS_VEC Q5 Q20 (Q7 :> LANE_H 0) 16 128 *)
+  0x6e6886c2;       (* arm_SUB_VEC Q2 Q22 Q8 16 128 *)
+  0x4e6886dd;       (* arm_ADD_VEC Q29 Q22 Q8 16 128 *)
+  0x4f5cd05a;       (* arm_SQRDMULH_VEC Q26 Q2 (Q12 :> LANE_H 1) 16 128 *)
+  0x3c84047d;       (* arm_STR Q29 X3 (Postimmediate_Offset (word 64)) *)
+  0x4f4c8043;       (* arm_MUL_VEC Q3 Q2 (Q12 :> LANE_H 0) 16 128 *)
+  0x6e7284a1;       (* arm_SUB_VEC Q1 Q5 Q18 16 128 *)
+  0x4f5cd034;       (* arm_SQRDMULH_VEC Q20 Q1 (Q12 :> LANE_H 1) 16 128 *)
+  0x4f4c802f;       (* arm_MUL_VEC Q15 Q1 (Q12 :> LANE_H 0) 16 128 *)
+  0x6f474343;       (* arm_MLS_VEC Q3 Q26 (Q7 :> LANE_H 0) 16 128 *)
+  0x6f47428f;       (* arm_MLS_VEC Q15 Q20 (Q7 :> LANE_H 0) 16 128 *)
+  0x4e7284b8;       (* arm_ADD_VEC Q24 Q5 Q18 16 128 *)
+  0x3c9e0063;       (* arm_STR Q3 X3 (Immediate_Offset (word 18446744073709551584)) *)
+  0x3c9d0078;       (* arm_STR Q24 X3 (Immediate_Offset (word 18446744073709551568)) *)
+  0x3c9f006f;       (* arm_STR Q15 X3 (Immediate_Offset (word 18446744073709551600)) *)
   0xd2800084;       (* arm_MOV X4 (rvalue (word 4)) *)
   0x3cc20420;       (* arm_LDR Q0 X1 (Postimmediate_Offset (word 32)) *)
   0x3cdf0021;       (* arm_LDR Q1 X1 (Immediate_Offset (word 18446744073709551600)) *)
-  0x3dc0700d;       (* arm_LDR Q13 X0 (Immediate_Offset (word 448)) *)
-  0x3dc06002;       (* arm_LDR Q2 X0 (Immediate_Offset (word 384)) *)
-  0x3dc03008;       (* arm_LDR Q8 X0 (Immediate_Offset (word 192)) *)
-  0x3dc0400c;       (* arm_LDR Q12 X0 (Immediate_Offset (word 256)) *)
-  0x3dc01017;       (* arm_LDR Q23 X0 (Immediate_Offset (word 64)) *)
-  0x6e6d845a;       (* arm_SUB_VEC Q26 Q2 Q13 16 128 *)
-  0x3dc0501b;       (* arm_LDR Q27 X0 (Immediate_Offset (word 320)) *)
-  0x4e6d844d;       (* arm_ADD_VEC Q13 Q2 Q13 16 128 *)
-  0x3dc00014;       (* arm_LDR Q20 X0 (Immediate_Offset (word 0)) *)
-  0x4f51db5c;       (* arm_SQRDMULH_VEC Q28 Q26 (Q1 :> LANE_H 5) 16 128 *)
-  0x3dc0200e;       (* arm_LDR Q14 X0 (Immediate_Offset (word 128)) *)
-  0x4f418b52;       (* arm_MUL_VEC Q18 Q26 (Q1 :> LANE_H 4) 16 128 *)
-  0x6e7b8582;       (* arm_SUB_VEC Q2 Q12 Q27 16 128 *)
-  0x4e778683;       (* arm_ADD_VEC Q3 Q20 Q23 16 128 *)
-  0x4e6885da;       (* arm_ADD_VEC Q26 Q14 Q8 16 128 *)
-  0x4f71d05f;       (* arm_SQRDMULH_VEC Q31 Q2 (Q1 :> LANE_H 3) 16 128 *)
-  0x6e7a846b;       (* arm_SUB_VEC Q11 Q3 Q26 16 128 *)
-  0x6f474392;       (* arm_MLS_VEC Q18 Q28 (Q7 :> LANE_H 0) 16 128 *)
-  0x4f61805d;       (* arm_MUL_VEC Q29 Q2 (Q1 :> LANE_H 2) 16 128 *)
-  0x6f4743fd;       (* arm_MLS_VEC Q29 Q31 (Q7 :> LANE_H 0) 16 128 *)
-  0x4f608176;       (* arm_MUL_VEC Q22 Q11 (Q0 :> LANE_H 2) 16 128 *)
-  0x6e7287bf;       (* arm_SUB_VEC Q31 Q29 Q18 16 128 *)
-  0x4f50dbfc;       (* arm_SQRDMULH_VEC Q28 Q31 (Q0 :> LANE_H 5) 16 128 *)
-  0x4f408be4;       (* arm_MUL_VEC Q4 Q31 (Q0 :> LANE_H 4) 16 128 *)
-  0xd1000484;       (* arm_SUB X4 X4 (rvalue (word 1)) *)
-  0x4f70d16f;       (* arm_SQRDMULH_VEC Q15 Q11 (Q0 :> LANE_H 3) 16 128 *)
-  0x6e77869f;       (* arm_SUB_VEC Q31 Q20 Q23 16 128 *)
-  0x6e6885c2;       (* arm_SUB_VEC Q2 Q14 Q8 16 128 *)
-  0x4f608be9;       (* arm_MUL_VEC Q9 Q31 (Q0 :> LANE_H 6) 16 128 *)
-  0x3dc06418;       (* arm_LDR Q24 X0 (Immediate_Offset (word 400)) *)
-  0x4e7b859e;       (* arm_ADD_VEC Q30 Q12 Q27 16 128 *)
-  0x3dc07411;       (* arm_LDR Q17 X0 (Immediate_Offset (word 464)) *)
-  0x4f51d04b;       (* arm_SQRDMULH_VEC Q11 Q2 (Q1 :> LANE_H 1) 16 128 *)
-  0x4e6d87c6;       (* arm_ADD_VEC Q6 Q30 Q13 16 128 *)
-  0x4e7a8479;       (* arm_ADD_VEC Q25 Q3 Q26 16 128 *)
-  0x4f70dbfb;       (* arm_SQRDMULH_VEC Q27 Q31 (Q0 :> LANE_H 7) 16 128 *)
-  0x3dc03408;       (* arm_LDR Q8 X0 (Immediate_Offset (word 208)) *)
-  0x6e71870e;       (* arm_SUB_VEC Q14 Q24 Q17 16 128 *)
-  0x4f418043;       (* arm_MUL_VEC Q3 Q2 (Q1 :> LANE_H 0) 16 128 *)
-  0x6f474163;       (* arm_MLS_VEC Q3 Q11 (Q7 :> LANE_H 0) 16 128 *)
-  0x6e668730;       (* arm_SUB_VEC Q16 Q25 Q6 16 128 *)
-  0x6e6d87da;       (* arm_SUB_VEC Q26 Q30 Q13 16 128 *)
-  0x6f474369;       (* arm_MLS_VEC Q9 Q27 (Q7 :> LANE_H 0) 16 128 *)
-  0x3dc0541b;       (* arm_LDR Q27 X0 (Immediate_Offset (word 336)) *)
-  0x4f40821e;       (* arm_MUL_VEC Q30 Q16 (Q0 :> LANE_H 0) 16 128 *)
+  0x3dc0601c;       (* arm_LDR Q28 X0 (Immediate_Offset (word 384)) *)
+  0x3dc0701a;       (* arm_LDR Q26 X0 (Immediate_Offset (word 448)) *)
+  0x3dc05003;       (* arm_LDR Q3 X0 (Immediate_Offset (word 320)) *)
+  0x3dc0400d;       (* arm_LDR Q13 X0 (Immediate_Offset (word 256)) *)
+  0x6e7a8795;       (* arm_SUB_VEC Q21 Q28 Q26 16 128 *)
+  0x4e7a8794;       (* arm_ADD_VEC Q20 Q28 Q26 16 128 *)
+  0x6e6385ba;       (* arm_SUB_VEC Q26 Q13 Q3 16 128 *)
+  0x4e6385a5;       (* arm_ADD_VEC Q5 Q13 Q3 16 128 *)
+  0x4f51dabc;       (* arm_SQRDMULH_VEC Q28 Q21 (Q1 :> LANE_H 5) 16 128 *)
+  0x6e7484a2;       (* arm_SUB_VEC Q2 Q5 Q20 16 128 *)
+  0x4f61834b;       (* arm_MUL_VEC Q11 Q26 (Q1 :> LANE_H 2) 16 128 *)
+  0x4f71d35a;       (* arm_SQRDMULH_VEC Q26 Q26 (Q1 :> LANE_H 3) 16 128 *)
+  0x4f418aa4;       (* arm_MUL_VEC Q4 Q21 (Q1 :> LANE_H 4) 16 128 *)
   0x6f474384;       (* arm_MLS_VEC Q4 Q28 (Q7 :> LANE_H 0) 16 128 *)
-  0x4e7287bc;       (* arm_ADD_VEC Q28 Q29 Q18 16 128 *)
-  0x4e638533;       (* arm_ADD_VEC Q19 Q9 Q3 16 128 *)
-  0x6e638523;       (* arm_SUB_VEC Q3 Q9 Q3 16 128 *)
-  0x4f50d20d;       (* arm_SQRDMULH_VEC Q13 Q16 (Q0 :> LANE_H 1) 16 128 *)
-  0x6e7c8677;       (* arm_SUB_VEC Q23 Q19 Q28 16 128 *)
-  0x4e7c8670;       (* arm_ADD_VEC Q16 Q19 Q28 16 128 *)
-  0x4f70d06c;       (* arm_SQRDMULH_VEC Q12 Q3 (Q0 :> LANE_H 3) 16 128 *)
-  0x4f60806a;       (* arm_MUL_VEC Q10 Q3 (Q0 :> LANE_H 2) 16 128 *)
-  0x3d801010;       (* arm_STR Q16 X0 (Immediate_Offset (word 64)) *)
-  0x6f4741be;       (* arm_MLS_VEC Q30 Q13 (Q7 :> LANE_H 0) 16 128 *)
-  0x6f47418a;       (* arm_MLS_VEC Q10 Q12 (Q7 :> LANE_H 0) 16 128 *)
-  0x3dc0440c;       (* arm_LDR Q12 X0 (Immediate_Offset (word 272)) *)
-  0x6f4741f6;       (* arm_MLS_VEC Q22 Q15 (Q7 :> LANE_H 0) 16 128 *)
-  0x3d80401e;       (* arm_STR Q30 X0 (Immediate_Offset (word 256)) *)
-  0x4f51d9c2;       (* arm_SQRDMULH_VEC Q2 Q14 (Q1 :> LANE_H 5) 16 128 *)
-  0x6e7b858f;       (* arm_SUB_VEC Q15 Q12 Q27 16 128 *)
-  0x4e66873e;       (* arm_ADD_VEC Q30 Q25 Q6 16 128 *)
-  0x4e648559;       (* arm_ADD_VEC Q25 Q10 Q4 16 128 *)
-  0x4f50db49;       (* arm_SQRDMULH_VEC Q9 Q26 (Q0 :> LANE_H 5) 16 128 *)
-  0x6e64854d;       (* arm_SUB_VEC Q13 Q10 Q4 16 128 *)
-  0x3d803019;       (* arm_STR Q25 X0 (Immediate_Offset (word 192)) *)
-  0x4f4189d2;       (* arm_MUL_VEC Q18 Q14 (Q1 :> LANE_H 4) 16 128 *)
-  0x4f4082ff;       (* arm_MUL_VEC Q31 Q23 (Q0 :> LANE_H 0) 16 128 *)
-  0x4f50d2ea;       (* arm_SQRDMULH_VEC Q10 Q23 (Q0 :> LANE_H 1) 16 128 *)
-  0x3dc01417;       (* arm_LDR Q23 X0 (Immediate_Offset (word 80)) *)
-  0x4f50d1b4;       (* arm_SQRDMULH_VEC Q20 Q13 (Q0 :> LANE_H 1) 16 128 *)
-  0x6f474052;       (* arm_MLS_VEC Q18 Q2 (Q7 :> LANE_H 0) 16 128 *)
-  0x4f408b45;       (* arm_MUL_VEC Q5 Q26 (Q0 :> LANE_H 4) 16 128 *)
-  0x4f4081ae;       (* arm_MUL_VEC Q14 Q13 (Q0 :> LANE_H 0) 16 128 *)
-  0x6f47428e;       (* arm_MLS_VEC Q14 Q20 (Q7 :> LANE_H 0) 16 128 *)
-  0x6f474125;       (* arm_MLS_VEC Q5 Q9 (Q7 :> LANE_H 0) 16 128 *)
-  0x4f71d1e9;       (* arm_SQRDMULH_VEC Q9 Q15 (Q1 :> LANE_H 3) 16 128 *)
-  0x3dc00414;       (* arm_LDR Q20 X0 (Immediate_Offset (word 16)) *)
-  0x6f47415f;       (* arm_MLS_VEC Q31 Q10 (Q7 :> LANE_H 0) 16 128 *)
-  0x3d80700e;       (* arm_STR Q14 X0 (Immediate_Offset (word 448)) *)
-  0x3dc0240e;       (* arm_LDR Q14 X0 (Immediate_Offset (word 144)) *)
-  0x6e6586ca;       (* arm_SUB_VEC Q10 Q22 Q5 16 128 *)
-  0x4f6181fd;       (* arm_MUL_VEC Q29 Q15 (Q1 :> LANE_H 2) 16 128 *)
-  0x4e6586cd;       (* arm_ADD_VEC Q13 Q22 Q5 16 128 *)
-  0x3c81041e;       (* arm_STR Q30 X0 (Postimmediate_Offset (word 16)) *)
-  0x6f47413d;       (* arm_MLS_VEC Q29 Q9 (Q7 :> LANE_H 0) 16 128 *)
-  0x3d801c0d;       (* arm_STR Q13 X0 (Immediate_Offset (word 112)) *)
-  0x3d804c1f;       (* arm_STR Q31 X0 (Immediate_Offset (word 304)) *)
-  0x4e6885da;       (* arm_ADD_VEC Q26 Q14 Q8 16 128 *)
-  0x4e778683;       (* arm_ADD_VEC Q3 Q20 Q23 16 128 *)
-  0x4f50d15c;       (* arm_SQRDMULH_VEC Q28 Q10 (Q0 :> LANE_H 1) 16 128 *)
-  0x4f408155;       (* arm_MUL_VEC Q21 Q10 (Q0 :> LANE_H 0) 16 128 *)
-  0x6e7a846b;       (* arm_SUB_VEC Q11 Q3 Q26 16 128 *)
-  0x6e7287ad;       (* arm_SUB_VEC Q13 Q29 Q18 16 128 *)
-  0x4f608176;       (* arm_MUL_VEC Q22 Q11 (Q0 :> LANE_H 2) 16 128 *)
-  0x6f474395;       (* arm_MLS_VEC Q21 Q28 (Q7 :> LANE_H 0) 16 128 *)
-  0x4f50d9bc;       (* arm_SQRDMULH_VEC Q28 Q13 (Q0 :> LANE_H 5) 16 128 *)
-  0x4f4089a4;       (* arm_MUL_VEC Q4 Q13 (Q0 :> LANE_H 4) 16 128 *)
-  0x4e71870d;       (* arm_ADD_VEC Q13 Q24 Q17 16 128 *)
-  0x3d805c15;       (* arm_STR Q21 X0 (Immediate_Offset (word 368)) *)
+  0x6f47434b;       (* arm_MLS_VEC Q11 Q26 (Q7 :> LANE_H 0) 16 128 *)
+  0x4f50d85c;       (* arm_SQRDMULH_VEC Q28 Q2 (Q0 :> LANE_H 5) 16 128 *)
+  0x6e648578;       (* arm_SUB_VEC Q24 Q11 Q4 16 128 *)
+  0x4f408b06;       (* arm_MUL_VEC Q6 Q24 (Q0 :> LANE_H 4) 16 128 *)
+  0xd1000484;       (* arm_SUB X4 X4 (rvalue (word 1)) *)
+  0x4f50db18;       (* arm_SQRDMULH_VEC Q24 Q24 (Q0 :> LANE_H 5) 16 128 *)
+  0x3dc0201d;       (* arm_LDR Q29 X0 (Immediate_Offset (word 128)) *)
+  0x3dc03009;       (* arm_LDR Q9 X0 (Immediate_Offset (word 192)) *)
+  0x3dc00013;       (* arm_LDR Q19 X0 (Immediate_Offset (word 0)) *)
+  0x3dc01012;       (* arm_LDR Q18 X0 (Immediate_Offset (word 64)) *)
+  0x4f408843;       (* arm_MUL_VEC Q3 Q2 (Q0 :> LANE_H 4) 16 128 *)
+  0x4e7484b1;       (* arm_ADD_VEC Q17 Q5 Q20 16 128 *)
+  0x6f474383;       (* arm_MLS_VEC Q3 Q28 (Q7 :> LANE_H 0) 16 128 *)
+  0x4e6987a2;       (* arm_ADD_VEC Q2 Q29 Q9 16 128 *)
+  0x6f474306;       (* arm_MLS_VEC Q6 Q24 (Q7 :> LANE_H 0) 16 128 *)
+  0x6e728674;       (* arm_SUB_VEC Q20 Q19 Q18 16 128 *)
+  0x4e728679;       (* arm_ADD_VEC Q25 Q19 Q18 16 128 *)
+  0x6e6987b8;       (* arm_SUB_VEC Q24 Q29 Q9 16 128 *)
+  0x4f608a8a;       (* arm_MUL_VEC Q10 Q20 (Q0 :> LANE_H 6) 16 128 *)
+  0x6e62873b;       (* arm_SUB_VEC Q27 Q25 Q2 16 128 *)
+  0x4e62872c;       (* arm_ADD_VEC Q12 Q25 Q2 16 128 *)
+  0x4f70da93;       (* arm_SQRDMULH_VEC Q19 Q20 (Q0 :> LANE_H 7) 16 128 *)
+  0x4e648575;       (* arm_ADD_VEC Q21 Q11 Q4 16 128 *)
+  0x4f41830f;       (* arm_MUL_VEC Q15 Q24 (Q1 :> LANE_H 0) 16 128 *)
+  0x6e718582;       (* arm_SUB_VEC Q2 Q12 Q17 16 128 *)
+  0x4e718590;       (* arm_ADD_VEC Q16 Q12 Q17 16 128 *)
+  0x4f608379;       (* arm_MUL_VEC Q25 Q27 (Q0 :> LANE_H 2) 16 128 *)
+  0x4f51d318;       (* arm_SQRDMULH_VEC Q24 Q24 (Q1 :> LANE_H 1) 16 128 *)
+  0x6f47426a;       (* arm_MLS_VEC Q10 Q19 (Q7 :> LANE_H 0) 16 128 *)
+  0x4f50d045;       (* arm_SQRDMULH_VEC Q5 Q2 (Q0 :> LANE_H 1) 16 128 *)
+  0x6f47430f;       (* arm_MLS_VEC Q15 Q24 (Q7 :> LANE_H 0) 16 128 *)
+  0x3dc07418;       (* arm_LDR Q24 X0 (Immediate_Offset (word 464)) *)
+  0x4f408044;       (* arm_MUL_VEC Q4 Q2 (Q0 :> LANE_H 0) 16 128 *)
+  0x6f4740a4;       (* arm_MLS_VEC Q4 Q5 (Q7 :> LANE_H 0) 16 128 *)
+  0x6e6f855c;       (* arm_SUB_VEC Q28 Q10 Q15 16 128 *)
+  0x4f70d377;       (* arm_SQRDMULH_VEC Q23 Q27 (Q0 :> LANE_H 3) 16 128 *)
+  0x4e6f855f;       (* arm_ADD_VEC Q31 Q10 Q15 16 128 *)
+  0x6e7587f2;       (* arm_SUB_VEC Q18 Q31 Q21 16 128 *)
+  0x4f60838a;       (* arm_MUL_VEC Q10 Q28 (Q0 :> LANE_H 2) 16 128 *)
+  0x3d804004;       (* arm_STR Q4 X0 (Immediate_Offset (word 256)) *)
+  0x3dc0640d;       (* arm_LDR Q13 X0 (Immediate_Offset (word 400)) *)
+  0x4f50d24c;       (* arm_SQRDMULH_VEC Q12 Q18 (Q0 :> LANE_H 1) 16 128 *)
+  0x3dc04411;       (* arm_LDR Q17 X0 (Immediate_Offset (word 272)) *)
+  0x4e7587e9;       (* arm_ADD_VEC Q9 Q31 Q21 16 128 *)
+  0x4f70d395;       (* arm_SQRDMULH_VEC Q21 Q28 (Q0 :> LANE_H 3) 16 128 *)
+  0x3dc05404;       (* arm_LDR Q4 X0 (Immediate_Offset (word 336)) *)
+  0x6f4742f9;       (* arm_MLS_VEC Q25 Q23 (Q7 :> LANE_H 0) 16 128 *)
+  0x6e7885a8;       (* arm_SUB_VEC Q8 Q13 Q24 16 128 *)
+  0x4f51d913;       (* arm_SQRDMULH_VEC Q19 Q8 (Q1 :> LANE_H 5) 16 128 *)
+  0x6e64862e;       (* arm_SUB_VEC Q14 Q17 Q4 16 128 *)
+  0x6f4742aa;       (* arm_MLS_VEC Q10 Q21 (Q7 :> LANE_H 0) 16 128 *)
+  0x4e638737;       (* arm_ADD_VEC Q23 Q25 Q3 16 128 *)
+  0x6e63873f;       (* arm_SUB_VEC Q31 Q25 Q3 16 128 *)
+  0x4f6181cb;       (* arm_MUL_VEC Q11 Q14 (Q1 :> LANE_H 2) 16 128 *)
+  0x4f50d3fb;       (* arm_SQRDMULH_VEC Q27 Q31 (Q0 :> LANE_H 1) 16 128 *)
+  0x6e668542;       (* arm_SUB_VEC Q2 Q10 Q6 16 128 *)
+  0x4e648625;       (* arm_ADD_VEC Q5 Q17 Q4 16 128 *)
+  0x4f4083fd;       (* arm_MUL_VEC Q29 Q31 (Q0 :> LANE_H 0) 16 128 *)
+  0x4e7885b4;       (* arm_ADD_VEC Q20 Q13 Q24 16 128 *)
+  0x4e668555;       (* arm_ADD_VEC Q21 Q10 Q6 16 128 *)
+  0x4f50d044;       (* arm_SQRDMULH_VEC Q4 Q2 (Q0 :> LANE_H 1) 16 128 *)
+  0x4f408043;       (* arm_MUL_VEC Q3 Q2 (Q0 :> LANE_H 0) 16 128 *)
+  0x6e7484a2;       (* arm_SUB_VEC Q2 Q5 Q20 16 128 *)
+  0x4f71d1d8;       (* arm_SQRDMULH_VEC Q24 Q14 (Q1 :> LANE_H 3) 16 128 *)
+  0x6f474083;       (* arm_MLS_VEC Q3 Q4 (Q7 :> LANE_H 0) 16 128 *)
+  0x4f418904;       (* arm_MUL_VEC Q4 Q8 (Q1 :> LANE_H 4) 16 128 *)
+  0x6f47430b;       (* arm_MLS_VEC Q11 Q24 (Q7 :> LANE_H 0) 16 128 *)
+  0x6f47437d;       (* arm_MLS_VEC Q29 Q27 (Q7 :> LANE_H 0) 16 128 *)
+  0x6f474264;       (* arm_MLS_VEC Q4 Q19 (Q7 :> LANE_H 0) 16 128 *)
+  0x4f408251;       (* arm_MUL_VEC Q17 Q18 (Q0 :> LANE_H 0) 16 128 *)
+  0x3d80601d;       (* arm_STR Q29 X0 (Immediate_Offset (word 384)) *)
+  0x6f474191;       (* arm_MLS_VEC Q17 Q12 (Q7 :> LANE_H 0) 16 128 *)
+  0x3d807003;       (* arm_STR Q3 X0 (Immediate_Offset (word 448)) *)
+  0x3c810410;       (* arm_STR Q16 X0 (Postimmediate_Offset (word 16)) *)
+  0x6e648578;       (* arm_SUB_VEC Q24 Q11 Q4 16 128 *)
+  0x3d800c09;       (* arm_STR Q9 X0 (Immediate_Offset (word 48)) *)
+  0x4f50d85c;       (* arm_SQRDMULH_VEC Q28 Q2 (Q0 :> LANE_H 5) 16 128 *)
+  0x3d801c17;       (* arm_STR Q23 X0 (Immediate_Offset (word 112)) *)
+  0x3d802c15;       (* arm_STR Q21 X0 (Immediate_Offset (word 176)) *)
+  0x4f408b06;       (* arm_MUL_VEC Q6 Q24 (Q0 :> LANE_H 4) 16 128 *)
+  0x3d804c11;       (* arm_STR Q17 X0 (Immediate_Offset (word 304)) *)
   0xd1000484;       (* arm_SUB X4 X4 (rvalue (word 1)) *)
   0xb5fff664;       (* arm_CBNZ X4 (word 2096844) *)
-  0x4f70d162;       (* arm_SQRDMULH_VEC Q2 Q11 (Q0 :> LANE_H 3) 16 128 *)
-  0x6e778689;       (* arm_SUB_VEC Q9 Q20 Q23 16 128 *)
-  0x6e6885d1;       (* arm_SUB_VEC Q17 Q14 Q8 16 128 *)
-  0x4e7b859b;       (* arm_ADD_VEC Q27 Q12 Q27 16 128 *)
-  0x6f474384;       (* arm_MLS_VEC Q4 Q28 (Q7 :> LANE_H 0) 16 128 *)
-  0x4e7a847c;       (* arm_ADD_VEC Q28 Q3 Q26 16 128 *)
-  0x4e7287ae;       (* arm_ADD_VEC Q14 Q29 Q18 16 128 *)
-  0x4f608937;       (* arm_MUL_VEC Q23 Q9 (Q0 :> LANE_H 6) 16 128 *)
-  0x4e6d8778;       (* arm_ADD_VEC Q24 Q27 Q13 16 128 *)
-  0x6e6d877b;       (* arm_SUB_VEC Q27 Q27 Q13 16 128 *)
-  0x6f474056;       (* arm_MLS_VEC Q22 Q2 (Q7 :> LANE_H 0) 16 128 *)
-  0x6e78878d;       (* arm_SUB_VEC Q13 Q28 Q24 16 128 *)
-  0x4f70d922;       (* arm_SQRDMULH_VEC Q2 Q9 (Q0 :> LANE_H 7) 16 128 *)
-  0x4e78879c;       (* arm_ADD_VEC Q28 Q28 Q24 16 128 *)
-  0x3c81041c;       (* arm_STR Q28 X0 (Postimmediate_Offset (word 16)) *)
-  0x4f51d23c;       (* arm_SQRDMULH_VEC Q28 Q17 (Q1 :> LANE_H 1) 16 128 *)
-  0x4f418229;       (* arm_MUL_VEC Q9 Q17 (Q1 :> LANE_H 0) 16 128 *)
-  0x4f4081b1;       (* arm_MUL_VEC Q17 Q13 (Q0 :> LANE_H 0) 16 128 *)
-  0x6f474389;       (* arm_MLS_VEC Q9 Q28 (Q7 :> LANE_H 0) 16 128 *)
-  0x6f474057;       (* arm_MLS_VEC Q23 Q2 (Q7 :> LANE_H 0) 16 128 *)
-  0x4f50d1ad;       (* arm_SQRDMULH_VEC Q13 Q13 (Q0 :> LANE_H 1) 16 128 *)
-  0x4f50db62;       (* arm_SQRDMULH_VEC Q2 Q27 (Q0 :> LANE_H 5) 16 128 *)
-  0x4e6986fc;       (* arm_ADD_VEC Q28 Q23 Q9 16 128 *)
-  0x4f408b7b;       (* arm_MUL_VEC Q27 Q27 (Q0 :> LANE_H 4) 16 128 *)
-  0x6e6986e9;       (* arm_SUB_VEC Q9 Q23 Q9 16 128 *)
-  0x6e6e8797;       (* arm_SUB_VEC Q23 Q28 Q14 16 128 *)
-  0x4e6e879c;       (* arm_ADD_VEC Q28 Q28 Q14 16 128 *)
-  0x4f70d12e;       (* arm_SQRDMULH_VEC Q14 Q9 (Q0 :> LANE_H 3) 16 128 *)
-  0x6f47405b;       (* arm_MLS_VEC Q27 Q2 (Q7 :> LANE_H 0) 16 128 *)
-  0x3d800c1c;       (* arm_STR Q28 X0 (Immediate_Offset (word 48)) *)
-  0x4f608122;       (* arm_MUL_VEC Q2 Q9 (Q0 :> LANE_H 2) 16 128 *)
-  0x6f4741c2;       (* arm_MLS_VEC Q2 Q14 (Q7 :> LANE_H 0) 16 128 *)
-  0x6e7b86dc;       (* arm_SUB_VEC Q28 Q22 Q27 16 128 *)
-  0x4e7b86db;       (* arm_ADD_VEC Q27 Q22 Q27 16 128 *)
-  0x6f4741b1;       (* arm_MLS_VEC Q17 Q13 (Q7 :> LANE_H 0) 16 128 *)
-  0x3d801c1b;       (* arm_STR Q27 X0 (Immediate_Offset (word 112)) *)
-  0x4f4082fb;       (* arm_MUL_VEC Q27 Q23 (Q0 :> LANE_H 0) 16 128 *)
-  0x4e64844d;       (* arm_ADD_VEC Q13 Q2 Q4 16 128 *)
-  0x6e648442;       (* arm_SUB_VEC Q2 Q2 Q4 16 128 *)
-  0x4f50d2e9;       (* arm_SQRDMULH_VEC Q9 Q23 (Q0 :> LANE_H 1) 16 128 *)
-  0x3d803c11;       (* arm_STR Q17 X0 (Immediate_Offset (word 240)) *)
-  0x3d802c0d;       (* arm_STR Q13 X0 (Immediate_Offset (word 176)) *)
-  0x4f50d04d;       (* arm_SQRDMULH_VEC Q13 Q2 (Q0 :> LANE_H 1) 16 128 *)
-  0x4f408042;       (* arm_MUL_VEC Q2 Q2 (Q0 :> LANE_H 0) 16 128 *)
-  0x6f47413b;       (* arm_MLS_VEC Q27 Q9 (Q7 :> LANE_H 0) 16 128 *)
-  0x4f50d389;       (* arm_SQRDMULH_VEC Q9 Q28 (Q0 :> LANE_H 1) 16 128 *)
-  0x6f4741a2;       (* arm_MLS_VEC Q2 Q13 (Q7 :> LANE_H 0) 16 128 *)
-  0x3d804c1b;       (* arm_STR Q27 X0 (Immediate_Offset (word 304)) *)
-  0x4f40839b;       (* arm_MUL_VEC Q27 Q28 (Q0 :> LANE_H 0) 16 128 *)
-  0x6f47413b;       (* arm_MLS_VEC Q27 Q9 (Q7 :> LANE_H 0) 16 128 *)
-  0x3d806c02;       (* arm_STR Q2 X0 (Immediate_Offset (word 432)) *)
-  0x3d805c1b;       (* arm_STR Q27 X0 (Immediate_Offset (word 368)) *)
-  0x6d4027e8;       (* arm_LDP D8 D9 SP (Immediate_Offset (word 0)) *)
-  0x6d412fea;       (* arm_LDP D10 D11 SP (Immediate_Offset (word 16)) *)
-  0x6d4237ec;       (* arm_LDP D12 D13 SP (Immediate_Offset (word 32)) *)
-  0x6d433fee;       (* arm_LDP D14 D15 SP (Immediate_Offset (word 48)) *)
+  0x3dc00009;       (* arm_LDR Q9 X0 (Immediate_Offset (word 0)) *)
+  0x4f50db19;       (* arm_SQRDMULH_VEC Q25 Q24 (Q0 :> LANE_H 5) 16 128 *)
+  0x3dc03015;       (* arm_LDR Q21 X0 (Immediate_Offset (word 192)) *)
+  0x3dc01010;       (* arm_LDR Q16 X0 (Immediate_Offset (word 64)) *)
+  0x4f40885e;       (* arm_MUL_VEC Q30 Q2 (Q0 :> LANE_H 4) 16 128 *)
+  0x3dc02011;       (* arm_LDR Q17 X0 (Immediate_Offset (word 128)) *)
+  0x6f47439e;       (* arm_MLS_VEC Q30 Q28 (Q7 :> LANE_H 0) 16 128 *)
+  0x4e70852f;       (* arm_ADD_VEC Q15 Q9 Q16 16 128 *)
+  0x6e758632;       (* arm_SUB_VEC Q18 Q17 Q21 16 128 *)
+  0x6f474326;       (* arm_MLS_VEC Q6 Q25 (Q7 :> LANE_H 0) 16 128 *)
+  0x4e758633;       (* arm_ADD_VEC Q19 Q17 Q21 16 128 *)
+  0x6e70852e;       (* arm_SUB_VEC Q14 Q9 Q16 16 128 *)
+  0x4f418248;       (* arm_MUL_VEC Q8 Q18 (Q1 :> LANE_H 0) 16 128 *)
+  0x4e7385fb;       (* arm_ADD_VEC Q27 Q15 Q19 16 128 *)
+  0x4f70d9d6;       (* arm_SQRDMULH_VEC Q22 Q14 (Q0 :> LANE_H 7) 16 128 *)
+  0x4f51d243;       (* arm_SQRDMULH_VEC Q3 Q18 (Q1 :> LANE_H 1) 16 128 *)
+  0x4e648570;       (* arm_ADD_VEC Q16 Q11 Q4 16 128 *)
+  0x4f6089dd;       (* arm_MUL_VEC Q29 Q14 (Q0 :> LANE_H 6) 16 128 *)
+  0x6f4742dd;       (* arm_MLS_VEC Q29 Q22 (Q7 :> LANE_H 0) 16 128 *)
+  0x6e7385f6;       (* arm_SUB_VEC Q22 Q15 Q19 16 128 *)
+  0x4e7484ba;       (* arm_ADD_VEC Q26 Q5 Q20 16 128 *)
+  0x6f474068;       (* arm_MLS_VEC Q8 Q3 (Q7 :> LANE_H 0) 16 128 *)
+  0x6e7a8775;       (* arm_SUB_VEC Q21 Q27 Q26 16 128 *)
+  0x4e7a8778;       (* arm_ADD_VEC Q24 Q27 Q26 16 128 *)
+  0x4f70d2d7;       (* arm_SQRDMULH_VEC Q23 Q22 (Q0 :> LANE_H 3) 16 128 *)
+  0x3c810418;       (* arm_STR Q24 X0 (Postimmediate_Offset (word 16)) *)
+  0x4f6082cd;       (* arm_MUL_VEC Q13 Q22 (Q0 :> LANE_H 2) 16 128 *)
+  0x6e6887b9;       (* arm_SUB_VEC Q25 Q29 Q8 16 128 *)
+  0x4e6887b2;       (* arm_ADD_VEC Q18 Q29 Q8 16 128 *)
+  0x4f4082ae;       (* arm_MUL_VEC Q14 Q21 (Q0 :> LANE_H 0) 16 128 *)
+  0x4e70865a;       (* arm_ADD_VEC Q26 Q18 Q16 16 128 *)
+  0x4f70d33f;       (* arm_SQRDMULH_VEC Q31 Q25 (Q0 :> LANE_H 3) 16 128 *)
+  0x6f4742ed;       (* arm_MLS_VEC Q13 Q23 (Q7 :> LANE_H 0) 16 128 *)
+  0x3d800c1a;       (* arm_STR Q26 X0 (Immediate_Offset (word 48)) *)
+  0x6e70864c;       (* arm_SUB_VEC Q12 Q18 Q16 16 128 *)
+  0x4f608322;       (* arm_MUL_VEC Q2 Q25 (Q0 :> LANE_H 2) 16 128 *)
+  0x6f4743e2;       (* arm_MLS_VEC Q2 Q31 (Q7 :> LANE_H 0) 16 128 *)
+  0x4f40818a;       (* arm_MUL_VEC Q10 Q12 (Q0 :> LANE_H 0) 16 128 *)
+  0x6e7e85a3;       (* arm_SUB_VEC Q3 Q13 Q30 16 128 *)
+  0x4e7e85b3;       (* arm_ADD_VEC Q19 Q13 Q30 16 128 *)
+  0x4f50d07c;       (* arm_SQRDMULH_VEC Q28 Q3 (Q0 :> LANE_H 1) 16 128 *)
+  0x6e668452;       (* arm_SUB_VEC Q18 Q2 Q6 16 128 *)
+  0x3d801c13;       (* arm_STR Q19 X0 (Immediate_Offset (word 112)) *)
+  0x4f50d197;       (* arm_SQRDMULH_VEC Q23 Q12 (Q0 :> LANE_H 1) 16 128 *)
+  0x4e66845a;       (* arm_ADD_VEC Q26 Q2 Q6 16 128 *)
+  0x4f50d251;       (* arm_SQRDMULH_VEC Q17 Q18 (Q0 :> LANE_H 1) 16 128 *)
+  0x4f50d2be;       (* arm_SQRDMULH_VEC Q30 Q21 (Q0 :> LANE_H 1) 16 128 *)
+  0x6f4742ea;       (* arm_MLS_VEC Q10 Q23 (Q7 :> LANE_H 0) 16 128 *)
+  0x4f408252;       (* arm_MUL_VEC Q18 Q18 (Q0 :> LANE_H 0) 16 128 *)
+  0x3d802c1a;       (* arm_STR Q26 X0 (Immediate_Offset (word 176)) *)
+  0x6f4743ce;       (* arm_MLS_VEC Q14 Q30 (Q7 :> LANE_H 0) 16 128 *)
+  0x3d804c0a;       (* arm_STR Q10 X0 (Immediate_Offset (word 304)) *)
+  0x6f474232;       (* arm_MLS_VEC Q18 Q17 (Q7 :> LANE_H 0) 16 128 *)
+  0x4f408077;       (* arm_MUL_VEC Q23 Q3 (Q0 :> LANE_H 0) 16 128 *)
+  0x3d803c0e;       (* arm_STR Q14 X0 (Immediate_Offset (word 240)) *)
+  0x6f474397;       (* arm_MLS_VEC Q23 Q28 (Q7 :> LANE_H 0) 16 128 *)
+  0x3d806c12;       (* arm_STR Q18 X0 (Immediate_Offset (word 432)) *)
+  0x3d805c17;       (* arm_STR Q23 X0 (Immediate_Offset (word 368)) *)
+  0x6d4027e8;       (* arm_LDP D8 D9 SP (Immediate_Offset (iword (&0))) *)
+  0x6d412fea;       (* arm_LDP D10 D11 SP (Immediate_Offset (iword (&16))) *)
+  0x6d4237ec;       (* arm_LDP D12 D13 SP (Immediate_Offset (iword (&32))) *)
+  0x6d433fee;       (* arm_LDP D14 D15 SP (Immediate_Offset (iword (&48))) *)
   0x910103ff;       (* arm_ADD SP SP (rvalue (word 64)) *)
   0xd65f03c0        (* arm_RET X30 *)
-]
-[114; 252; 114; 252; 53; 251; 53; 251; 219; 0; 219; 0; 87; 3; 87; 3; 3; 221;
- 3; 221; 210; 208; 210; 208; 108; 8; 108; 8; 224; 32; 224; 32; 151; 4; 151;
- 4; 138; 1; 138; 1; 251; 251; 251; 251; 68; 251; 68; 251; 46; 45; 46; 45; 38;
- 15; 38; 15; 111; 216; 111; 216; 102; 209; 102; 209; 139; 252; 139; 252; 195;
- 4; 195; 4; 175; 5; 175; 5; 71; 6; 71; 6; 249; 221; 249; 221; 223; 46; 223;
- 46; 242; 55; 242; 55; 202; 61; 202; 61; 120; 253; 120; 253; 55; 250; 55;
- 250; 200; 2; 200; 2; 170; 2; 170; 2; 22; 231; 22; 231; 14; 199; 14; 199; 96;
- 27; 96; 27; 57; 26; 57; 26; 138; 252; 138; 252; 155; 4; 155; 4; 254; 251;
- 254; 251; 188; 251; 188; 251; 239; 221; 239; 221; 85; 45; 85; 45; 141; 216;
- 141; 216; 3; 214; 3; 214; 42; 2; 42; 2; 137; 251; 137; 251; 109; 254; 109;
- 254; 13; 2; 13; 2; 77; 21; 77; 21; 13; 212; 13; 212; 129; 240; 129; 240; 48;
- 20; 48; 20; 159; 3; 159; 3; 2; 250; 2; 250; 205; 1; 205; 1; 98; 250; 98;
- 250; 165; 35; 165; 35; 5; 197; 5; 197; 186; 17; 186; 17; 181; 200; 181; 200;
- 223; 2; 223; 2; 207; 253; 207; 253; 11; 253; 11; 253; 193; 254; 193; 254;
- 67; 28; 67; 28; 110; 234; 110; 234; 229; 226; 229; 226; 188; 243; 188; 243;
- 95; 3; 95; 3; 206; 4; 206; 4; 44; 2; 44; 2; 217; 251; 217; 251; 47; 33; 47;
- 33; 75; 47; 75; 47; 97; 21; 97; 21; 33; 215; 33; 215; 60; 254; 60; 254; 217;
- 252; 217; 252; 101; 250; 101; 250; 242; 3; 242; 3; 159; 238; 159; 238; 249;
- 224; 249; 224; 211; 200; 211; 200; 214; 38; 214; 38; 147; 249; 147; 249; 12;
- 3; 12; 3; 109; 0; 109; 0; 7; 4; 7; 4; 192; 192; 192; 192; 254; 29; 254; 29;
- 49; 4; 49; 4; 164; 39; 164; 39; 215; 4; 215; 4; 137; 254; 137; 254; 12; 5;
- 12; 5; 208; 249; 208; 249; 164; 47; 164; 47; 149; 241; 149; 241; 173; 49;
- 173; 49; 24; 195; 24; 195; 134; 5; 134; 5; 216; 250; 216; 250; 223; 255;
- 223; 255; 208; 1; 208; 1; 94; 54; 94; 54; 63; 205; 63; 205; 187; 254; 187;
- 254; 215; 17; 215; 17; 127; 253; 127; 253; 224; 3; 224; 3; 173; 3; 173; 3;
- 253; 3; 253; 3; 91; 231; 91; 231; 36; 38; 36; 38; 46; 36; 46; 36; 66; 39;
- 66; 39; 244; 254; 244; 254; 35; 253; 35; 253; 124; 3; 124; 3; 85; 252; 85;
- 252; 178; 245; 178; 245; 209; 227; 209; 227; 76; 34; 76; 34; 229; 219; 229;
- 219; 136; 253; 136; 253; 48; 3; 48; 3; 72; 5; 72; 5; 118; 253; 118; 253;
- 179; 231; 179; 231; 96; 31; 96; 31; 252; 51; 252; 51; 2; 231; 2; 231; 130;
- 2; 130; 2; 72; 252; 72; 252; 4; 6; 4; 6; 141; 249; 141; 249; 175; 24; 175;
- 24; 101; 219; 101; 219; 55; 59; 55; 59; 133; 192; 133; 192; 75; 250; 75;
- 250; 202; 5; 202; 5; 28; 2; 28; 2; 90; 6; 90; 6; 211; 199; 211; 199; 252;
- 56; 252; 56; 195; 20; 195; 20; 133; 62; 133; 62; 250; 4; 250; 4; 28; 4; 28;
- 4; 1; 4; 1; 4; 83; 251; 83; 251; 252; 48; 252; 48; 115; 40; 115; 40; 105;
- 39; 105; 39; 250; 209; 250; 209; 23; 1; 23; 1; 149; 4; 149; 4; 23; 255; 23;
- 255; 155; 2; 155; 2; 186; 10; 186; 10; 26; 45; 26; 45; 11; 247; 11; 247;
- 165; 25; 165; 25; 58; 1; 58; 1; 12; 253; 12; 253; 48; 0; 48; 0; 127; 250;
- 127; 250; 19; 12; 19; 12; 239; 226; 239; 226; 216; 1; 216; 1; 211; 201; 211;
- 201; 37; 6; 37; 6; 76; 0; 76; 0; 181; 254; 181; 254; 223; 254; 223; 254;
- 123; 60; 123; 60; 236; 2; 236; 2; 70; 243; 70; 243; 227; 244; 227; 244; 180;
- 251; 180; 251; 45; 253; 45; 253; 168; 2; 168; 2; 56; 2; 56; 2; 180; 213;
- 180; 213; 51; 228; 51; 228; 37; 26; 37; 26; 215; 21; 215; 21; 17; 4; 17; 4;
- 155; 249; 155; 249; 185; 253; 185; 253; 239; 255; 239; 255; 7; 40; 7; 40;
- 15; 193; 15; 193; 149; 233; 149; 233; 89; 255; 89; 255; 47; 6; 222; 60; 203;
- 252; 111; 224; 75; 5; 26; 52; 0; 0; 0; 0; 199; 253; 31; 234; 194; 1; 77; 17;
- 168; 3; 253; 35; 0; 0; 0; 0; 69; 0; 167; 2; 191; 1; 48; 17; 233; 253; 110;
- 235; 0; 0; 0; 0; 31; 2; 225; 20; 211; 4; 124; 47; 110; 250; 44; 201; 0; 0;
- 0; 0; 227; 252; 91; 225; 203; 250; 191; 204; 65; 4; 223; 41; 0; 0; 0; 0; 63;
- 255; 148; 248; 200; 255; 217; 253; 27; 1; 226; 10; 0; 0; 0; 0; 130; 5; 55;
- 54; 60; 250; 63; 199; 197; 250; 132; 204; 0; 0; 0; 0; 218; 251; 43; 215;
- 114; 3; 234; 33; 216; 254; 158; 244; 0; 0; 0; 0; 64; 6; 133; 61; 40; 0; 138;
- 1; 237; 2; 205; 28; 176; 252; 101; 223; 152; 5; 15; 55; 138; 253; 199; 231;
- 175; 2; 106; 26; 0; 0; 0; 0];;
+];;
 
 let MLKEM_INTT_EXEC = ARM_MK_EXEC_RULE mlkem_intt_mc;;
 
 (* ------------------------------------------------------------------------- *)
-(* Correctness proof.                                                        *)
+(* Data tables that are assumed in the precondition.                         *)
+(* ------------------------------------------------------------------------- *)
+
+let intt_zetas_layer01234 = define
+ `intt_zetas_layer01234:int list =
+   [&1583; &15582; -- &821; -- &8081; &1355; &13338; &0; &0; -- &569; -- &5601;
+    &450; &4429; &936; &9213; &0; &0; &69; &679; &447; &4400; -- &535;
+    -- &5266; &0; &0; &543; &5345; &1235; &12156; -- &1426; -- &14036; &0;
+    &0; -- &797; -- &7845; -- &1333; -- &13121; &1089; &10719; &0; &0;
+    -- &193; -- &1900; -- &56; -- &551; &283; &2786; &0; &0; &1410; &13879;
+    -- &1476; -- &14529; -- &1339; -- &13180; &0; &0; -- &1062; -- &10453;
+    &882; &8682; -- &296; -- &2914; &0; &0; &1600; &15749; &40; &394;
+    &749; &7373; -- &848; -- &8347; &1432; &14095; -- &630; -- &6201;
+    &687; &6762; &0; &0]`;;
+
+let intt_zetas_layer56 = define
+ `intt_zetas_layer56:int list =
+   [-- &910; -- &910; -- &1227; -- &1227; &219; &219; &855; &855; -- &8957;
+    -- &8957; -- &12078; -- &12078; &2156; &2156; &8416; &8416; &1175;
+    &1175; &394; &394; -- &1029; -- &1029; -- &1212; -- &1212; &11566;
+    &11566; &3878; &3878; -- &10129; -- &10129; -- &11930; -- &11930;
+    -- &885; -- &885; &1219; &1219; &1455; &1455; &1607; &1607; -- &8711;
+    -- &8711; &11999; &11999; &14322; &14322; &15818; &15818; -- &648;
+    -- &648; -- &1481; -- &1481; &712; &712; &682; &682; -- &6378; -- &6378;
+    -- &14578; -- &14578; &7008; &7008; &6713; &6713; -- &886; -- &886;
+    &1179; &1179; -- &1026; -- &1026; -- &1092; -- &1092; -- &8721;
+    -- &8721; &11605; &11605; -- &10099; -- &10099; -- &10749; -- &10749;
+    &554; &554; -- &1143; -- &1143; -- &403; -- &403; &525; &525; &5453;
+    &5453; -- &11251; -- &11251; -- &3967; -- &3967; &5168; &5168; &927;
+    &927; -- &1534; -- &1534; &461; &461; -- &1438; -- &1438; &9125;
+    &9125; -- &15099; -- &15099; &4538; &4538; -- &14155; -- &14155; &735;
+    &735; -- &561; -- &561; -- &757; -- &757; -- &319; -- &319; &7235;
+    &7235; -- &5522; -- &5522; -- &7451; -- &7451; -- &3140; -- &3140;
+    &863; &863; &1230; &1230; &556; &556; -- &1063; -- &1063; &8495;
+    &8495; &12107; &12107; &5473; &5473; -- &10463; -- &10463; -- &452;
+    -- &452; -- &807; -- &807; -- &1435; -- &1435; &1010; &1010; -- &4449;
+    -- &4449; -- &7943; -- &7943; -- &14125; -- &14125; &9942; &9942;
+    -- &1645; -- &1645; &780; &780; &109; &109; &1031; &1031; -- &16192;
+    -- &16192; &7678; &7678; &1073; &1073; &10148; &10148; &1239; &1239;
+    -- &375; -- &375; &1292; &1292; -- &1584; -- &1584; &12196; &12196;
+    -- &3691; -- &3691; &12717; &12717; -- &15592; -- &15592; &1414; &1414;
+    -- &1320; -- &1320; -- &33; -- &33; &464; &464; &13918; &13918;
+    -- &12993; -- &12993; -- &325; -- &325; &4567; &4567; -- &641; -- &641;
+    &992; &992; &941; &941; &1021; &1021; -- &6309; -- &6309; &9764;
+    &9764; &9262; &9262; &10050; &10050; -- &268; -- &268; -- &733;
+    -- &733; &892; &892; -- &939; -- &939; -- &2638; -- &2638; -- &7215;
+    -- &7215; &8780; &8780; -- &9243; -- &9243; -- &632; -- &632; &816; &816;
+    &1352; &1352; -- &650; -- &650; -- &6221; -- &6221; &8032; &8032;
+    &13308; &13308; -- &6398; -- &6398; &642; &642; -- &952; -- &952;
+    &1540; &1540; -- &1651; -- &1651; &6319; &6319; -- &9371; -- &9371;
+    &15159; &15159; -- &16251; -- &16251; -- &1461; -- &1461; &1482;
+    &1482; &540; &540; &1626; &1626; -- &14381; -- &14381; &14588; &14588;
+    &5315; &5315; &16005; &16005; &1274; &1274; &1052; &1052; &1025;
+    &1025; -- &1197; -- &1197; &12540; &12540; &10355; &10355; &10089;
+    &10089; -- &11782; -- &11782; &279; &279; &1173; &1173; -- &233;
+    -- &233; &667; &667; &2746; &2746; &11546; &11546; -- &2293; -- &2293;
+    &6565; &6565; &314; &314; -- &756; -- &756; &48; &48; -- &1409;
+    -- &1409; &3091; &3091; -- &7441; -- &7441; &472; &472; -- &13869;
+    -- &13869; &1573; &1573; &76; &76; -- &331; -- &331; -- &289; -- &289;
+    &15483; &15483; &748; &748; -- &3258; -- &3258; -- &2845; -- &2845;
+    -- &1100; -- &1100; -- &723; -- &723; &680; &680; &568; &568; -- &10828;
+    -- &10828; -- &7117; -- &7117; &6693; &6693; &5591; &5591; &1041;
+    &1041; -- &1637; -- &1637; -- &583; -- &583; -- &17; -- &17; &10247;
+    &10247; -- &16113; -- &16113; -- &5739; -- &5739; -- &167; -- &167]`;;
+
+let intt_constants = define
+ `intt_constants z_01234 z_56 s <=>
+        (!i. i < 80
+             ==> read(memory :> bytes16(word_add z_01234 (word(2 * i)))) s =
+                 iword(EL i intt_zetas_layer01234)) /\
+        (!i. i < 384
+             ==> read(memory :> bytes16(word_add z_56 (word(2 * i)))) s =
+                 iword(EL i intt_zetas_layer56))`;;
+
+(* ------------------------------------------------------------------------- *)
+(* Some convenient proof tools.                                              *)
 (* ------------------------------------------------------------------------- *)
 
 let READ_MEMORY_MERGE_CONV =
@@ -488,26 +506,33 @@ let SIMD_SIMPLIFY_TAC =
     CONV_RULE(RAND_CONV SIMD_SIMPLIFY_CONV) o
     check (simdable o concl)));;
 
-let BYTES_LOADED_DATA = prove
- (`bytes_loaded s (word (pc + 0x5dc)) mlkem_intt_data <=>
-   read (memory :> bytes(word (pc + 0x5dc),928)) s =
-   num_of_bytelist mlkem_intt_data`,
-  REWRITE_TAC[bytes_loaded; READ_BYTELIST_EQ_BYTES;
-    CONV_RULE (RAND_CONV LENGTH_CONV)
-     (AP_TERM `LENGTH:byte list->num` mlkem_intt_data)]);;
+let MEMORY_128_FROM_16_TAC =
+  let a_tm = `a:int64` and n_tm = `n:num` and i64_ty = `:int64`
+  and pat = `read (memory :> bytes128(word_add a (word n))) s0` in
+  fun v n ->
+    let pat' = subst[mk_var(v,i64_ty),a_tm] pat in
+    let f i =
+      let itm = mk_small_numeral(16*i) in
+      READ_MEMORY_MERGE_CONV 3 (subst[itm,n_tm] pat') in
+    MP_TAC(end_itlist CONJ (map f (0--(n-1))));;
+
+(* ------------------------------------------------------------------------- *)
+(* Correctness proof.                                                        *)
+(* ------------------------------------------------------------------------- *)
 
 let MLKEM_INTT_CORRECT = prove
- (`!a x pc.
-      nonoverlapping (word pc,0x97c) (a,512)
+ (`!a z_01234 z_56 x pc.
+      ALL (nonoverlapping (a,512))
+          [(word pc,0x5d0); (z_01234,160); (z_56,768)]
       ==> ensures arm
-           (\s. aligned_bytes_loaded s (word pc)
-                 (APPEND mlkem_intt_mc mlkem_intt_data) /\
+           (\s. aligned_bytes_loaded s (word pc) mlkem_intt_mc /\
                 read PC s = word (pc + 0x14) /\
-                C_ARGUMENTS [a] s /\
+                C_ARGUMENTS [a; z_01234; z_56] s /\
+                intt_constants z_01234 z_56 s /\
                 !i. i < 256
                     ==> read(memory :> bytes16(word_add a (word(2 * i)))) s =
                         x i)
-           (\s. read PC s = word(pc + 0x5c4) /\
+           (\s. read PC s = word(pc + 0x5b8) /\
                 !i. i < 256
                     ==> let zi =
                          read(memory :> bytes16(word_add a (word(2 * i)))) s in
@@ -516,62 +541,41 @@ let MLKEM_INTT_CORRECT = prove
            (MAYCHANGE_REGS_AND_FLAGS_PERMITTED_BY_ABI ,,
             MAYCHANGE [Q8; Q9; Q10; Q11; Q12; Q13; Q14; Q15] ,,
             MAYCHANGE [memory :> bytes(a,512)])`,
-  MAP_EVERY X_GEN_TAC [`a:int64`; `x:num->int16`; `pc:num`] THEN
+  MAP_EVERY X_GEN_TAC
+   [`a:int64`; `z_01234:int64`; `z_56:int64`; `x:num->int16`; `pc:num`] THEN
   REWRITE_TAC[MAYCHANGE_REGS_AND_FLAGS_PERMITTED_BY_ABI; C_ARGUMENTS;
-              NONOVERLAPPING_CLAUSES] THEN
+              NONOVERLAPPING_CLAUSES; ALL] THEN
   DISCH_THEN(REPEAT_TCL CONJUNCTS_THEN ASSUME_TAC) THEN
-
-  (*** Fiddle around with the constant table stuff ***)
-
-  REWRITE_TAC[ALIGNED_BYTES_LOADED_APPEND_CLAUSE] THEN
-  REWRITE_TAC[fst MLKEM_INTT_EXEC] THEN REWRITE_TAC[BYTES_LOADED_DATA] THEN
 
   (*** Manually expand the cases in the hypotheses ***)
 
+  REWRITE_TAC[intt_constants] THEN
   CONV_TAC(RATOR_CONV(LAND_CONV(ONCE_DEPTH_CONV
    (EXPAND_CASES_CONV THENC ONCE_DEPTH_CONV NUM_MULT_CONV)))) THEN
-
+  REWRITE_TAC[intt_zetas_layer01234; intt_zetas_layer56] THEN
+  CONV_TAC(ONCE_DEPTH_CONV EL_CONV) THEN
+  CONV_TAC(ONCE_DEPTH_CONV WORD_IWORD_CONV) THEN REWRITE_TAC[WORD_ADD_0] THEN
   ENSURES_INIT_TAC "s0" THEN
 
   (*** Manually restructure to match the 128-bit loads. It would be nicer
    *** if the simulation machinery did this automatically.
    ***)
 
-  MP_TAC(end_itlist CONJ (map (fun n -> READ_MEMORY_MERGE_CONV 3
-            (subst[mk_small_numeral(16*n),`n:num`]
-                  `read (memory :> bytes128(word_add a (word n))) s0`))
-            (0--31))) THEN
-  ASM_REWRITE_TAC[WORD_ADD_0] THEN
+  MEMORY_128_FROM_16_TAC "a" 32 THEN
+  MEMORY_128_FROM_16_TAC "z_01234" 10 THEN
+  MEMORY_128_FROM_16_TAC "z_56" 48 THEN
+  ASM_REWRITE_TAC[WORD_ADD_0] THEN CONV_TAC WORD_REDUCE_CONV THEN
   DISCARD_MATCHING_ASSUMPTIONS [`read (memory :> bytes16 a) s = x`] THEN
-  STRIP_TAC THEN
+  REPEAT STRIP_TAC THEN
 
-  (*** Palaver to address the precomputed tables via "wpc" ***)
+  (*** Ghost up initial contents of Q7 since it isn't fully initialized ***)
 
-  ASSUME_TAC(WORD_RULE
-   `word(pc + 0x8dc):int64 = word_add (word(pc + 0x5dc)) (word 768)`) THEN
-  FIRST_ASSUM(MP_TAC o GEN_REWRITE_RULE I [GSYM BYTES_LOADED_DATA]) THEN
-  ABBREV_TAC `wpc:int64 = word(pc + 0x5dc)` THEN
-  SUBST1_TAC(WORD_RULE `wpc:int64 = word(val wpc + 0)`) THEN
-  REWRITE_TAC[mlkem_intt_data] THEN CONV_TAC(LAND_CONV DATA64_CONV) THEN
-  REWRITE_TAC[WORD_RULE `word(val x + n) = word_add x (word n)`] THEN
-  REWRITE_TAC[bytes_loaded_nil] THEN STRIP_TAC THEN
-  SUBGOAL_THEN `nonoverlapping (a:int64,512) (wpc:int64,928)` MP_TAC THEN
-  REWRITE_TAC[NONOVERLAPPING_CLAUSES] THENL
-   [EXPAND_TAC "wpc" THEN NONOVERLAPPING_TAC;
-    DISCH_TAC] THEN
-  MP_TAC(end_itlist CONJ (map (fun n -> READ_MEMORY_MERGE_CONV 1
-            (subst[mk_small_numeral(16*n),`n:num`]
-                  `read (memory :> bytes128(word_add wpc (word n))) s0`))
-            (0--57))) THEN
-  ASM_REWRITE_TAC[WORD_ADD_0] THEN
-  CONV_TAC(LAND_CONV(DEPTH_CONV WORD_NUM_RED_CONV)) THEN
-  DISCARD_MATCHING_ASSUMPTIONS [`read (memory :> bytes64 a) s = x`] THEN
-  STRIP_TAC THEN
+  ABBREV_TAC `v7_init:int128 = read Q7 s0` THEN
 
   (*** Simulate all the way to the end, in effect unrolling loops ***)
 
   MAP_EVERY (fun n -> ARM_STEPS_TAC MLKEM_INTT_EXEC [n] THEN SIMD_SIMPLIFY_TAC)
-            (1--1184) THEN
+            (1--1181) THEN
   ENSURES_FINAL_STATE_TAC THEN ASM_REWRITE_TAC[] THEN
 
   (*** Reverse the restructuring by splitting the 128-bit words up ***)
@@ -586,7 +590,7 @@ let MLKEM_INTT_CORRECT = prove
   CONV_TAC(ONCE_DEPTH_CONV let_CONV) THEN REWRITE_TAC[INT_ABS_BOUNDS] THEN
   GEN_REWRITE_TAC (BINDER_CONV o RAND_CONV) [GSYM I_THM] THEN
   CONV_TAC(EXPAND_CASES_CONV THENC ONCE_DEPTH_CONV NUM_MULT_CONV) THEN
-  ASM_REWRITE_TAC[I_THM; WORD_ADD_0] THEN DISCARD_STATE_TAC "s1184" THEN
+  ASM_REWRITE_TAC[I_THM; WORD_ADD_0] THEN DISCARD_STATE_TAC "s1181" THEN
   REPEAT(W(fun (asl,w) ->
      if length(conjuncts w) > 3 then CONJ_TAC else NO_TAC)) THEN
 
@@ -609,18 +613,19 @@ let MLKEM_INTT_CORRECT = prove
 (*** Subroutine form, somewhat messy elaboration of the usual wrapper ***)
 
 let MLKEM_INTT_SUBROUTINE_CORRECT = prove
- (`!a x pc stackpointer returnaddress.
+ (`!a z_01234 z_56 x pc stackpointer returnaddress.
       aligned 16 stackpointer /\
-      ALL (nonoverlapping (word_sub stackpointer (word 64),64))
-          [(word pc,0x97c); (a,512)] /\
-      nonoverlapping (word pc,0x97c) (a,512)
+      ALLPAIRS nonoverlapping
+       [(a,512); (word_sub stackpointer (word 64),64)]
+       [(word pc,0x5d0); (z_01234,160); (z_56,768)] /\
+      nonoverlapping (a,512) (word_sub stackpointer (word 64),64)
       ==> ensures arm
-           (\s. aligned_bytes_loaded s (word pc)
-                 (APPEND mlkem_intt_mc mlkem_intt_data) /\
+           (\s. aligned_bytes_loaded s (word pc) mlkem_intt_mc /\
                 read PC s = word pc /\
                 read SP s = stackpointer /\
                 read X30 s = returnaddress /\
-                C_ARGUMENTS [a] s /\
+                C_ARGUMENTS [a; z_01234; z_56] s /\
+                intt_constants z_01234 z_56 s /\
                 !i. i < 256
                     ==> read(memory :> bytes16(word_add a (word(2 * i)))) s =
                         x i)
@@ -634,14 +639,13 @@ let MLKEM_INTT_SUBROUTINE_CORRECT = prove
             MAYCHANGE [memory :> bytes(a,512);
                        memory :> bytes(word_sub stackpointer (word 64),64)])`,
   let TWEAK_CONV =
+    REWRITE_CONV[intt_constants] THENC
     ONCE_DEPTH_CONV let_CONV THENC
     ONCE_DEPTH_CONV EXPAND_CASES_CONV THENC
     ONCE_DEPTH_CONV NUM_MULT_CONV THENC
     PURE_REWRITE_CONV [WORD_ADD_0] in
-  REWRITE_TAC[ALIGNED_BYTES_LOADED_APPEND_CLAUSE; BYTES_LOADED_DATA;
-              fst MLKEM_INTT_EXEC] THEN
+  REWRITE_TAC[fst MLKEM_INTT_EXEC] THEN
   CONV_TAC TWEAK_CONV THEN
   ARM_ADD_RETURN_STACK_TAC ~pre_post_nsteps:(5,5) MLKEM_INTT_EXEC
-   (REWRITE_RULE[ALIGNED_BYTES_LOADED_APPEND_CLAUSE; BYTES_LOADED_DATA;
-                 fst MLKEM_INTT_EXEC] (CONV_RULE TWEAK_CONV MLKEM_INTT_CORRECT))
+   (REWRITE_RULE[fst MLKEM_INTT_EXEC] (CONV_RULE TWEAK_CONV MLKEM_INTT_CORRECT))
     `[D8; D9; D10; D11; D12; D13; D14; D15]` 64);;
