arm/proofs/mlkem_ntt.ml
@@ -10,22 +10,17 @@
 needs "arm/proofs/base.ml";;
 needs "arm/proofs/utils/mlkem.ml";;
 
-(**** print_coda_from_elf (-1) "arm/mlkem/mlkem_ntt.o";;
+(**** print_literal_from_elf "arm/mlkem/mlkem_ntt.o";;
  ****)
 
-let mlkem_ntt_mc,mlkem_ntt_data = define_coda_literal_from_elf
-  "mlkem_ntt_mc" "mlkem_ntt_data" "arm/mlkem/mlkem_ntt.o"
+let mlkem_ntt_mc = define_assert_from_elf
+ "mlkem_ntt_mc" "arm/mlkem/mlkem_ntt.o"
 [
   0xd10103ff;       (* arm_SUB SP SP (rvalue (word 64)) *)
-  0x6d0027e8;       (* arm_STP D8 D9 SP (Immediate_Offset (word 0)) *)
-  0x6d012fea;       (* arm_STP D10 D11 SP (Immediate_Offset (word 16)) *)
-  0x6d0237ec;       (* arm_STP D12 D13 SP (Immediate_Offset (word 32)) *)
-  0x6d033fee;       (* arm_STP D14 D15 SP (Immediate_Offset (word 48)) *)
-  0x10002821;       (* arm_ADR X1 (word 1284) *)
-  0x91000021;       (* arm_ADD X1 X1 (rvalue (word 0)) *)
-  0x10002ce2;       (* arm_ADR X2 (word 1436) *)
-  0x91000042;       (* arm_ADD X2 X2 (rvalue (word 0)) *)
-  0x4e020fe7;       (* arm_DUP_GEN Q7 XZR 16 128 *)
+  0x6d0027e8;       (* arm_STP D8 D9 SP (Immediate_Offset (iword (&0))) *)
+  0x6d012fea;       (* arm_STP D10 D11 SP (Immediate_Offset (iword (&16))) *)
+  0x6d0237ec;       (* arm_STP D12 D13 SP (Immediate_Offset (iword (&32))) *)
+  0x6d033fee;       (* arm_STP D14 D15 SP (Immediate_Offset (iword (&48))) *)
   0x5281a025;       (* arm_MOV W5 (rvalue (word 3329)) *)
   0x4e021ca7;       (* arm_INS_GEN Q7 W5 0 16 *)
   0x5289d7e5;       (* arm_MOV W5 (rvalue (word 20159)) *)
@@ -34,374 +29,396 @@ let mlkem_ntt_mc,mlkem_ntt_data = define_coda_literal_from_elf
   0xd2800084;       (* arm_MOV X4 (rvalue (word 4)) *)
   0x3cc20420;       (* arm_LDR Q0 X1 (Postimmediate_Offset (word 32)) *)
   0x3cdf0021;       (* arm_LDR Q1 X1 (Immediate_Offset (word 18446744073709551600)) *)
-  0x3dc06017;       (* arm_LDR Q23 X0 (Immediate_Offset (word 384)) *)
-  0x3dc00019;       (* arm_LDR Q25 X0 (Immediate_Offset (word 0)) *)
-  0x3dc0400f;       (* arm_LDR Q15 X0 (Immediate_Offset (word 256)) *)
-  0x3dc03013;       (* arm_LDR Q19 X0 (Immediate_Offset (word 192)) *)
-  0x3dc0701e;       (* arm_LDR Q30 X0 (Immediate_Offset (word 448)) *)
-  0x3dc0201f;       (* arm_LDR Q31 X0 (Immediate_Offset (word 128)) *)
-  0x3dc0500e;       (* arm_LDR Q14 X0 (Immediate_Offset (word 320)) *)
+  0x3dc0601a;       (* arm_LDR Q26 X0 (Immediate_Offset (word 384)) *)
+  0x3dc0400e;       (* arm_LDR Q14 X0 (Immediate_Offset (word 256)) *)
   0x3dc0100c;       (* arm_LDR Q12 X0 (Immediate_Offset (word 64)) *)
-  0x4f50d2f2;       (* arm_SQRDMULH_VEC Q18 Q23 (Q0 :> LANE_H 1) 16 128 *)
-  0x4f4082f7;       (* arm_MUL_VEC Q23 Q23 (Q0 :> LANE_H 0) 16 128 *)
-  0x4f50d1e2;       (* arm_SQRDMULH_VEC Q2 Q15 (Q0 :> LANE_H 1) 16 128 *)
-  0x4f4081e3;       (* arm_MUL_VEC Q3 Q15 (Q0 :> LANE_H 0) 16 128 *)
-  0x4f50d3cf;       (* arm_SQRDMULH_VEC Q15 Q30 (Q0 :> LANE_H 1) 16 128 *)
-  0x4f4083de;       (* arm_MUL_VEC Q30 Q30 (Q0 :> LANE_H 0) 16 128 *)
-  0x6f474257;       (* arm_MLS_VEC Q23 Q18 (Q7 :> LANE_H 0) 16 128 *)
-  0x6f4741fe;       (* arm_MLS_VEC Q30 Q15 (Q7 :> LANE_H 0) 16 128 *)
-  0x4f4081c5;       (* arm_MUL_VEC Q5 Q14 (Q0 :> LANE_H 0) 16 128 *)
-  0x4e7787e6;       (* arm_ADD_VEC Q6 Q31 Q23 16 128 *)
-  0x6e7787ed;       (* arm_SUB_VEC Q13 Q31 Q23 16 128 *)
-  0x4f50d1d7;       (* arm_SQRDMULH_VEC Q23 Q14 (Q0 :> LANE_H 1) 16 128 *)
-  0x6e7e866f;       (* arm_SUB_VEC Q15 Q19 Q30 16 128 *)
-  0x4e7e8678;       (* arm_ADD_VEC Q24 Q19 Q30 16 128 *)
-  0x6f474043;       (* arm_MLS_VEC Q3 Q2 (Q7 :> LANE_H 0) 16 128 *)
-  0x4f50d9f3;       (* arm_SQRDMULH_VEC Q19 Q15 (Q0 :> LANE_H 5) 16 128 *)
-  0x6f4742e5;       (* arm_MLS_VEC Q5 Q23 (Q7 :> LANE_H 0) 16 128 *)
-  0x4e63872e;       (* arm_ADD_VEC Q14 Q25 Q3 16 128 *)
-  0x4f70d0ca;       (* arm_SQRDMULH_VEC Q10 Q6 (Q0 :> LANE_H 3) 16 128 *)
-  0x4f4089ff;       (* arm_MUL_VEC Q31 Q15 (Q0 :> LANE_H 4) 16 128 *)
-  0x6e658591;       (* arm_SUB_VEC Q17 Q12 Q5 16 128 *)
-  0x6f47427f;       (* arm_MLS_VEC Q31 Q19 (Q7 :> LANE_H 0) 16 128 *)
-  0x4f70d302;       (* arm_SQRDMULH_VEC Q2 Q24 (Q0 :> LANE_H 3) 16 128 *)
-  0x4f4089ab;       (* arm_MUL_VEC Q11 Q13 (Q0 :> LANE_H 4) 16 128 *)
+  0x3dc03004;       (* arm_LDR Q4 X0 (Immediate_Offset (word 192)) *)
+  0x3dc0000b;       (* arm_LDR Q11 X0 (Immediate_Offset (word 0)) *)
+  0x3dc05016;       (* arm_LDR Q22 X0 (Immediate_Offset (word 320)) *)
+  0x3dc0700a;       (* arm_LDR Q10 X0 (Immediate_Offset (word 448)) *)
+  0x3dc0201c;       (* arm_LDR Q28 X0 (Immediate_Offset (word 128)) *)
+  0x4f50d357;       (* arm_SQRDMULH_VEC Q23 Q26 (Q0 :> LANE_H 1) 16 128 *)
+  0x4f40835a;       (* arm_MUL_VEC Q26 Q26 (Q0 :> LANE_H 0) 16 128 *)
+  0x4f50d1d8;       (* arm_SQRDMULH_VEC Q24 Q14 (Q0 :> LANE_H 1) 16 128 *)
+  0x4f4081c9;       (* arm_MUL_VEC Q9 Q14 (Q0 :> LANE_H 0) 16 128 *)
+  0x4f50d2ce;       (* arm_SQRDMULH_VEC Q14 Q22 (Q0 :> LANE_H 1) 16 128 *)
+  0x4f4082d6;       (* arm_MUL_VEC Q22 Q22 (Q0 :> LANE_H 0) 16 128 *)
+  0x4f50d15d;       (* arm_SQRDMULH_VEC Q29 Q10 (Q0 :> LANE_H 1) 16 128 *)
+  0x6f4741d6;       (* arm_MLS_VEC Q22 Q14 (Q7 :> LANE_H 0) 16 128 *)
+  0x6f4742fa;       (* arm_MLS_VEC Q26 Q23 (Q7 :> LANE_H 0) 16 128 *)
+  0x4f40814e;       (* arm_MUL_VEC Q14 Q10 (Q0 :> LANE_H 0) 16 128 *)
+  0x4e76858a;       (* arm_ADD_VEC Q10 Q12 Q22 16 128 *)
+  0x6e76858c;       (* arm_SUB_VEC Q12 Q12 Q22 16 128 *)
+  0x6f4743ae;       (* arm_MLS_VEC Q14 Q29 (Q7 :> LANE_H 0) 16 128 *)
+  0x6e7a8796;       (* arm_SUB_VEC Q22 Q28 Q26 16 128 *)
+  0x4e7a8797;       (* arm_ADD_VEC Q23 Q28 Q26 16 128 *)
+  0x6f474309;       (* arm_MLS_VEC Q9 Q24 (Q7 :> LANE_H 0) 16 128 *)
+  0x4f50dada;       (* arm_SQRDMULH_VEC Q26 Q22 (Q0 :> LANE_H 5) 16 128 *)
+  0x6e6e849c;       (* arm_SUB_VEC Q28 Q4 Q14 16 128 *)
+  0x4e6e848e;       (* arm_ADD_VEC Q14 Q4 Q14 16 128 *)
+  0x4f408acd;       (* arm_MUL_VEC Q13 Q22 (Q0 :> LANE_H 4) 16 128 *)
+  0x6e698572;       (* arm_SUB_VEC Q18 Q11 Q9 16 128 *)
+  0x4f50db84;       (* arm_SQRDMULH_VEC Q4 Q28 (Q0 :> LANE_H 5) 16 128 *)
+  0x4f70d1d6;       (* arm_SQRDMULH_VEC Q22 Q14 (Q0 :> LANE_H 3) 16 128 *)
+  0x4f408b9c;       (* arm_MUL_VEC Q28 Q28 (Q0 :> LANE_H 4) 16 128 *)
+  0x6f47409c;       (* arm_MLS_VEC Q28 Q4 (Q7 :> LANE_H 0) 16 128 *)
+  0x4f6081ce;       (* arm_MUL_VEC Q14 Q14 (Q0 :> LANE_H 2) 16 128 *)
+  0x6f4742ce;       (* arm_MLS_VEC Q14 Q22 (Q7 :> LANE_H 0) 16 128 *)
+  0x4e7c8584;       (* arm_ADD_VEC Q4 Q12 Q28 16 128 *)
+  0x6e7c858c;       (* arm_SUB_VEC Q12 Q12 Q28 16 128 *)
+  0x6f47434d;       (* arm_MLS_VEC Q13 Q26 (Q7 :> LANE_H 0) 16 128 *)
+  0x4f71d09a;       (* arm_SQRDMULH_VEC Q26 Q4 (Q1 :> LANE_H 3) 16 128 *)
+  0x6e6e8556;       (* arm_SUB_VEC Q22 Q10 Q14 16 128 *)
+  0x4e6e8553;       (* arm_ADD_VEC Q19 Q10 Q14 16 128 *)
+  0x4f618083;       (* arm_MUL_VEC Q3 Q4 (Q1 :> LANE_H 2) 16 128 *)
+  0x4f51d2ce;       (* arm_SQRDMULH_VEC Q14 Q22 (Q1 :> LANE_H 1) 16 128 *)
+  0x4f4182dc;       (* arm_MUL_VEC Q28 Q22 (Q1 :> LANE_H 0) 16 128 *)
+  0x6f474343;       (* arm_MLS_VEC Q3 Q26 (Q7 :> LANE_H 0) 16 128 *)
+  0x6f4741dc;       (* arm_MLS_VEC Q28 Q14 (Q7 :> LANE_H 0) 16 128 *)
+  0x4f51d98e;       (* arm_SQRDMULH_VEC Q14 Q12 (Q1 :> LANE_H 5) 16 128 *)
+  0x4f41899a;       (* arm_MUL_VEC Q26 Q12 (Q1 :> LANE_H 4) 16 128 *)
+  0x4f70da75;       (* arm_SQRDMULH_VEC Q21 Q19 (Q0 :> LANE_H 7) 16 128 *)
+  0x6f4741da;       (* arm_MLS_VEC Q26 Q14 (Q7 :> LANE_H 0) 16 128 *)
   0xd1000484;       (* arm_SUB X4 X4 (rvalue (word 1)) *)
-  0x3dc06412;       (* arm_LDR Q18 X0 (Immediate_Offset (word 400)) *)
-  0x4f6080d0;       (* arm_MUL_VEC Q16 Q6 (Q0 :> LANE_H 2) 16 128 *)
-  0x6e63873c;       (* arm_SUB_VEC Q28 Q25 Q3 16 128 *)
-  0x3dc00419;       (* arm_LDR Q25 X0 (Immediate_Offset (word 16)) *)
-  0x6f474150;       (* arm_MLS_VEC Q16 Q10 (Q7 :> LANE_H 0) 16 128 *)
-  0x3dc04417;       (* arm_LDR Q23 X0 (Immediate_Offset (word 272)) *)
-  0x3dc03409;       (* arm_LDR Q9 X0 (Immediate_Offset (word 208)) *)
-  0x3dc02413;       (* arm_LDR Q19 X0 (Immediate_Offset (word 144)) *)
-  0x4e658588;       (* arm_ADD_VEC Q8 Q12 Q5 16 128 *)
-  0x4f50d25d;       (* arm_SQRDMULH_VEC Q29 Q18 (Q0 :> LANE_H 1) 16 128 *)
-  0x3dc07416;       (* arm_LDR Q22 X0 (Immediate_Offset (word 464)) *)
-  0x4e7f862a;       (* arm_ADD_VEC Q10 Q17 Q31 16 128 *)
-  0x3dc05404;       (* arm_LDR Q4 X0 (Immediate_Offset (word 336)) *)
-  0x4f50d2ec;       (* arm_SQRDMULH_VEC Q12 Q23 (Q0 :> LANE_H 1) 16 128 *)
-  0x4f4082e3;       (* arm_MUL_VEC Q3 Q23 (Q0 :> LANE_H 0) 16 128 *)
-  0x4f408254;       (* arm_MUL_VEC Q20 Q18 (Q0 :> LANE_H 0) 16 128 *)
-  0x6f4743b4;       (* arm_MLS_VEC Q20 Q29 (Q7 :> LANE_H 0) 16 128 *)
-  0x4f50d2d2;       (* arm_SQRDMULH_VEC Q18 Q22 (Q0 :> LANE_H 1) 16 128 *)
-  0x4f408085;       (* arm_MUL_VEC Q5 Q4 (Q0 :> LANE_H 0) 16 128 *)
-  0x4f50d9a6;       (* arm_SQRDMULH_VEC Q6 Q13 (Q0 :> LANE_H 5) 16 128 *)
-  0x4f608318;       (* arm_MUL_VEC Q24 Q24 (Q0 :> LANE_H 2) 16 128 *)
-  0x6f474058;       (* arm_MLS_VEC Q24 Q2 (Q7 :> LANE_H 0) 16 128 *)
-  0x4f4082da;       (* arm_MUL_VEC Q26 Q22 (Q0 :> LANE_H 0) 16 128 *)
-  0x6f4740cb;       (* arm_MLS_VEC Q11 Q6 (Q7 :> LANE_H 0) 16 128 *)
-  0x4e788502;       (* arm_ADD_VEC Q2 Q8 Q24 16 128 *)
-  0x6f47425a;       (* arm_MLS_VEC Q26 Q18 (Q7 :> LANE_H 0) 16 128 *)
-  0x4f60884d;       (* arm_MUL_VEC Q13 Q2 (Q0 :> LANE_H 6) 16 128 *)
-  0x4e6b878f;       (* arm_ADD_VEC Q15 Q28 Q11 16 128 *)
-  0x4f50d095;       (* arm_SQRDMULH_VEC Q21 Q4 (Q0 :> LANE_H 1) 16 128 *)
-  0x6e6b878b;       (* arm_SUB_VEC Q11 Q28 Q11 16 128 *)
-  0x6e7f8632;       (* arm_SUB_VEC Q18 Q17 Q31 16 128 *)
-  0x4f61815f;       (* arm_MUL_VEC Q31 Q10 (Q1 :> LANE_H 2) 16 128 *)
-  0x4f70d85b;       (* arm_SQRDMULH_VEC Q27 Q2 (Q0 :> LANE_H 7) 16 128 *)
-  0x4f51da5c;       (* arm_SQRDMULH_VEC Q28 Q18 (Q1 :> LANE_H 5) 16 128 *)
-  0x4f418a46;       (* arm_MUL_VEC Q6 Q18 (Q1 :> LANE_H 4) 16 128 *)
-  0x6f47436d;       (* arm_MLS_VEC Q13 Q27 (Q7 :> LANE_H 0) 16 128 *)
-  0x6f474386;       (* arm_MLS_VEC Q6 Q28 (Q7 :> LANE_H 0) 16 128 *)
-  0x4f71d151;       (* arm_SQRDMULH_VEC Q17 Q10 (Q1 :> LANE_H 3) 16 128 *)
-  0x6f474183;       (* arm_MLS_VEC Q3 Q12 (Q7 :> LANE_H 0) 16 128 *)
-  0x4e66856a;       (* arm_ADD_VEC Q10 Q11 Q6 16 128 *)
-  0x6e78851b;       (* arm_SUB_VEC Q27 Q8 Q24 16 128 *)
-  0x6f4742a5;       (* arm_MLS_VEC Q5 Q21 (Q7 :> LANE_H 0) 16 128 *)
-  0x3d80600a;       (* arm_STR Q10 X0 (Immediate_Offset (word 384)) *)
-  0x4e7085ca;       (* arm_ADD_VEC Q10 Q14 Q16 16 128 *)
-  0x4f51d368;       (* arm_SQRDMULH_VEC Q8 Q27 (Q1 :> LANE_H 1) 16 128 *)
-  0x3dc0140c;       (* arm_LDR Q12 X0 (Immediate_Offset (word 80)) *)
-  0x6e668562;       (* arm_SUB_VEC Q2 Q11 Q6 16 128 *)
-  0x6f47423f;       (* arm_MLS_VEC Q31 Q17 (Q7 :> LANE_H 0) 16 128 *)
-  0x4e6d854b;       (* arm_ADD_VEC Q11 Q10 Q13 16 128 *)
-  0x6e6d854a;       (* arm_SUB_VEC Q10 Q10 Q13 16 128 *)
-  0x3d807002;       (* arm_STR Q2 X0 (Immediate_Offset (word 448)) *)
-  0x4f418375;       (* arm_MUL_VEC Q21 Q27 (Q1 :> LANE_H 0) 16 128 *)
-  0x6e658591;       (* arm_SUB_VEC Q17 Q12 Q5 16 128 *)
-  0x3d80100a;       (* arm_STR Q10 X0 (Immediate_Offset (word 64)) *)
-  0x4e748666;       (* arm_ADD_VEC Q6 Q19 Q20 16 128 *)
-  0x6f474115;       (* arm_MLS_VEC Q21 Q8 (Q7 :> LANE_H 0) 16 128 *)
-  0x6e7a853d;       (* arm_SUB_VEC Q29 Q9 Q26 16 128 *)
-  0x4e7f85e4;       (* arm_ADD_VEC Q4 Q15 Q31 16 128 *)
-  0x6e7085d6;       (* arm_SUB_VEC Q22 Q14 Q16 16 128 *)
-  0x4f50dbad;       (* arm_SQRDMULH_VEC Q13 Q29 (Q0 :> LANE_H 5) 16 128 *)
-  0x3d804004;       (* arm_STR Q4 X0 (Immediate_Offset (word 256)) *)
-  0x4e63872e;       (* arm_ADD_VEC Q14 Q25 Q3 16 128 *)
-  0x4f70d0ca;       (* arm_SQRDMULH_VEC Q10 Q6 (Q0 :> LANE_H 3) 16 128 *)
-  0x6e7586dc;       (* arm_SUB_VEC Q28 Q22 Q21 16 128 *)
-  0x6e7f85fb;       (* arm_SUB_VEC Q27 Q15 Q31 16 128 *)
-  0x4f408bbf;       (* arm_MUL_VEC Q31 Q29 (Q0 :> LANE_H 4) 16 128 *)
-  0x4e7586de;       (* arm_ADD_VEC Q30 Q22 Q21 16 128 *)
-  0x4e7a8538;       (* arm_ADD_VEC Q24 Q9 Q26 16 128 *)
-  0x6f4741bf;       (* arm_MLS_VEC Q31 Q13 (Q7 :> LANE_H 0) 16 128 *)
-  0x6e74866d;       (* arm_SUB_VEC Q13 Q19 Q20 16 128 *)
-  0x3d80201e;       (* arm_STR Q30 X0 (Immediate_Offset (word 128)) *)
-  0x3d80501b;       (* arm_STR Q27 X0 (Immediate_Offset (word 320)) *)
-  0x4f70d302;       (* arm_SQRDMULH_VEC Q2 Q24 (Q0 :> LANE_H 3) 16 128 *)
-  0x3d80301c;       (* arm_STR Q28 X0 (Immediate_Offset (word 192)) *)
-  0x3c81040b;       (* arm_STR Q11 X0 (Postimmediate_Offset (word 16)) *)
-  0x4f4089ab;       (* arm_MUL_VEC Q11 Q13 (Q0 :> LANE_H 4) 16 128 *)
+  0x3dc06411;       (* arm_LDR Q17 X0 (Immediate_Offset (word 400)) *)
+  0x4f608a76;       (* arm_MUL_VEC Q22 Q19 (Q0 :> LANE_H 6) 16 128 *)
+  0x3dc04418;       (* arm_LDR Q24 X0 (Immediate_Offset (word 272)) *)
+  0x4e6d8653;       (* arm_ADD_VEC Q19 Q18 Q13 16 128 *)
+  0x6f4742b6;       (* arm_MLS_VEC Q22 Q21 (Q7 :> LANE_H 0) 16 128 *)
+  0x6e6d8655;       (* arm_SUB_VEC Q21 Q18 Q13 16 128 *)
+  0x3dc0340d;       (* arm_LDR Q13 X0 (Immediate_Offset (word 208)) *)
+  0x3dc01412;       (* arm_LDR Q18 X0 (Immediate_Offset (word 80)) *)
+  0x4f50d22e;       (* arm_SQRDMULH_VEC Q14 Q17 (Q0 :> LANE_H 1) 16 128 *)
+  0x3dc0541e;       (* arm_LDR Q30 X0 (Immediate_Offset (word 336)) *)
+  0x3dc07404;       (* arm_LDR Q4 X0 (Immediate_Offset (word 464)) *)
+  0x4e698562;       (* arm_ADD_VEC Q2 Q11 Q9 16 128 *)
+  0x4f70d2fb;       (* arm_SQRDMULH_VEC Q27 Q23 (Q0 :> LANE_H 3) 16 128 *)
+  0x3dc0040b;       (* arm_LDR Q11 X0 (Immediate_Offset (word 16)) *)
+  0x6e7a86b0;       (* arm_SUB_VEC Q16 Q21 Q26 16 128 *)
+  0x3dc02406;       (* arm_LDR Q6 X0 (Immediate_Offset (word 144)) *)
+  0x6e63867d;       (* arm_SUB_VEC Q29 Q19 Q3 16 128 *)
+  0x4f6082ef;       (* arm_MUL_VEC Q15 Q23 (Q0 :> LANE_H 2) 16 128 *)
+  0x4e7a86ac;       (* arm_ADD_VEC Q12 Q21 Q26 16 128 *)
+  0x4f50d3da;       (* arm_SQRDMULH_VEC Q26 Q30 (Q0 :> LANE_H 1) 16 128 *)
+  0x4e638663;       (* arm_ADD_VEC Q3 Q19 Q3 16 128 *)
+  0x3d80501d;       (* arm_STR Q29 X0 (Immediate_Offset (word 320)) *)
+  0x6f47436f;       (* arm_MLS_VEC Q15 Q27 (Q7 :> LANE_H 0) 16 128 *)
+  0x3d804003;       (* arm_STR Q3 X0 (Immediate_Offset (word 256)) *)
+  0x3d80600c;       (* arm_STR Q12 X0 (Immediate_Offset (word 384)) *)
+  0x4f40822a;       (* arm_MUL_VEC Q10 Q17 (Q0 :> LANE_H 0) 16 128 *)
+  0x3d807010;       (* arm_STR Q16 X0 (Immediate_Offset (word 448)) *)
+  0x6f4741ca;       (* arm_MLS_VEC Q10 Q14 (Q7 :> LANE_H 0) 16 128 *)
+  0x6e6f8451;       (* arm_SUB_VEC Q17 Q2 Q15 16 128 *)
+  0x4f4083cc;       (* arm_MUL_VEC Q12 Q30 (Q0 :> LANE_H 0) 16 128 *)
+  0x6e7c8630;       (* arm_SUB_VEC Q16 Q17 Q28 16 128 *)
+  0x6f47434c;       (* arm_MLS_VEC Q12 Q26 (Q7 :> LANE_H 0) 16 128 *)
+  0x6e6a84d9;       (* arm_SUB_VEC Q25 Q6 Q10 16 128 *)
+  0x3d803010;       (* arm_STR Q16 X0 (Immediate_Offset (word 192)) *)
+  0x4f50d308;       (* arm_SQRDMULH_VEC Q8 Q24 (Q0 :> LANE_H 1) 16 128 *)
+  0x4e6a84d7;       (* arm_ADD_VEC Q23 Q6 Q10 16 128 *)
+  0x4f50d08e;       (* arm_SQRDMULH_VEC Q14 Q4 (Q0 :> LANE_H 1) 16 128 *)
+  0x4e6c8650;       (* arm_ADD_VEC Q16 Q18 Q12 16 128 *)
+  0x4f408309;       (* arm_MUL_VEC Q9 Q24 (Q0 :> LANE_H 0) 16 128 *)
+  0x6e6c8645;       (* arm_SUB_VEC Q5 Q18 Q12 16 128 *)
+  0x4e7c863a;       (* arm_ADD_VEC Q26 Q17 Q28 16 128 *)
+  0x4f408095;       (* arm_MUL_VEC Q21 Q4 (Q0 :> LANE_H 0) 16 128 *)
+  0x4e6f845b;       (* arm_ADD_VEC Q27 Q2 Q15 16 128 *)
+  0x3d80201a;       (* arm_STR Q26 X0 (Immediate_Offset (word 128)) *)
+  0x6f4741d5;       (* arm_MLS_VEC Q21 Q14 (Q7 :> LANE_H 0) 16 128 *)
+  0x6e76876c;       (* arm_SUB_VEC Q12 Q27 Q22 16 128 *)
+  0x4e76877d;       (* arm_ADD_VEC Q29 Q27 Q22 16 128 *)
+  0x6f474109;       (* arm_MLS_VEC Q9 Q8 (Q7 :> LANE_H 0) 16 128 *)
+  0x3d80100c;       (* arm_STR Q12 X0 (Immediate_Offset (word 64)) *)
+  0x3c81041d;       (* arm_STR Q29 X0 (Postimmediate_Offset (word 16)) *)
+  0x4f50db32;       (* arm_SQRDMULH_VEC Q18 Q25 (Q0 :> LANE_H 5) 16 128 *)
+  0x6e7585ba;       (* arm_SUB_VEC Q26 Q13 Q21 16 128 *)
+  0x4e7585b5;       (* arm_ADD_VEC Q21 Q13 Q21 16 128 *)
+  0x4f408b2d;       (* arm_MUL_VEC Q13 Q25 (Q0 :> LANE_H 4) 16 128 *)
+  0x4f50db5c;       (* arm_SQRDMULH_VEC Q28 Q26 (Q0 :> LANE_H 5) 16 128 *)
+  0x4f70d2af;       (* arm_SQRDMULH_VEC Q15 Q21 (Q0 :> LANE_H 3) 16 128 *)
+  0x4f408b5f;       (* arm_MUL_VEC Q31 Q26 (Q0 :> LANE_H 4) 16 128 *)
+  0x6f47439f;       (* arm_MLS_VEC Q31 Q28 (Q7 :> LANE_H 0) 16 128 *)
+  0x4f6082bb;       (* arm_MUL_VEC Q27 Q21 (Q0 :> LANE_H 2) 16 128 *)
+  0x6f4741fb;       (* arm_MLS_VEC Q27 Q15 (Q7 :> LANE_H 0) 16 128 *)
+  0x4e7f84aa;       (* arm_ADD_VEC Q10 Q5 Q31 16 128 *)
+  0x6f47424d;       (* arm_MLS_VEC Q13 Q18 (Q7 :> LANE_H 0) 16 128 *)
+  0x6e698572;       (* arm_SUB_VEC Q18 Q11 Q9 16 128 *)
+  0x6e7f84ae;       (* arm_SUB_VEC Q14 Q5 Q31 16 128 *)
+  0x4f71d159;       (* arm_SQRDMULH_VEC Q25 Q10 (Q1 :> LANE_H 3) 16 128 *)
+  0x6e7b861a;       (* arm_SUB_VEC Q26 Q16 Q27 16 128 *)
+  0x4e7b8613;       (* arm_ADD_VEC Q19 Q16 Q27 16 128 *)
+  0x4f618143;       (* arm_MUL_VEC Q3 Q10 (Q1 :> LANE_H 2) 16 128 *)
+  0x4f51d35d;       (* arm_SQRDMULH_VEC Q29 Q26 (Q1 :> LANE_H 1) 16 128 *)
+  0x4f41835c;       (* arm_MUL_VEC Q28 Q26 (Q1 :> LANE_H 0) 16 128 *)
+  0x6f474323;       (* arm_MLS_VEC Q3 Q25 (Q7 :> LANE_H 0) 16 128 *)
+  0x6f4743bc;       (* arm_MLS_VEC Q28 Q29 (Q7 :> LANE_H 0) 16 128 *)
+  0x4f51d9c4;       (* arm_SQRDMULH_VEC Q4 Q14 (Q1 :> LANE_H 5) 16 128 *)
+  0x4f4189da;       (* arm_MUL_VEC Q26 Q14 (Q1 :> LANE_H 4) 16 128 *)
+  0x4f70da75;       (* arm_SQRDMULH_VEC Q21 Q19 (Q0 :> LANE_H 7) 16 128 *)
+  0x6f47409a;       (* arm_MLS_VEC Q26 Q4 (Q7 :> LANE_H 0) 16 128 *)
   0xd1000484;       (* arm_SUB X4 X4 (rvalue (word 1)) *)
   0xb5fff664;       (* arm_CBNZ X4 (word 2096844) *)
-  0x6e7f863d;       (* arm_SUB_VEC Q29 Q17 Q31 16 128 *)
-  0x4f6080c4;       (* arm_MUL_VEC Q4 Q6 (Q0 :> LANE_H 2) 16 128 *)
-  0x6e638733;       (* arm_SUB_VEC Q19 Q25 Q3 16 128 *)
-  0x4e658596;       (* arm_ADD_VEC Q22 Q12 Q5 16 128 *)
-  0x6f474144;       (* arm_MLS_VEC Q4 Q10 (Q7 :> LANE_H 0) 16 128 *)
-  0x4f608315;       (* arm_MUL_VEC Q21 Q24 (Q0 :> LANE_H 2) 16 128 *)
-  0x6f474055;       (* arm_MLS_VEC Q21 Q2 (Q7 :> LANE_H 0) 16 128 *)
-  0x6e6485dc;       (* arm_SUB_VEC Q28 Q14 Q4 16 128 *)
-  0x4f50d9a9;       (* arm_SQRDMULH_VEC Q9 Q13 (Q0 :> LANE_H 5) 16 128 *)
-  0x4e6485d7;       (* arm_ADD_VEC Q23 Q14 Q4 16 128 *)
-  0x4f51dba8;       (* arm_SQRDMULH_VEC Q8 Q29 (Q1 :> LANE_H 5) 16 128 *)
-  0x4f418bb4;       (* arm_MUL_VEC Q20 Q29 (Q1 :> LANE_H 4) 16 128 *)
-  0x4e7586c6;       (* arm_ADD_VEC Q6 Q22 Q21 16 128 *)
-  0x4f70d8de;       (* arm_SQRDMULH_VEC Q30 Q6 (Q0 :> LANE_H 7) 16 128 *)
-  0x6f474114;       (* arm_MLS_VEC Q20 Q8 (Q7 :> LANE_H 0) 16 128 *)
-  0x4f6088c8;       (* arm_MUL_VEC Q8 Q6 (Q0 :> LANE_H 6) 16 128 *)
-  0x4e7f8639;       (* arm_ADD_VEC Q25 Q17 Q31 16 128 *)
-  0x6f4743c8;       (* arm_MLS_VEC Q8 Q30 (Q7 :> LANE_H 0) 16 128 *)
-  0x4f71d33a;       (* arm_SQRDMULH_VEC Q26 Q25 (Q1 :> LANE_H 3) 16 128 *)
-  0x6e7586c5;       (* arm_SUB_VEC Q5 Q22 Q21 16 128 *)
-  0x6f47412b;       (* arm_MLS_VEC Q11 Q9 (Q7 :> LANE_H 0) 16 128 *)
-  0x4e6886e9;       (* arm_ADD_VEC Q9 Q23 Q8 16 128 *)
-  0x4f618323;       (* arm_MUL_VEC Q3 Q25 (Q1 :> LANE_H 2) 16 128 *)
-  0x6e6886e6;       (* arm_SUB_VEC Q6 Q23 Q8 16 128 *)
-  0x3c810409;       (* arm_STR Q9 X0 (Postimmediate_Offset (word 16)) *)
-  0x3d800c06;       (* arm_STR Q6 X0 (Immediate_Offset (word 48)) *)
-  0x4f51d0bf;       (* arm_SQRDMULH_VEC Q31 Q5 (Q1 :> LANE_H 1) 16 128 *)
-  0x4e6b867b;       (* arm_ADD_VEC Q27 Q19 Q11 16 128 *)
-  0x6f474343;       (* arm_MLS_VEC Q3 Q26 (Q7 :> LANE_H 0) 16 128 *)
-  0x6e6b867a;       (* arm_SUB_VEC Q26 Q19 Q11 16 128 *)
-  0x4f4180aa;       (* arm_MUL_VEC Q10 Q5 (Q1 :> LANE_H 0) 16 128 *)
-  0x6e748749;       (* arm_SUB_VEC Q9 Q26 Q20 16 128 *)
-  0x4e74874f;       (* arm_ADD_VEC Q15 Q26 Q20 16 128 *)
-  0x6f4743ea;       (* arm_MLS_VEC Q10 Q31 (Q7 :> LANE_H 0) 16 128 *)
-  0x3d806c09;       (* arm_STR Q9 X0 (Immediate_Offset (word 432)) *)
-  0x4e63877d;       (* arm_ADD_VEC Q29 Q27 Q3 16 128 *)
-  0x3d805c0f;       (* arm_STR Q15 X0 (Immediate_Offset (word 368)) *)
-  0x3d803c1d;       (* arm_STR Q29 X0 (Immediate_Offset (word 240)) *)
-  0x6e638764;       (* arm_SUB_VEC Q4 Q27 Q3 16 128 *)
-  0x6e6a879a;       (* arm_SUB_VEC Q26 Q28 Q10 16 128 *)
-  0x4e6a878f;       (* arm_ADD_VEC Q15 Q28 Q10 16 128 *)
-  0x3d804c04;       (* arm_STR Q4 X0 (Immediate_Offset (word 304)) *)
-  0x3d802c1a;       (* arm_STR Q26 X0 (Immediate_Offset (word 176)) *)
-  0x3d801c0f;       (* arm_STR Q15 X0 (Immediate_Offset (word 112)) *)
+  0x4e6d8654;       (* arm_ADD_VEC Q20 Q18 Q13 16 128 *)
+  0x4f70d2f0;       (* arm_SQRDMULH_VEC Q16 Q23 (Q0 :> LANE_H 3) 16 128 *)
+  0x6e6d8648;       (* arm_SUB_VEC Q8 Q18 Q13 16 128 *)
+  0x6e638685;       (* arm_SUB_VEC Q5 Q20 Q3 16 128 *)
+  0x4f6082fb;       (* arm_MUL_VEC Q27 Q23 (Q0 :> LANE_H 2) 16 128 *)
+  0x4e69857f;       (* arm_ADD_VEC Q31 Q11 Q9 16 128 *)
+  0x4e7a850e;       (* arm_ADD_VEC Q14 Q8 Q26 16 128 *)
+  0x6e7a851a;       (* arm_SUB_VEC Q26 Q8 Q26 16 128 *)
+  0x3d805005;       (* arm_STR Q5 X0 (Immediate_Offset (word 320)) *)
+  0x6f47421b;       (* arm_MLS_VEC Q27 Q16 (Q7 :> LANE_H 0) 16 128 *)
+  0x3d80600e;       (* arm_STR Q14 X0 (Immediate_Offset (word 384)) *)
+  0x4f608a79;       (* arm_MUL_VEC Q25 Q19 (Q0 :> LANE_H 6) 16 128 *)
+  0x3d80701a;       (* arm_STR Q26 X0 (Immediate_Offset (word 448)) *)
+  0x6f4742b9;       (* arm_MLS_VEC Q25 Q21 (Q7 :> LANE_H 0) 16 128 *)
+  0x6e7b87fa;       (* arm_SUB_VEC Q26 Q31 Q27 16 128 *)
+  0x4e63868f;       (* arm_ADD_VEC Q15 Q20 Q3 16 128 *)
+  0x4e7b87fd;       (* arm_ADD_VEC Q29 Q31 Q27 16 128 *)
+  0x6e7c8756;       (* arm_SUB_VEC Q22 Q26 Q28 16 128 *)
+  0x3d80400f;       (* arm_STR Q15 X0 (Immediate_Offset (word 256)) *)
+  0x4e7c875a;       (* arm_ADD_VEC Q26 Q26 Q28 16 128 *)
+  0x6e7987bb;       (* arm_SUB_VEC Q27 Q29 Q25 16 128 *)
+  0x4e7987b4;       (* arm_ADD_VEC Q20 Q29 Q25 16 128 *)
+  0x3d80201a;       (* arm_STR Q26 X0 (Immediate_Offset (word 128)) *)
+  0x3d803016;       (* arm_STR Q22 X0 (Immediate_Offset (word 192)) *)
+  0x3d80101b;       (* arm_STR Q27 X0 (Immediate_Offset (word 64)) *)
+  0x3c810414;       (* arm_STR Q20 X0 (Postimmediate_Offset (word 16)) *)
   0xaa0303e0;       (* arm_MOV X0 X3 *)
   0xd2800104;       (* arm_MOV X4 (rvalue (word 8)) *)
-  0x3dc00c10;       (* arm_LDR Q16 X0 (Immediate_Offset (word 48)) *)
-  0x3cc10426;       (* arm_LDR Q6 X1 (Postimmediate_Offset (word 16)) *)
-  0x3dc00014;       (* arm_LDR Q20 X0 (Immediate_Offset (word 0)) *)
-  0x4f56d20d;       (* arm_SQRDMULH_VEC Q13 Q16 (Q6 :> LANE_H 1) 16 128 *)
-  0x3dc0080a;       (* arm_LDR Q10 X0 (Immediate_Offset (word 32)) *)
-  0x3dc0041d;       (* arm_LDR Q29 X0 (Immediate_Offset (word 16)) *)
-  0x3dc00c52;       (* arm_LDR Q18 X2 (Immediate_Offset (word 48)) *)
-  0x4f46821b;       (* arm_MUL_VEC Q27 Q16 (Q6 :> LANE_H 0) 16 128 *)
-  0x3dc01045;       (* arm_LDR Q5 X2 (Immediate_Offset (word 64)) *)
-  0x4f56d15a;       (* arm_SQRDMULH_VEC Q26 Q10 (Q6 :> LANE_H 1) 16 128 *)
-  0x6f4741bb;       (* arm_MLS_VEC Q27 Q13 (Q7 :> LANE_H 0) 16 128 *)
-  0x4f46814e;       (* arm_MUL_VEC Q14 Q10 (Q6 :> LANE_H 0) 16 128 *)
-  0x6f47434e;       (* arm_MLS_VEC Q14 Q26 (Q7 :> LANE_H 0) 16 128 *)
-  0x6e7b87ad;       (* arm_SUB_VEC Q13 Q29 Q27 16 128 *)
-  0x4f56d9b6;       (* arm_SQRDMULH_VEC Q22 Q13 (Q6 :> LANE_H 5) 16 128 *)
-  0x4e7b87b0;       (* arm_ADD_VEC Q16 Q29 Q27 16 128 *)
-  0x4f4689be;       (* arm_MUL_VEC Q30 Q13 (Q6 :> LANE_H 4) 16 128 *)
-  0x6e6e869f;       (* arm_SUB_VEC Q31 Q20 Q14 16 128 *)
-  0x4f76d21a;       (* arm_SQRDMULH_VEC Q26 Q16 (Q6 :> LANE_H 3) 16 128 *)
-  0x6f4742de;       (* arm_MLS_VEC Q30 Q22 (Q7 :> LANE_H 0) 16 128 *)
-  0x4f66821d;       (* arm_MUL_VEC Q29 Q16 (Q6 :> LANE_H 2) 16 128 *)
-  0x6f47435d;       (* arm_MLS_VEC Q29 Q26 (Q7 :> LANE_H 0) 16 128 *)
+  0x3cc1042b;       (* arm_LDR Q11 X1 (Postimmediate_Offset (word 16)) *)
+  0x3dc00c09;       (* arm_LDR Q9 X0 (Immediate_Offset (word 48)) *)
+  0x3dc0081e;       (* arm_LDR Q30 X0 (Immediate_Offset (word 32)) *)
+  0x3cc6044c;       (* arm_LDR Q12 X2 (Postimmediate_Offset (word 96)) *)
+  0x3cdc0045;       (* arm_LDR Q5 X2 (Immediate_Offset (word 18446744073709551552)) *)
+  0x4f5bd137;       (* arm_SQRDMULH_VEC Q23 Q9 (Q11 :> LANE_H 1) 16 128 *)
+  0x3dc0000f;       (* arm_LDR Q15 X0 (Immediate_Offset (word 0)) *)
+  0x4f4b8126;       (* arm_MUL_VEC Q6 Q9 (Q11 :> LANE_H 0) 16 128 *)
+  0x3dc0041c;       (* arm_LDR Q28 X0 (Immediate_Offset (word 16)) *)
+  0x4f5bd3ca;       (* arm_SQRDMULH_VEC Q10 Q30 (Q11 :> LANE_H 1) 16 128 *)
+  0x6f4742e6;       (* arm_MLS_VEC Q6 Q23 (Q7 :> LANE_H 0) 16 128 *)
+  0x4f4b83c0;       (* arm_MUL_VEC Q0 Q30 (Q11 :> LANE_H 0) 16 128 *)
+  0x6f474140;       (* arm_MLS_VEC Q0 Q10 (Q7 :> LANE_H 0) 16 128 *)
+  0x3cdd0055;       (* arm_LDR Q21 X2 (Immediate_Offset (word 18446744073709551568)) *)
+  0x4e66879b;       (* arm_ADD_VEC Q27 Q28 Q6 16 128 *)
+  0x6e668799;       (* arm_SUB_VEC Q25 Q28 Q6 16 128 *)
+  0x4f6b8366;       (* arm_MUL_VEC Q6 Q27 (Q11 :> LANE_H 2) 16 128 *)
+  0x4f7bd371;       (* arm_SQRDMULH_VEC Q17 Q27 (Q11 :> LANE_H 3) 16 128 *)
+  0x4f5bdb33;       (* arm_SQRDMULH_VEC Q19 Q25 (Q11 :> LANE_H 5) 16 128 *)
+  0x3cdb0052;       (* arm_LDR Q18 X2 (Immediate_Offset (word 18446744073709551536)) *)
+  0x4f4b8b36;       (* arm_MUL_VEC Q22 Q25 (Q11 :> LANE_H 4) 16 128 *)
+  0x6f474226;       (* arm_MLS_VEC Q6 Q17 (Q7 :> LANE_H 0) 16 128 *)
+  0x6f474276;       (* arm_MLS_VEC Q22 Q19 (Q7 :> LANE_H 0) 16 128 *)
   0xd1000484;       (* arm_SUB X4 X4 (rvalue (word 1)) *)
-  0x3dc01811;       (* arm_LDR Q17 X0 (Immediate_Offset (word 96)) *)
-  0x3cc10428;       (* arm_LDR Q8 X1 (Postimmediate_Offset (word 16)) *)
-  0x6e7e87f0;       (* arm_SUB_VEC Q16 Q31 Q30 16 128 *)
-  0x4e7e87f7;       (* arm_ADD_VEC Q23 Q31 Q30 16 128 *)
-  0x4e6e8683;       (* arm_ADD_VEC Q3 Q20 Q14 16 128 *)
-  0x3dc01c09;       (* arm_LDR Q9 X0 (Immediate_Offset (word 112)) *)
-  0x4e902aec;       (* arm_TRN1 Q12 Q23 Q16 32 128 *)
-  0x3dc01014;       (* arm_LDR Q20 X0 (Immediate_Offset (word 64)) *)
-  0x4f58d222;       (* arm_SQRDMULH_VEC Q2 Q17 (Q8 :> LANE_H 1) 16 128 *)
-  0x6e7d847e;       (* arm_SUB_VEC Q30 Q3 Q29 16 128 *)
-  0x3dc01404;       (* arm_LDR Q4 X0 (Immediate_Offset (word 80)) *)
-  0x4e7d846b;       (* arm_ADD_VEC Q11 Q3 Q29 16 128 *)
-  0x4e906ae3;       (* arm_TRN2 Q3 Q23 Q16 32 128 *)
-  0x4f58d120;       (* arm_SQRDMULH_VEC Q0 Q9 (Q8 :> LANE_H 1) 16 128 *)
-  0x3dc00457;       (* arm_LDR Q23 X2 (Immediate_Offset (word 16)) *)
-  0x4e9e696e;       (* arm_TRN2 Q14 Q11 Q30 32 128 *)
-  0x4e9e296d;       (* arm_TRN1 Q13 Q11 Q30 32 128 *)
-  0x3cc60453;       (* arm_LDR Q19 X2 (Postimmediate_Offset (word 96)) *)
-  0x4f48812a;       (* arm_MUL_VEC Q10 Q9 (Q8 :> LANE_H 0) 16 128 *)
-  0x4ec369cf;       (* arm_TRN2 Q15 Q14 Q3 64 128 *)
-  0x3cdf0049;       (* arm_LDR Q9 X2 (Immediate_Offset (word 18446744073709551600)) *)
-  0x4ecc69be;       (* arm_TRN2 Q30 Q13 Q12 64 128 *)
-  0x6e77b5ff;       (* arm_SQRDMULH_VEC Q31 Q15 Q23 16 128 *)
-  0x4ecc29ac;       (* arm_TRN1 Q12 Q13 Q12 64 128 *)
-  0x4e739de6;       (* arm_MUL_VEC Q6 Q15 Q19 16 128 *)
-  0x6e77b7cf;       (* arm_SQRDMULH_VEC Q15 Q30 Q23 16 128 *)
-  0x6f4743e6;       (* arm_MLS_VEC Q6 Q31 (Q7 :> LANE_H 0) 16 128 *)
-  0x4ec329d7;       (* arm_TRN1 Q23 Q14 Q3 64 128 *)
-  0x4e739fde;       (* arm_MUL_VEC Q30 Q30 Q19 16 128 *)
-  0x6f4741fe;       (* arm_MLS_VEC Q30 Q15 (Q7 :> LANE_H 0) 16 128 *)
-  0x3cdc0055;       (* arm_LDR Q21 X2 (Immediate_Offset (word 18446744073709551552)) *)
-  0x6e6686f0;       (* arm_SUB_VEC Q16 Q23 Q6 16 128 *)
-  0x6f47400a;       (* arm_MLS_VEC Q10 Q0 (Q7 :> LANE_H 0) 16 128 *)
-  0x6e69b61d;       (* arm_SQRDMULH_VEC Q29 Q16 Q9 16 128 *)
+  0x3dc01c1b;       (* arm_LDR Q27 X0 (Immediate_Offset (word 112)) *)
+  0x3cc10424;       (* arm_LDR Q4 X1 (Postimmediate_Offset (word 16)) *)
+  0x6e6085e1;       (* arm_SUB_VEC Q1 Q15 Q0 16 128 *)
+  0x3dc0181e;       (* arm_LDR Q30 X0 (Immediate_Offset (word 96)) *)
+  0x4e6085f7;       (* arm_ADD_VEC Q23 Q15 Q0 16 128 *)
+  0x4e76842b;       (* arm_ADD_VEC Q11 Q1 Q22 16 128 *)
+  0x3cdf004a;       (* arm_LDR Q10 X2 (Immediate_Offset (word 18446744073709551600)) *)
+  0x6e6686f8;       (* arm_SUB_VEC Q24 Q23 Q6 16 128 *)
+  0x4f54d379;       (* arm_SQRDMULH_VEC Q25 Q27 (Q4 :> LANE_H 1) 16 128 *)
   0x4e6686e9;       (* arm_ADD_VEC Q9 Q23 Q6 16 128 *)
-  0x6e7e8583;       (* arm_SUB_VEC Q3 Q12 Q30 16 128 *)
-  0x4e7e858f;       (* arm_ADD_VEC Q15 Q12 Q30 16 128 *)
-  0x6e72b53e;       (* arm_SQRDMULH_VEC Q30 Q9 Q18 16 128 *)
-  0x4e6a848b;       (* arm_ADD_VEC Q11 Q4 Q10 16 128 *)
-  0x4e659e0d;       (* arm_MUL_VEC Q13 Q16 Q5 16 128 *)
-  0x6f4743ad;       (* arm_MLS_VEC Q13 Q29 (Q7 :> LANE_H 0) 16 128 *)
-  0x4e759d2c;       (* arm_MUL_VEC Q12 Q9 Q21 16 128 *)
-  0x6f4743cc;       (* arm_MLS_VEC Q12 Q30 (Q7 :> LANE_H 0) 16 128 *)
-  0x6e6d8461;       (* arm_SUB_VEC Q1 Q3 Q13 16 128 *)
-  0x4f48822e;       (* arm_MUL_VEC Q14 Q17 (Q8 :> LANE_H 0) 16 128 *)
-  0x4e6d847f;       (* arm_ADD_VEC Q31 Q3 Q13 16 128 *)
-  0x6e6a8483;       (* arm_SUB_VEC Q3 Q4 Q10 16 128 *)
-  0x6f47404e;       (* arm_MLS_VEC Q14 Q2 (Q7 :> LANE_H 0) 16 128 *)
-  0x4e812bf3;       (* arm_TRN1 Q19 Q31 Q1 32 128 *)
-  0x6e6c85fd;       (* arm_SUB_VEC Q29 Q15 Q12 16 128 *)
-  0x4e6c85ec;       (* arm_ADD_VEC Q12 Q15 Q12 16 128 *)
-  0x4f58d869;       (* arm_SQRDMULH_VEC Q9 Q3 (Q8 :> LANE_H 5) 16 128 *)
-  0x4e816bf0;       (* arm_TRN2 Q16 Q31 Q1 32 128 *)
-  0x4f78d17a;       (* arm_SQRDMULH_VEC Q26 Q11 (Q8 :> LANE_H 3) 16 128 *)
-  0x4e9d698d;       (* arm_TRN2 Q13 Q12 Q29 32 128 *)
-  0x4e9d298c;       (* arm_TRN1 Q12 Q12 Q29 32 128 *)
-  0x3dc00c52;       (* arm_LDR Q18 X2 (Immediate_Offset (word 48)) *)
-  0x4f48887e;       (* arm_MUL_VEC Q30 Q3 (Q8 :> LANE_H 4) 16 128 *)
-  0x4ed069b7;       (* arm_TRN2 Q23 Q13 Q16 64 128 *)
-  0x4ed029a0;       (* arm_TRN1 Q0 Q13 Q16 64 128 *)
-  0x3dc01045;       (* arm_LDR Q5 X2 (Immediate_Offset (word 64)) *)
-  0x6f47413e;       (* arm_MLS_VEC Q30 Q9 (Q7 :> LANE_H 0) 16 128 *)
-  0x3d800c17;       (* arm_STR Q23 X0 (Immediate_Offset (word 48)) *)
-  0x3d800400;       (* arm_STR Q0 X0 (Immediate_Offset (word 16)) *)
-  0x4ed32996;       (* arm_TRN1 Q22 Q12 Q19 64 128 *)
-  0x4f68817d;       (* arm_MUL_VEC Q29 Q11 (Q8 :> LANE_H 2) 16 128 *)
-  0x4ed3698f;       (* arm_TRN2 Q15 Q12 Q19 64 128 *)
-  0x3c840416;       (* arm_STR Q22 X0 (Postimmediate_Offset (word 64)) *)
-  0x6e6e869f;       (* arm_SUB_VEC Q31 Q20 Q14 16 128 *)
-  0x6f47435d;       (* arm_MLS_VEC Q29 Q26 (Q7 :> LANE_H 0) 16 128 *)
-  0x3c9e000f;       (* arm_STR Q15 X0 (Immediate_Offset (word 18446744073709551584)) *)
+  0x6e768430;       (* arm_SUB_VEC Q16 Q1 Q22 16 128 *)
+  0x4f44837f;       (* arm_MUL_VEC Q31 Q27 (Q4 :> LANE_H 0) 16 128 *)
+  0x4e98692e;       (* arm_TRN2 Q14 Q9 Q24 32 128 *)
+  0x4f54d3c1;       (* arm_SQRDMULH_VEC Q1 Q30 (Q4 :> LANE_H 1) 16 128 *)
+  0x4e906968;       (* arm_TRN2 Q8 Q11 Q16 32 128 *)
+  0x4e90296b;       (* arm_TRN1 Q11 Q11 Q16 32 128 *)
+  0x4ec869d3;       (* arm_TRN2 Q19 Q14 Q8 64 128 *)
+  0x6f47433f;       (* arm_MLS_VEC Q31 Q25 (Q7 :> LANE_H 0) 16 128 *)
+  0x3dc0140f;       (* arm_LDR Q15 X0 (Immediate_Offset (word 80)) *)
+  0x4e982922;       (* arm_TRN1 Q2 Q9 Q24 32 128 *)
+  0x6e72b671;       (* arm_SQRDMULH_VEC Q17 Q19 Q18 16 128 *)
+  0x4ec829c9;       (* arm_TRN1 Q9 Q14 Q8 64 128 *)
+  0x4e6c9e7d;       (* arm_MUL_VEC Q29 Q19 Q12 16 128 *)
+  0x4ecb685b;       (* arm_TRN2 Q27 Q2 Q11 64 128 *)
+  0x4e7f85e0;       (* arm_ADD_VEC Q0 Q15 Q31 16 128 *)
+  0x6e7f85f0;       (* arm_SUB_VEC Q16 Q15 Q31 16 128 *)
+  0x6e72b76d;       (* arm_SQRDMULH_VEC Q13 Q27 Q18 16 128 *)
+  0x6f47423d;       (* arm_MLS_VEC Q29 Q17 (Q7 :> LANE_H 0) 16 128 *)
+  0x3cde0051;       (* arm_LDR Q17 X2 (Immediate_Offset (word 18446744073709551584)) *)
+  0x3dc0100f;       (* arm_LDR Q15 X0 (Immediate_Offset (word 64)) *)
+  0x4e6c9f78;       (* arm_MUL_VEC Q24 Q27 Q12 16 128 *)
+  0x4ecb2853;       (* arm_TRN1 Q19 Q2 Q11 64 128 *)
+  0x3dc00452;       (* arm_LDR Q18 X2 (Immediate_Offset (word 16)) *)
+  0x4f648006;       (* arm_MUL_VEC Q6 Q0 (Q4 :> LANE_H 2) 16 128 *)
+  0x3cc6044c;       (* arm_LDR Q12 X2 (Postimmediate_Offset (word 96)) *)
+  0x4e7d8539;       (* arm_ADD_VEC Q25 Q9 Q29 16 128 *)
+  0x6f4741b8;       (* arm_MLS_VEC Q24 Q13 (Q7 :> LANE_H 0) 16 128 *)
+  0x6e7d8534;       (* arm_SUB_VEC Q20 Q9 Q29 16 128 *)
+  0x6e75b737;       (* arm_SQRDMULH_VEC Q23 Q25 Q21 16 128 *)
+  0x4e659f23;       (* arm_MUL_VEC Q3 Q25 Q5 16 128 *)
+  0x4e78866d;       (* arm_ADD_VEC Q13 Q19 Q24 16 128 *)
+  0x6e6ab69b;       (* arm_SQRDMULH_VEC Q27 Q20 Q10 16 128 *)
+  0x6f4742e3;       (* arm_MLS_VEC Q3 Q23 (Q7 :> LANE_H 0) 16 128 *)
+  0x6e78867d;       (* arm_SUB_VEC Q29 Q19 Q24 16 128 *)
+  0x4e719e9a;       (* arm_MUL_VEC Q26 Q20 Q17 16 128 *)
+  0x6f47437a;       (* arm_MLS_VEC Q26 Q27 (Q7 :> LANE_H 0) 16 128 *)
+  0x4e6385bb;       (* arm_ADD_VEC Q27 Q13 Q3 16 128 *)
+  0x4f74d00e;       (* arm_SQRDMULH_VEC Q14 Q0 (Q4 :> LANE_H 3) 16 128 *)
+  0x6e6385b3;       (* arm_SUB_VEC Q19 Q13 Q3 16 128 *)
+  0x3cdc0045;       (* arm_LDR Q5 X2 (Immediate_Offset (word 18446744073709551552)) *)
+  0x4f4483c0;       (* arm_MUL_VEC Q0 Q30 (Q4 :> LANE_H 0) 16 128 *)
+  0x4e932b68;       (* arm_TRN1 Q8 Q27 Q19 32 128 *)
+  0x6e7a87b5;       (* arm_SUB_VEC Q21 Q29 Q26 16 128 *)
+  0x4e7a87ab;       (* arm_ADD_VEC Q11 Q29 Q26 16 128 *)
+  0x4e936b7e;       (* arm_TRN2 Q30 Q27 Q19 32 128 *)
+  0x4f54da13;       (* arm_SQRDMULH_VEC Q19 Q16 (Q4 :> LANE_H 5) 16 128 *)
+  0x4e95696a;       (* arm_TRN2 Q10 Q11 Q21 32 128 *)
+  0x4f448a16;       (* arm_MUL_VEC Q22 Q16 (Q4 :> LANE_H 4) 16 128 *)
+  0x4e95297c;       (* arm_TRN1 Q28 Q11 Q21 32 128 *)
+  0x4eca2bdd;       (* arm_TRN1 Q29 Q30 Q10 64 128 *)
+  0x3cdd0055;       (* arm_LDR Q21 X2 (Immediate_Offset (word 18446744073709551568)) *)
+  0x6f474020;       (* arm_MLS_VEC Q0 Q1 (Q7 :> LANE_H 0) 16 128 *)
+  0x4edc6914;       (* arm_TRN2 Q20 Q8 Q28 64 128 *)
+  0x4eca6bda;       (* arm_TRN2 Q26 Q30 Q10 64 128 *)
+  0x3d80041d;       (* arm_STR Q29 X0 (Immediate_Offset (word 16)) *)
+  0x4edc2903;       (* arm_TRN1 Q3 Q8 Q28 64 128 *)
+  0x6f474276;       (* arm_MLS_VEC Q22 Q19 (Q7 :> LANE_H 0) 16 128 *)
+  0x3d800814;       (* arm_STR Q20 X0 (Immediate_Offset (word 32)) *)
+  0x3d800c1a;       (* arm_STR Q26 X0 (Immediate_Offset (word 48)) *)
+  0x6f4741c6;       (* arm_MLS_VEC Q6 Q14 (Q7 :> LANE_H 0) 16 128 *)
+  0x3c840403;       (* arm_STR Q3 X0 (Postimmediate_Offset (word 64)) *)
   0xd1000484;       (* arm_SUB X4 X4 (rvalue (word 1)) *)
   0xb5fff704;       (* arm_CBNZ X4 (word 2096864) *)
-  0x4e6e868f;       (* arm_ADD_VEC Q15 Q20 Q14 16 128 *)
-  0x6e7e87f3;       (* arm_SUB_VEC Q19 Q31 Q30 16 128 *)
-  0x4e7e87ec;       (* arm_ADD_VEC Q12 Q31 Q30 16 128 *)
-  0x3dc01456;       (* arm_LDR Q22 X2 (Immediate_Offset (word 80)) *)
-  0x4e7d85fa;       (* arm_ADD_VEC Q26 Q15 Q29 16 128 *)
-  0x6e7d85ef;       (* arm_SUB_VEC Q15 Q15 Q29 16 128 *)
-  0x4e936982;       (* arm_TRN2 Q2 Q12 Q19 32 128 *)
-  0x4e932998;       (* arm_TRN1 Q24 Q12 Q19 32 128 *)
-  0x4e8f6b40;       (* arm_TRN2 Q0 Q26 Q15 32 128 *)
-  0x3dc0045e;       (* arm_LDR Q30 X2 (Immediate_Offset (word 16)) *)
-  0x3cc6044a;       (* arm_LDR Q10 X2 (Postimmediate_Offset (word 96)) *)
-  0x4e8f2b4e;       (* arm_TRN1 Q14 Q26 Q15 32 128 *)
-  0x3cdc0057;       (* arm_LDR Q23 X2 (Immediate_Offset (word 18446744073709551552)) *)
-  0x4ec26808;       (* arm_TRN2 Q8 Q0 Q2 64 128 *)
-  0x4ed869df;       (* arm_TRN2 Q31 Q14 Q24 64 128 *)
-  0x4ed829cc;       (* arm_TRN1 Q12 Q14 Q24 64 128 *)
-  0x6e7eb50f;       (* arm_SQRDMULH_VEC Q15 Q8 Q30 16 128 *)
-  0x4ec22813;       (* arm_TRN1 Q19 Q0 Q2 64 128 *)
-  0x4e6a9d03;       (* arm_MUL_VEC Q3 Q8 Q10 16 128 *)
-  0x6e7eb7fe;       (* arm_SQRDMULH_VEC Q30 Q31 Q30 16 128 *)
-  0x6f4741e3;       (* arm_MLS_VEC Q3 Q15 (Q7 :> LANE_H 0) 16 128 *)
-  0x4e6a9fef;       (* arm_MUL_VEC Q15 Q31 Q10 16 128 *)
-  0x6f4743cf;       (* arm_MLS_VEC Q15 Q30 (Q7 :> LANE_H 0) 16 128 *)
-  0x4e638666;       (* arm_ADD_VEC Q6 Q19 Q3 16 128 *)
-  0x6e638663;       (* arm_SUB_VEC Q3 Q19 Q3 16 128 *)
-  0x6e72b4de;       (* arm_SQRDMULH_VEC Q30 Q6 Q18 16 128 *)
-  0x4e779cd3;       (* arm_MUL_VEC Q19 Q6 Q23 16 128 *)
-  0x4e6f859f;       (* arm_ADD_VEC Q31 Q12 Q15 16 128 *)
-  0x6e6f858b;       (* arm_SUB_VEC Q11 Q12 Q15 16 128 *)
-  0x6e76b477;       (* arm_SQRDMULH_VEC Q23 Q3 Q22 16 128 *)
-  0x6f4743d3;       (* arm_MLS_VEC Q19 Q30 (Q7 :> LANE_H 0) 16 128 *)
-  0x4e659c60;       (* arm_MUL_VEC Q0 Q3 Q5 16 128 *)
-  0x6f4742e0;       (* arm_MLS_VEC Q0 Q23 (Q7 :> LANE_H 0) 16 128 *)
-  0x6e7387fe;       (* arm_SUB_VEC Q30 Q31 Q19 16 128 *)
-  0x4e7387ef;       (* arm_ADD_VEC Q15 Q31 Q19 16 128 *)
-  0x4e9e69f3;       (* arm_TRN2 Q19 Q15 Q30 32 128 *)
-  0x4e9e29ef;       (* arm_TRN1 Q15 Q15 Q30 32 128 *)
-  0x6e608577;       (* arm_SUB_VEC Q23 Q11 Q0 16 128 *)
-  0x4e60856c;       (* arm_ADD_VEC Q12 Q11 Q0 16 128 *)
-  0x4e972983;       (* arm_TRN1 Q3 Q12 Q23 32 128 *)
-  0x4e97699d;       (* arm_TRN2 Q29 Q12 Q23 32 128 *)
-  0x4ec329ed;       (* arm_TRN1 Q13 Q15 Q3 64 128 *)
-  0x4edd6a6c;       (* arm_TRN2 Q12 Q19 Q29 64 128 *)
-  0x4edd2a77;       (* arm_TRN1 Q23 Q19 Q29 64 128 *)
-  0x4ec369ef;       (* arm_TRN2 Q15 Q15 Q3 64 128 *)
-  0x3c84040d;       (* arm_STR Q13 X0 (Postimmediate_Offset (word 64)) *)
-  0x3c9f000c;       (* arm_STR Q12 X0 (Immediate_Offset (word 18446744073709551600)) *)
-  0x3c9e000f;       (* arm_STR Q15 X0 (Immediate_Offset (word 18446744073709551584)) *)
-  0x3c9d0017;       (* arm_STR Q23 X0 (Immediate_Offset (word 18446744073709551568)) *)
-  0x6d4027e8;       (* arm_LDP D8 D9 SP (Immediate_Offset (word 0)) *)
-  0x6d412fea;       (* arm_LDP D10 D11 SP (Immediate_Offset (word 16)) *)
-  0x6d4237ec;       (* arm_LDP D12 D13 SP (Immediate_Offset (word 32)) *)
-  0x6d433fee;       (* arm_LDP D14 D15 SP (Immediate_Offset (word 48)) *)
+  0x4e6085e4;       (* arm_ADD_VEC Q4 Q15 Q0 16 128 *)
+  0x6e6085ee;       (* arm_SUB_VEC Q14 Q15 Q0 16 128 *)
+  0x3cdf005a;       (* arm_LDR Q26 X2 (Immediate_Offset (word 18446744073709551600)) *)
+  0x4e7685c8;       (* arm_ADD_VEC Q8 Q14 Q22 16 128 *)
+  0x6e7685db;       (* arm_SUB_VEC Q27 Q14 Q22 16 128 *)
+  0x6e66848d;       (* arm_SUB_VEC Q13 Q4 Q6 16 128 *)
+  0x4e66849d;       (* arm_ADD_VEC Q29 Q4 Q6 16 128 *)
+  0x4e9b690b;       (* arm_TRN2 Q11 Q8 Q27 32 128 *)
+  0x4e8d6ba1;       (* arm_TRN2 Q1 Q29 Q13 32 128 *)
+  0x4e9b291b;       (* arm_TRN1 Q27 Q8 Q27 32 128 *)
+  0x4e8d2bb1;       (* arm_TRN1 Q17 Q29 Q13 32 128 *)
+  0x4ecb683c;       (* arm_TRN2 Q28 Q1 Q11 64 128 *)
+  0x4ecb2830;       (* arm_TRN1 Q16 Q1 Q11 64 128 *)
+  0x6e72b780;       (* arm_SQRDMULH_VEC Q0 Q28 Q18 16 128 *)
+  0x4edb6a33;       (* arm_TRN2 Q19 Q17 Q27 64 128 *)
+  0x4edb2a21;       (* arm_TRN1 Q1 Q17 Q27 64 128 *)
+  0x4e6c9f9b;       (* arm_MUL_VEC Q27 Q28 Q12 16 128 *)
+  0x6e72b669;       (* arm_SQRDMULH_VEC Q9 Q19 Q18 16 128 *)
+  0x6f47401b;       (* arm_MLS_VEC Q27 Q0 (Q7 :> LANE_H 0) 16 128 *)
+  0x4e6c9e74;       (* arm_MUL_VEC Q20 Q19 Q12 16 128 *)
+  0x6f474134;       (* arm_MLS_VEC Q20 Q9 (Q7 :> LANE_H 0) 16 128 *)
+  0x6e7b861e;       (* arm_SUB_VEC Q30 Q16 Q27 16 128 *)
+  0x4e7b8619;       (* arm_ADD_VEC Q25 Q16 Q27 16 128 *)
+  0x6e7ab7ce;       (* arm_SQRDMULH_VEC Q14 Q30 Q26 16 128 *)
+  0x3cde005a;       (* arm_LDR Q26 X2 (Immediate_Offset (word 18446744073709551584)) *)
+  0x6e75b73f;       (* arm_SQRDMULH_VEC Q31 Q25 Q21 16 128 *)
+  0x4e74843b;       (* arm_ADD_VEC Q27 Q1 Q20 16 128 *)
+  0x4e7a9fcf;       (* arm_MUL_VEC Q15 Q30 Q26 16 128 *)
+  0x6f4741cf;       (* arm_MLS_VEC Q15 Q14 (Q7 :> LANE_H 0) 16 128 *)
+  0x6e74843a;       (* arm_SUB_VEC Q26 Q1 Q20 16 128 *)
+  0x4e659f2c;       (* arm_MUL_VEC Q12 Q25 Q5 16 128 *)
+  0x6f4743ec;       (* arm_MLS_VEC Q12 Q31 (Q7 :> LANE_H 0) 16 128 *)
+  0x6e6f8742;       (* arm_SUB_VEC Q2 Q26 Q15 16 128 *)
+  0x4e6f8740;       (* arm_ADD_VEC Q0 Q26 Q15 16 128 *)
+  0x4e82680e;       (* arm_TRN2 Q14 Q0 Q2 32 128 *)
+  0x6e6c877a;       (* arm_SUB_VEC Q26 Q27 Q12 16 128 *)
+  0x4e6c877b;       (* arm_ADD_VEC Q27 Q27 Q12 16 128 *)
+  0x4e822811;       (* arm_TRN1 Q17 Q0 Q2 32 128 *)
+  0x4e9a2b65;       (* arm_TRN1 Q5 Q27 Q26 32 128 *)
+  0x4e9a6b7a;       (* arm_TRN2 Q26 Q27 Q26 32 128 *)
+  0x4ece2b59;       (* arm_TRN1 Q25 Q26 Q14 64 128 *)
+  0x4ed128a0;       (* arm_TRN1 Q0 Q5 Q17 64 128 *)
+  0x4ece6b55;       (* arm_TRN2 Q21 Q26 Q14 64 128 *)
+  0x4ed168ba;       (* arm_TRN2 Q26 Q5 Q17 64 128 *)
+  0x3d800419;       (* arm_STR Q25 X0 (Immediate_Offset (word 16)) *)
+  0x3c840400;       (* arm_STR Q0 X0 (Postimmediate_Offset (word 64)) *)
+  0x3c9f0015;       (* arm_STR Q21 X0 (Immediate_Offset (word 18446744073709551600)) *)
+  0x3c9e001a;       (* arm_STR Q26 X0 (Immediate_Offset (word 18446744073709551584)) *)
+  0x6d4027e8;       (* arm_LDP D8 D9 SP (Immediate_Offset (iword (&0))) *)
+  0x6d412fea;       (* arm_LDP D10 D11 SP (Immediate_Offset (iword (&16))) *)
+  0x6d4237ec;       (* arm_LDP D12 D13 SP (Immediate_Offset (iword (&32))) *)
+  0x6d433fee;       (* arm_LDP D14 D15 SP (Immediate_Offset (iword (&48))) *)
   0x910103ff;       (* arm_ADD SP SP (rvalue (word 64)) *)
   0xd65f03c0        (* arm_RET X30 *)
-]
-[192; 249; 123; 194; 19; 253; 51; 227; 216; 255; 118; 254; 81; 253; 150; 229;
- 118; 2; 57; 24; 104; 250; 241; 200; 80; 3; 155; 32; 0; 0; 0; 0; 38; 4; 213;
- 40; 40; 1; 98; 11; 142; 252; 22; 222; 0; 0; 0; 0; 126; 250; 201; 201; 59; 5;
- 124; 51; 196; 5; 193; 56; 0; 0; 0; 0; 193; 0; 108; 7; 229; 254; 30; 245; 56;
- 0; 39; 2; 0; 0; 0; 0; 29; 3; 165; 30; 191; 251; 33; 214; 53; 5; 65; 51; 0;
- 0; 0; 0; 225; 253; 31; 235; 146; 5; 212; 54; 45; 251; 132; 208; 0; 0; 0; 0;
- 187; 255; 89; 253; 23; 2; 146; 20; 65; 254; 208; 238; 0; 0; 0; 0; 57; 2;
- 225; 21; 88; 252; 3; 220; 62; 254; 179; 238; 0; 0; 0; 0; 209; 249; 34; 195;
- 181; 250; 230; 203; 53; 3; 145; 31; 0; 0; 0; 0; 33; 1; 33; 1; 75; 1; 75; 1;
- 180; 255; 180; 255; 219; 249; 219; 249; 29; 11; 29; 11; 186; 12; 186; 12;
- 20; 253; 20; 253; 133; 195; 133; 195; 17; 0; 17; 0; 71; 2; 71; 2; 101; 6;
- 101; 6; 239; 251; 239; 251; 167; 0; 167; 0; 107; 22; 107; 22; 241; 62; 241;
- 62; 249; 215; 249; 215; 200; 253; 200; 253; 88; 253; 88; 253; 211; 2; 211;
- 2; 76; 4; 76; 4; 41; 234; 41; 234; 219; 229; 219; 229; 205; 27; 205; 27; 76;
- 42; 76; 42; 173; 4; 173; 4; 255; 251; 255; 251; 228; 251; 228; 251; 6; 251;
- 6; 251; 6; 46; 6; 46; 151; 216; 151; 216; 141; 215; 141; 215; 4; 207; 4;
- 207; 129; 5; 129; 5; 208; 255; 208; 255; 244; 2; 244; 2; 198; 254; 198; 254;
- 45; 54; 45; 54; 40; 254; 40; 254; 17; 29; 17; 29; 237; 243; 237; 243; 101;
- 253; 101; 253; 233; 0; 233; 0; 107; 251; 107; 251; 233; 254; 233; 254; 91;
- 230; 91; 230; 245; 8; 245; 8; 230; 210; 230; 210; 70; 245; 70; 245; 138; 2;
- 138; 2; 184; 250; 184; 250; 208; 252; 208; 252; 120; 2; 120; 2; 254; 24;
- 254; 24; 4; 204; 4; 204; 160; 224; 160; 224; 77; 24; 77; 24; 166; 249; 166;
- 249; 228; 253; 228; 253; 54; 250; 54; 250; 181; 5; 181; 5; 123; 193; 123;
- 193; 61; 235; 61; 235; 4; 199; 4; 199; 45; 56; 45; 56; 115; 6; 115; 6; 252;
- 249; 252; 249; 184; 3; 184; 3; 126; 253; 126; 253; 123; 63; 123; 63; 201;
- 196; 201; 196; 155; 36; 155; 36; 81; 231; 81; 231; 48; 254; 48; 254; 33; 0;
- 33; 0; 40; 5; 40; 5; 122; 250; 122; 250; 41; 238; 41; 238; 69; 1; 69; 1;
- 193; 50; 193; 50; 162; 201; 162; 201; 171; 3; 171; 3; 132; 252; 132; 252;
- 221; 2; 221; 2; 12; 1; 12; 1; 27; 36; 27; 36; 180; 221; 180; 221; 47; 28;
- 47; 28; 78; 10; 78; 10; 3; 252; 3; 252; 83; 252; 83; 252; 32; 252; 32; 252;
- 129; 2; 129; 2; 190; 216; 190; 216; 210; 219; 210; 219; 220; 217; 220; 217;
- 165; 24; 165; 24; 14; 252; 14; 252; 155; 5; 155; 5; 39; 3; 39; 3; 196; 1;
- 196; 1; 42; 217; 42; 217; 45; 55; 45; 55; 7; 31; 7; 31; 97; 17; 97; 17; 48;
- 6; 48; 6; 244; 250; 244; 250; 119; 1; 119; 1; 41; 251; 41; 251; 232; 60;
- 232; 60; 83; 206; 83; 206; 107; 14; 107; 14; 92; 208; 92; 208; 249; 251;
- 249; 251; 147; 255; 147; 255; 244; 252; 244; 252; 109; 6; 109; 6; 92; 216;
- 92; 216; 207; 251; 207; 251; 2; 226; 2; 226; 64; 63; 64; 63; 158; 5; 158; 5;
- 51; 254; 51; 254; 254; 5; 254; 5; 97; 252; 97; 252; 75; 55; 75; 55; 70; 238;
- 70; 238; 251; 58; 251; 58; 91; 220; 91; 220; 39; 4; 39; 4; 212; 253; 212;
- 253; 50; 251; 50; 251; 161; 252; 161; 252; 223; 40; 223; 40; 159; 234; 159;
- 234; 181; 208; 181; 208; 209; 222; 209; 222; 63; 1; 63; 1; 245; 2; 245; 2;
- 49; 2; 49; 2; 33; 253; 33; 253; 68; 12; 68; 12; 27; 29; 27; 29; 146; 21;
- 146; 21; 189; 227; 189; 227; 86; 253; 86; 253; 56; 253; 56; 253; 201; 5;
- 201; 5; 136; 2; 136; 2; 199; 229; 199; 229; 160; 228; 160; 228; 242; 56;
- 242; 56; 234; 24; 234; 24; 243; 253; 243; 253; 147; 1; 147; 1; 119; 4; 119;
- 4; 214; 253; 214; 253; 208; 235; 208; 235; 127; 15; 127; 15; 243; 43; 243;
- 43; 179; 234; 179; 234; 68; 4; 68; 4; 2; 4; 2; 4; 101; 251; 101; 251; 118;
- 3; 118; 3; 253; 41; 253; 41; 115; 39; 115; 39; 171; 210; 171; 210; 17; 34;
- 17; 34; 169; 252; 169; 252; 37; 255; 37; 255; 203; 4; 203; 4; 142; 3; 142;
- 3; 32; 223; 32; 223; 148; 247; 148; 247; 46; 47; 46; 47; 253; 34; 253; 34;
- 185; 249; 185; 249; 81; 250; 81; 250; 61; 251; 61; 251; 117; 3; 117; 3; 54;
- 194; 54; 194; 14; 200; 14; 200; 33; 209; 33; 209; 7; 34; 7; 34; 188; 4; 188;
- 4; 5; 4; 5; 4; 118; 254; 118; 254; 105; 251; 105; 251; 154; 46; 154; 46;
- 145; 39; 145; 39; 218; 240; 218; 240; 210; 210; 210; 210];;
+];;
 
 let MLKEM_NTT_EXEC = ARM_MK_EXEC_RULE mlkem_ntt_mc;;
 
 (* ------------------------------------------------------------------------- *)
-(* Correctness proof.                                                        *)
+(* Data tables that are assumed in the precondition.                         *)
+(* ------------------------------------------------------------------------- *)
+
+let ntt_zetas_layer01234 = define
+ `ntt_zetas_layer01234:int list =
+   [-- &1600; -- &15749; -- &749; -- &7373; -- &40; -- &394; -- &687; -- &6762;
+    &630; &6201; -- &1432; -- &14095; &848; &8347; &0; &0; &1062; &10453; &296;
+    &2914; -- &882; -- &8682; &0; &0; -- &1410; -- &13879; &1339; &13180; &1476;
+    &14529; &0; &0; &193; &1900; -- &283; -- &2786; &56; &551; &0; &0; &797;
+    &7845; -- &1089; -- &10719; &1333; &13121; &0; &0; -- &543; -- &5345;
+    &1426; &14036; -- &1235; -- &12156; &0; &0; -- &69; -- &679; &535; &5266;
+    -- &447; -- &4400; &0; &0; &569; &5601; -- &936; -- &9213; -- &450;
+    -- &4429; &0; &0; -- &1583; -- &15582; -- &1355; -- &13338; &821;
+    &8081; &0; &0]`;;
+
+let ntt_zetas_layer56 = define
+`ntt_zetas_layer56:int list =
+  [&289; &289; &331; &331; -- &76; -- &76; -- &1573; -- &1573; &2845;
+   &2845; &3258; &3258; -- &748; -- &748; -- &15483; -- &15483; &17; &17;
+   &583; &583; &1637; &1637; -- &1041; -- &1041; &167; &167; &5739;
+   &5739; &16113; &16113; -- &10247; -- &10247; -- &568; -- &568;
+   -- &680; -- &680; &723; &723; &1100; &1100; -- &5591; -- &5591; -- &6693;
+   -- &6693; &7117; &7117; &10828; &10828; &1197; &1197; -- &1025;
+   -- &1025; -- &1052; -- &1052; -- &1274; -- &1274; &11782; &11782;
+   -- &10089; -- &10089; -- &10355; -- &10355; -- &12540; -- &12540; &1409;
+   &1409; -- &48; -- &48; &756; &756; -- &314; -- &314; &13869; &13869;
+   -- &472; -- &472; &7441; &7441; -- &3091; -- &3091; -- &667; -- &667;
+   &233; &233; -- &1173; -- &1173; -- &279; -- &279; -- &6565; -- &6565;
+   &2293; &2293; -- &11546; -- &11546; -- &2746; -- &2746; &650; &650;
+   -- &1352; -- &1352; -- &816; -- &816; &632; &632; &6398; &6398;
+   -- &13308; -- &13308; -- &8032; -- &8032; &6221; &6221; -- &1626;
+   -- &1626; -- &540; -- &540; -- &1482; -- &1482; &1461; &1461; -- &16005;
+   -- &16005; -- &5315; -- &5315; -- &14588; -- &14588; &14381; &14381;
+   &1651; &1651; -- &1540; -- &1540; &952; &952; -- &642; -- &642;
+   &16251; &16251; -- &15159; -- &15159; &9371; &9371; -- &6319;
+   -- &6319; -- &464; -- &464; &33; &33; &1320; &1320; -- &1414; -- &1414;
+   -- &4567; -- &4567; &325; &325; &12993; &12993; -- &13918; -- &13918;
+   &939; &939; -- &892; -- &892; &733; &733; &268; &268; &9243; &9243;
+   -- &8780; -- &8780; &7215; &7215; &2638; &2638; -- &1021; -- &1021;
+   -- &941; -- &941; -- &992; -- &992; &641; &641; -- &10050; -- &10050;
+   -- &9262; -- &9262; -- &9764; -- &9764; &6309; &6309; -- &1010; -- &1010;
+   &1435; &1435; &807; &807; &452; &452; -- &9942; -- &9942; &14125;
+   &14125; &7943; &7943; &4449; &4449; &1584; &1584; -- &1292; -- &1292;
+   &375; &375; -- &1239; -- &1239; &15592; &15592; -- &12717; -- &12717;
+   &3691; &3691; -- &12196; -- &12196; -- &1031; -- &1031; -- &109;
+   -- &109; -- &780; -- &780; &1645; &1645; -- &10148; -- &10148; -- &1073;
+   -- &1073; -- &7678; -- &7678; &16192; &16192; &1438; &1438; -- &461;
+   -- &461; &1534; &1534; -- &927; -- &927; &14155; &14155; -- &4538;
+   -- &4538; &15099; &15099; -- &9125; -- &9125; &1063; &1063; -- &556;
+   -- &556; -- &1230; -- &1230; -- &863; -- &863; &10463; &10463; -- &5473;
+   -- &5473; -- &12107; -- &12107; -- &8495; -- &8495; &319; &319; &757;
+   &757; &561; &561; -- &735; -- &735; &3140; &3140; &7451; &7451; &5522;
+   &5522; -- &7235; -- &7235; -- &682; -- &682; -- &712; -- &712; &1481;
+   &1481; &648; &648; -- &6713; -- &6713; -- &7008; -- &7008; &14578;
+   &14578; &6378; &6378; -- &525; -- &525; &403; &403; &1143; &1143;
+   -- &554; -- &554; -- &5168; -- &5168; &3967; &3967; &11251; &11251;
+   -- &5453; -- &5453; &1092; &1092; &1026; &1026; -- &1179; -- &1179; &886;
+   &886; &10749; &10749; &10099; &10099; -- &11605; -- &11605; &8721;
+   &8721; -- &855; -- &855; -- &219; -- &219; &1227; &1227; &910; &910;
+   -- &8416; -- &8416; -- &2156; -- &2156; &12078; &12078; &8957; &8957;
+   -- &1607; -- &1607; -- &1455; -- &1455; -- &1219; -- &1219; &885;
+   &885; -- &15818; -- &15818; -- &14322; -- &14322; -- &11999;
+   -- &11999; &8711; &8711; &1212; &1212; &1029; &1029; -- &394; -- &394;
+   -- &1175; -- &1175; &11930; &11930; &10129; &10129; -- &3878; -- &3878;
+   -- &11566; -- &11566]`;;
+
+let ntt_constants = define
+ `ntt_constants z_01234 z_56 s <=>
+        (!i. i < 80
+             ==> read(memory :> bytes16(word_add z_01234 (word(2 * i)))) s =
+                 iword(EL i ntt_zetas_layer01234)) /\
+        (!i. i < 384
+             ==> read(memory :> bytes16(word_add z_56 (word(2 * i)))) s =
+                 iword(EL i ntt_zetas_layer56))`;;
+
+(* ------------------------------------------------------------------------- *)
+(* Some convenient proof tools.                                              *)
 (* ------------------------------------------------------------------------- *)
 
 let READ_MEMORY_MERGE_CONV =
@@ -439,26 +456,33 @@ let SIMD_SIMPLIFY_TAC =
     CONV_RULE(RAND_CONV SIMD_SIMPLIFY_CONV) o
     check (simdable o concl)));;
 
-let BYTES_LOADED_DATA = prove
- (`bytes_loaded s (word (pc + 0x518)) mlkem_ntt_data <=>
-   read (memory :> bytes(word (pc + 0x518),928)) s =
-   num_of_bytelist mlkem_ntt_data`,
-  REWRITE_TAC[bytes_loaded; READ_BYTELIST_EQ_BYTES;
-    CONV_RULE (RAND_CONV LENGTH_CONV)
-     (AP_TERM `LENGTH:byte list->num` mlkem_ntt_data)]);;
+let MEMORY_128_FROM_16_TAC =
+  let a_tm = `a:int64` and n_tm = `n:num` and i64_ty = `:int64`
+  and pat = `read (memory :> bytes128(word_add a (word n))) s0` in
+  fun v n ->
+    let pat' = subst[mk_var(v,i64_ty),a_tm] pat in
+    let f i =
+      let itm = mk_small_numeral(16*i) in
+      READ_MEMORY_MERGE_CONV 3 (subst[itm,n_tm] pat') in
+    MP_TAC(end_itlist CONJ (map f (0--(n-1))));;
+
+(* ------------------------------------------------------------------------- *)
+(* Correctness proof.                                                        *)
+(* ------------------------------------------------------------------------- *)
 
 let MLKEM_NTT_CORRECT = prove
- (`!a x pc.
-      nonoverlapping (word pc,0x8b8) (a,512)
+ (`!a z_01234 z_56 x pc.
+      ALL (nonoverlapping (a,512))
+          [(word pc,0x504); (z_01234,160); (z_56,768)]
       ==> ensures arm
-           (\s. aligned_bytes_loaded s (word pc)
-                  (APPEND mlkem_ntt_mc mlkem_ntt_data) /\
+           (\s. aligned_bytes_loaded s (word pc) mlkem_ntt_mc /\
                 read PC s = word (pc + 0x14) /\
-                C_ARGUMENTS [a] s /\
+                C_ARGUMENTS [a; z_01234; z_56] s /\
+                ntt_constants z_01234 z_56 s /\
                 !i. i < 256
                     ==> read(memory :> bytes16(word_add a (word(2 * i)))) s =
                         x i)
-           (\s. read PC s = word(pc + 0x500) /\
+           (\s. read PC s = word(pc + 0x4ec) /\
                 ((!i. i < 256 ==> abs(ival(x i)) <= &8191)
                  ==> !i. i < 256
                          ==> let zi =
@@ -468,62 +492,41 @@ let MLKEM_NTT_CORRECT = prove
            (MAYCHANGE_REGS_AND_FLAGS_PERMITTED_BY_ABI ,,
             MAYCHANGE [Q8; Q9; Q10; Q11; Q12; Q13; Q14; Q15] ,,
             MAYCHANGE [memory :> bytes(a,512)])`,
-  MAP_EVERY X_GEN_TAC [`a:int64`; `x:num->int16`; `pc:num`] THEN
+  MAP_EVERY X_GEN_TAC
+   [`a:int64`; `z_01234:int64`; `z_56:int64`; `x:num->int16`; `pc:num`] THEN
   REWRITE_TAC[MAYCHANGE_REGS_AND_FLAGS_PERMITTED_BY_ABI; C_ARGUMENTS;
-              NONOVERLAPPING_CLAUSES] THEN
+              NONOVERLAPPING_CLAUSES; ALL] THEN
   DISCH_THEN(REPEAT_TCL CONJUNCTS_THEN ASSUME_TAC) THEN
-
-  (*** Fiddle around with the constant table stuff ***)
-
-  REWRITE_TAC[ALIGNED_BYTES_LOADED_APPEND_CLAUSE] THEN
-  REWRITE_TAC[fst MLKEM_NTT_EXEC] THEN REWRITE_TAC[BYTES_LOADED_DATA] THEN
 
   (*** Manually expand the cases in the hypotheses ***)
 
+  REWRITE_TAC[ntt_constants] THEN
   CONV_TAC(RATOR_CONV(LAND_CONV(ONCE_DEPTH_CONV
    (EXPAND_CASES_CONV THENC ONCE_DEPTH_CONV NUM_MULT_CONV)))) THEN
-
+  REWRITE_TAC[ntt_zetas_layer01234; ntt_zetas_layer56] THEN
+  CONV_TAC(ONCE_DEPTH_CONV EL_CONV) THEN
+  CONV_TAC(ONCE_DEPTH_CONV WORD_IWORD_CONV) THEN REWRITE_TAC[WORD_ADD_0] THEN
   ENSURES_INIT_TAC "s0" THEN
 
   (*** Manually restructure to match the 128-bit loads. It would be nicer
    *** if the simulation machinery did this automatically.
    ***)
 
-  MP_TAC(end_itlist CONJ (map (fun n -> READ_MEMORY_MERGE_CONV 3
-            (subst[mk_small_numeral(16*n),`n:num`]
-                  `read (memory :> bytes128(word_add a (word n))) s0`))
-            (0--31))) THEN
-  ASM_REWRITE_TAC[WORD_ADD_0] THEN
+  MEMORY_128_FROM_16_TAC "a" 32 THEN
+  MEMORY_128_FROM_16_TAC "z_01234" 10 THEN
+  MEMORY_128_FROM_16_TAC "z_56" 48 THEN
+  ASM_REWRITE_TAC[WORD_ADD_0] THEN CONV_TAC WORD_REDUCE_CONV THEN
   DISCARD_MATCHING_ASSUMPTIONS [`read (memory :> bytes16 a) s = x`] THEN
-  STRIP_TAC THEN
+  REPEAT STRIP_TAC THEN
 
-  (*** Palaver to address the precomputed tables via "wpc" ***)
+  (*** Ghost up initial contents of Q7 since it isn't fully initialized ***)
 
-  ASSUME_TAC(WORD_RULE
-   `word(pc + 0x5b8):int64 = word_add (word(pc + 0x518)) (word 160)`) THEN
-  FIRST_ASSUM(MP_TAC o GEN_REWRITE_RULE I [GSYM BYTES_LOADED_DATA]) THEN
-  ABBREV_TAC `wpc:int64 = word(pc + 0x518)` THEN
-  SUBST1_TAC(WORD_RULE `wpc:int64 = word(val wpc + 0)`) THEN
-  REWRITE_TAC[mlkem_ntt_data] THEN CONV_TAC(LAND_CONV DATA64_CONV) THEN
-  REWRITE_TAC[WORD_RULE `word(val x + n) = word_add x (word n)`] THEN
-  REWRITE_TAC[bytes_loaded_nil] THEN STRIP_TAC THEN
-  SUBGOAL_THEN `nonoverlapping (a:int64,512) (wpc:int64,928)` MP_TAC THEN
-  REWRITE_TAC[NONOVERLAPPING_CLAUSES] THENL
-   [EXPAND_TAC "wpc" THEN NONOVERLAPPING_TAC;
-    DISCH_TAC] THEN
-  MP_TAC(end_itlist CONJ (map (fun n -> READ_MEMORY_MERGE_CONV 1
-            (subst[mk_small_numeral(16*n),`n:num`]
-                  `read (memory :> bytes128(word_add wpc (word n))) s0`))
-            (0--57))) THEN
-  ASM_REWRITE_TAC[WORD_ADD_0] THEN
-  CONV_TAC(LAND_CONV(DEPTH_CONV WORD_NUM_RED_CONV)) THEN
-  DISCARD_MATCHING_ASSUMPTIONS [`read (memory :> bytes64 a) s = x`] THEN
-  STRIP_TAC THEN
+  ABBREV_TAC `v7_init:int128 = read Q7 s0` THEN
 
   (*** Simulate all the way to the end, in effect unrolling loops ***)
 
   MAP_EVERY (fun n -> ARM_STEPS_TAC MLKEM_NTT_EXEC [n] THEN SIMD_SIMPLIFY_TAC)
-            (1--909) THEN
+            (1--904) THEN
   ENSURES_FINAL_STATE_TAC THEN ASM_REWRITE_TAC[] THEN
 
   (*** Reverse the restructuring by splitting the 128-bit words up ***)
@@ -539,7 +542,7 @@ let MLKEM_NTT_CORRECT = prove
   CONV_TAC(ONCE_DEPTH_CONV let_CONV) THEN REWRITE_TAC[INT_ABS_BOUNDS] THEN
   GEN_REWRITE_TAC (BINDER_CONV o RAND_CONV) [GSYM I_THM] THEN
   CONV_TAC(EXPAND_CASES_CONV THENC ONCE_DEPTH_CONV NUM_MULT_CONV) THEN
-  ASM_REWRITE_TAC[I_THM; WORD_ADD_0] THEN DISCARD_STATE_TAC "s909" THEN
+  ASM_REWRITE_TAC[I_THM; WORD_ADD_0] THEN DISCARD_STATE_TAC "s904" THEN
   REPEAT(W(fun (asl,w) ->
      if length(conjuncts w) > 3 then CONJ_TAC else NO_TAC)) THEN
 
@@ -566,18 +569,19 @@ let MLKEM_NTT_CORRECT = prove
 (*** Subroutine form, somewhat messy elaboration of the usual wrapper ***)
 
 let MLKEM_NTT_SUBROUTINE_CORRECT = prove
- (`!a x pc stackpointer returnaddress.
+ (`!a z_01234 z_56 x pc stackpointer returnaddress.
       aligned 16 stackpointer /\
-      ALL (nonoverlapping (word_sub stackpointer (word 64),64))
-          [(word pc,0x8b8); (a,512)] /\
-      nonoverlapping (word pc,0x8b8) (a,512)
+      ALLPAIRS nonoverlapping
+       [(a,512); (word_sub stackpointer (word 64),64)]
+       [(word pc,0x504); (z_01234,160); (z_56,768)] /\
+      nonoverlapping (a,512) (word_sub stackpointer (word 64),64)
       ==> ensures arm
-           (\s. aligned_bytes_loaded s (word pc)
-                  (APPEND mlkem_ntt_mc mlkem_ntt_data) /\
+           (\s. aligned_bytes_loaded s (word pc) mlkem_ntt_mc /\
                 read PC s = word pc /\
                 read SP s = stackpointer /\
                 read X30 s = returnaddress /\
-                C_ARGUMENTS [a] s /\
+                C_ARGUMENTS [a; z_01234; z_56] s /\
+                ntt_constants z_01234 z_56 s /\
                 !i. i < 256
                     ==> read(memory :> bytes16(word_add a (word(2 * i)))) s =
                         x i)
@@ -592,14 +596,13 @@ let MLKEM_NTT_SUBROUTINE_CORRECT = prove
             MAYCHANGE [memory :> bytes(a,512);
                        memory :> bytes(word_sub stackpointer (word 64),64)])`,
   let TWEAK_CONV =
+    REWRITE_CONV[ntt_constants] THENC
     ONCE_DEPTH_CONV let_CONV THENC
     ONCE_DEPTH_CONV EXPAND_CASES_CONV THENC
     ONCE_DEPTH_CONV NUM_MULT_CONV THENC
     PURE_REWRITE_CONV [WORD_ADD_0] in
-  REWRITE_TAC[ALIGNED_BYTES_LOADED_APPEND_CLAUSE; BYTES_LOADED_DATA;
-              fst MLKEM_NTT_EXEC] THEN
+  REWRITE_TAC[fst MLKEM_NTT_EXEC] THEN
   CONV_TAC TWEAK_CONV THEN
   ARM_ADD_RETURN_STACK_TAC ~pre_post_nsteps:(5,5) MLKEM_NTT_EXEC
-   (REWRITE_RULE[ALIGNED_BYTES_LOADED_APPEND_CLAUSE; BYTES_LOADED_DATA;
-                 fst MLKEM_NTT_EXEC] (CONV_RULE TWEAK_CONV MLKEM_NTT_CORRECT))
+   (REWRITE_RULE[fst MLKEM_NTT_EXEC] (CONV_RULE TWEAK_CONV MLKEM_NTT_CORRECT))
     `[D8; D9; D10; D11; D12; D13; D14; D15]` 64);;
